Towards proving that the extensible model models the axioms

candle/overloading/semantics/holModelConservativityScript.sml
@@ -1306,7 +1306,8 @@ val type_interpretation_ext_of_def =
      One:'U
    else if ~(orth_ctxt (upd::ctxt) /\ extends_init (upd::ctxt)) then
      One:'U
-   else if ty ∈ FST (indep_frag_upd (upd::ctxt) upd (total_fragment (sigof (upd::ctxt))))  then
+   else if ty ∈ FST (indep_frag_upd (upd::ctxt) upd (total_fragment (sigof (upd::ctxt)))) ∧
+           (∀tm. upd ≠ NewAxiom tm) then
     Δ ty
    else
      case mapPartial (type_matches ty) (upd::ctxt) of
@@ -1360,7 +1361,8 @@ val type_interpretation_ext_of_def =
      One:'U
    else if ~(orth_ctxt (upd::ctxt) /\ extends_init (upd::ctxt)) then
      One:'U
-   else if (name,ty) ∈ SND (indep_frag_upd (upd::ctxt) upd (total_fragment (sigof (upd::ctxt))))  then
+   else if ((name,ty) ∈ SND (indep_frag_upd (upd::ctxt) upd (total_fragment (sigof (upd::ctxt))))) ∧
+           (∀tm. upd ≠ NewAxiom tm) then
      Γ (name,ty)
    else
      case FILTER ($<> []) (MAP (defn_matches name ty) (upd::ctxt)) of
@@ -1499,10 +1501,12 @@ val type_interpretation_ext_of_def =
     disch_then(qspec_then `INL ty` mp_tac) >>
     simp[]
   ) >>
-    rpt strip_tac
+    rpt conj_tac >> rpt gen_tac >>
+    rpt(disch_then (MAP_EVERY assume_tac o CONJUNCTS))
     (* protect ext *)
     >> qabbrev_tac `ext = upd::ctxt`
     >- (
+      qpat_x_assum ‘_ ∨ _’ kall_tac >>
       fs[subst_clos_term_ext_rel_def,subst_clos_def] >>
       drule instance_subst_soundness >> strip_tac >>
       rename1 `mapPartial _ _ = [(pred,name,tvs)]` >>
@@ -1554,6 +1558,7 @@ val type_interpretation_ext_of_def =
         rveq >> simp[]
     )
     >- (
+      qpat_x_assum ‘_ ∨ _’ kall_tac >>
       fs[subst_clos_term_ext_rel_def,subst_clos_def] >>
        drule instance_subst_soundness >> strip_tac >>
        rename1 `mapPartial _ _ = [(pred,name,tvs)]` >>
@@ -1629,6 +1634,7 @@ val type_interpretation_ext_of_def =
        rveq >> simp[]
       )
     >- (
+      qpat_x_assum ‘_ ∨ _’ kall_tac >>
       fs[subst_clos_term_ext_rel_def,subst_clos_def] >>
        drule instance_subst_soundness >> strip_tac >>
        rename1 `mapPartial _ _ = [(pred,name,tvs)]` >>
@@ -1681,6 +1687,7 @@ val type_interpretation_ext_of_def =
        metis_tac[]
     )
     >- (
+      qpat_x_assum ‘_ ∨ _’ kall_tac >>
       fs[MEM_FLAT,MEM_MAP,PULL_EXISTS] >>
        fs[subst_clos_term_ext_rel_def,subst_clos_def] >>
        drule instance_subst_soundness >> strip_tac >>
@@ -1747,7 +1754,7 @@ val type_interpretation_ext_of_def =
        simp[EXISTS_OR_THM,LEFT_AND_OVER_OR,RIGHT_AND_OVER_OR] >>
        qunabbrev_tac `aty` >> metis_tac[welltyped_def,WELLTYPED_LEMMA]
     )
-    >- (
+    >- (qpat_x_assum ‘_ ∨ _’ kall_tac >>
        fs[subst_clos_term_ext_rel_def,subst_clos_def] >>
        drule instance_subst_soundness >> strip_tac >>
        rename1 `instance_subst _ _ _ = SOME(sigma,r)` >>
@@ -1802,6 +1809,7 @@ val type_interpretation_ext_of_def =
     )
     >- (
     (* abs/rep case *)
+       qpat_x_assum ‘_ ∨ _’ kall_tac >>
        simp[subst_clos_term_ext_rel_def] >>
        FULL_CASE_TAC >>
        fs[allTypes'_defn] >>
@@ -1885,6 +1893,7 @@ val type_interpretation_ext_of_def =
         simp[EXISTS_OR_THM,LEFT_AND_OVER_OR,RIGHT_AND_OVER_OR] >>
         rveq >> fs[])) >-
       ((* abs or rep matches two distinct typedefs (impossible) *)
+       qpat_x_assum ‘_ ∨ _’ kall_tac >>
        fs[mllistTheory.mapPartial_thm,FILTER_EQ_CONS,FILTER_EQ_NIL,MAP_EQ_APPEND,MAP_EQ_CONS] >>
        rveq >>
        fs[IS_SOME_EXISTS] >>
@@ -1906,6 +1915,7 @@ val type_interpretation_ext_of_def =
        rw[updates_cases]
       ) >-
       ((* No definition matches (hence constant must have been declared with NewConst) *)
+       qpat_x_assum ‘_ ∨ _’ kall_tac >>
        fs[term_ok_def] >>
        drule ALOOKUP_MEM >>
        rw[MEM_FLAT,MEM_MAP,PULL_EXISTS] >>
@@ -1971,10 +1981,12 @@ Theorem model_conservative_extension_prop:
     ∧ inhabited ind
     ∧ is_frag_interpretation (total_fragment (sigof ctxt)) Δ Γ
     ⇒
-      (!c ty. (c,ty) ∈ SND (indep_frag_upd (upd::ctxt) upd (total_fragment (sigof (upd::ctxt))))
+      (!c ty. (c,ty) ∈ SND (indep_frag_upd (upd::ctxt) upd (total_fragment (sigof (upd::ctxt)))) ∧
+          (∀tm. upd ≠ NewAxiom tm)
         ⇒ term_interpretation_ext_of ind upd ctxt Δ Γ c ty = Γ (c,ty))
       ∧
-      (!ty. ty ∈ FST (indep_frag_upd (upd::ctxt) upd (total_fragment (sigof (upd::ctxt))))
+      (!ty. ty ∈ FST (indep_frag_upd (upd::ctxt) upd (total_fragment (sigof (upd::ctxt)))) ∧
+          (∀tm. upd ≠ NewAxiom tm)
         ⇒ type_interpretation_ext_of ind upd ctxt Δ Γ ty = Δ ty)
 Proof
   rpt strip_tac
@@ -2227,7 +2239,7 @@ Theorem interpretation_is_total_frag_interpretation_lemma:
         ∧ ty ∈ ground_types (sigof (upd::ctxt)) /\ inhabited ind /\
         ty ∈ nonbuiltin_types
     ⇒
-        inhabited (type_interpretation_ext_of0 ^mem ind upd ctxt Δ Γ ty)) /\
+        inhabited (type_interpretation_ext_of ind upd ctxt Δ Γ ty)) /\
   (∀^mem ind upd ctxt Δ Γ c ty.
      is_set_theory ^mem ⇒
         orth_ctxt (upd::ctxt) /\ terminating(subst_clos (dependency (upd::ctxt)))
@@ -2237,7 +2249,7 @@ Theorem interpretation_is_total_frag_interpretation_lemma:
         ∧ (c,ty) ∈ ground_consts (sigof (upd::ctxt)) /\ inhabited ind
         /\ (c,ty) ∈ nonbuiltin_constinsts ⇒
         term_interpretation_ext_of0 ^mem ind upd ctxt Δ Γ c ty ⋲
-        ext_type_frag_builtins (type_interpretation_ext_of0 ^mem ind upd ctxt Δ Γ) ty
+        ext_type_frag_builtins (type_interpretation_ext_of ind upd ctxt Δ Γ) ty
   )
 Proof
   ho_match_mp_tac type_interpretation_ext_of_ind >> rpt strip_tac >>
@@ -2260,6 +2272,7 @@ Proof
          fs[is_frag_interpretation_def,total_fragment_def,is_type_frag_interpretation_def]) >>
       TOP_CASE_TAC >- metis_tac[mem_one] >>
       reverse TOP_CASE_TAC >- rw[mem_one] >>
+      qpat_assum ‘~(_ ∧ (∀tm. upd ≠ NewAxiom tm))’ (fn thm => ABBREV_TAC “a1 = ^(concl thm)”) >>
       PairCases_on `h` >> rename1 `pred,ty',tvs` >>
       simp[] >>
       drule type_matches_is_instance' >>
@@ -2392,6 +2405,7 @@ Proof
                  suffices_by metis_tac[] >>
                drule_then match_mp_tac (MP_CANON ext_inhabited_frag_inhabited') >>
                metis_tac[]) >>
+            qpat_assum ‘~(_ ∧ (∀tm. upd ≠ NewAxiom tm))’ (fn thm => ABBREV_TAC “aaa = ^(concl thm)”) >>
             (* Hilbert choice *)
             fs[] >>
             fs[term_ok_def] >>
@@ -2439,6 +2453,7 @@ Proof
                drule_then match_mp_tac (MP_CANON ext_inhabited_frag_inhabited') >>
                metis_tac[]) >>
             (* Hilbert choice *)
+            qpat_assum ‘~(_ ∧ (∀tm. upd ≠ NewAxiom tm))’ (fn thm => ABBREV_TAC “aaa = ^(concl thm)”) >>
             fs[] >>
             fs[term_ok_def] >>
             simp[ext_type_frag_builtins_Fun] >>
@@ -2476,6 +2491,7 @@ Proof
          rw[] >>
          MAP_FIRST drule [rep_matches_is_instance,abs_matches_is_instance] >>
          disch_then(MAP_EVERY assume_tac o CONJUNCTS) >>
+         qpat_assum ‘~(_ ∧ (∀tm. upd ≠ NewAxiom tm))’ (fn thm => ABBREV_TAC “aaa = ^(concl thm)”) >>
          FULL_SIMP_TAC bool_ss [instance_subst_completeness] >>
          rveq >>
          fs[IS_SOME_EXISTS] >>
@@ -2779,8 +2795,8 @@ Theorem model_conservative_extension:
     ∧ is_frag_interpretation (total_fragment (sigof ctxt)) Δ Γ
     ⇒
         is_frag_interpretation (total_fragment (sigof (upd::ctxt)))
-          (type_interpretation_ext_of0 ^mem ind upd ctxt Δ Γ)
-          (UNCURRY (term_interpretation_ext_of0 ^mem ind upd ctxt Δ Γ))
+          (type_interpretation_ext_of ind upd ctxt Δ Γ)
+          (UNCURRY (term_interpretation_ext_of ind upd ctxt Δ Γ))
 Proof
   rw[]
   >> ‘ctxt extends []’ by(drule_then match_mp_tac extends_trans >> simp[init_ctxt_extends])
@@ -2808,6 +2824,3021 @@ Proof
   >> disch_then match_mp_tac
   >> asm_rewrite_tac[]
   >> goal_assum drule
+QED
+
+Theorem interpretation_is_total_frag_interpretation:
+  is_set_theory ^mem ⇒
+    ∀ctxt. orth_ctxt(upd::ctxt) /\ terminating(subst_clos (dependency(upd::ctxt))) /\ ctxt extends [] /\ ctxt extends init_ctxt /\ inhabited ind ∧ upd updates ctxt ∧
+        is_frag_interpretation (total_fragment (sigof ctxt))
+          Δ Γ
+    ⇒
+        is_frag_interpretation (total_fragment (sigof(upd::ctxt)))
+          (type_interpretation_ext_of ind upd ctxt Δ Γ)
+          (UNCURRY (term_interpretation_ext_of ind upd ctxt Δ Γ))
+Proof
+  rw[is_frag_interpretation_def,total_fragment_def,is_type_frag_interpretation_def,
+     GSYM PFORALL_THM] >>
+  MAP_FIRST (match_mp_tac o MP_CANON) (CONJUNCTS interpretation_is_total_frag_interpretation_lemma) >>
+  rw[is_frag_interpretation_def,total_fragment_def,is_type_frag_interpretation_def,
+     GSYM PFORALL_THM] >>
+  metis_tac[]
+QED
+
+(* TODO: can we state this with less typing? *)
+Theorem type_interpretation_ext_of_alt:
+  (!^mem ind ctxt ty Δ Γ. is_set_theory ^mem /\ ctxt extends init_ctxt /\
+                  is_frag_interpretation (total_fragment(sigof ctxt))
+                   (type_interpretation_ext_of ind (HD ctxt) (TL ctxt) Δ Γ)
+                   (UNCURRY (term_interpretation_ext_of ind (HD ctxt) (TL ctxt) Δ Γ)) /\
+                  ty ∈ ground_types (sigof ctxt) /\
+                  ty ∈ nonbuiltin_types ∧ ctxt ≠ []
+   ==> type_interpretation_ext_of ind (HD ctxt) (TL ctxt) Δ Γ ty =
+   if ~terminating(subst_clos (dependency ctxt)) then
+     One:'U
+   else if ~orth_ctxt ctxt then
+     One:'U
+   else if ty ∈ FST (indep_frag_upd ctxt (HD ctxt) (total_fragment (sigof ctxt)))  then
+     Δ ty
+   else
+     case mapPartial (type_matches ty) ctxt of
+     | [] =>
+       if ty = Tyapp (strlit "ind") [] then
+         ind
+       else
+         One
+     | [(pred,ty',tvs)] =>
+       (case instance_subst [(ty, (Tyapp ty' (MAP Tyvar tvs)))] [] [] of
+         | SOME(sigma,e) =>
+            let pty = domain(typeof pred);
+                consts = consts_of_term pred ∩ nonbuiltin_constinsts;
+                inst_consts = {(c,ty) | ?ty'. ty = TYPE_SUBST sigma ty' /\ (c,ty') ∈ consts};
+                sigma' = (λx. REV_ASSOCD (Tyvar x) sigma (Tyvar x));
+                γ = (λ(c,ty). term_interpretation_ext_of0 ^mem ind (HD ctxt) (TL ctxt) Δ Γ c ty);
+                δ = type_interpretation_ext_of0 ^mem ind (HD ctxt) (TL ctxt) Δ Γ;
+                tst = termsem (ext_type_frag_builtins δ)
+                              (ext_term_frag_builtins
+                                (ext_type_frag_builtins δ)
+                                γ)
+                              empty_valuation
+                              sigma'
+                              pred
+            in
+              if ?tm.
+                  tm ⋲
+                  (ext_type_frag_builtins δ (TYPE_SUBST sigma pty)
+                  suchthat (λtm. tst ' tm = True)) then
+                ext_type_frag_builtins δ (TYPE_SUBST sigma pty)
+                  suchthat (λtm. tst ' tm = True)
+              else
+                ext_type_frag_builtins δ (TYPE_SUBST sigma pty)
+         | NONE => One:'U)
+     | _ => One:'U
+  ) /\
+  (!^mem ind ctxt name ty Δ Γ.
+   is_set_theory ^mem /\ ctxt extends init_ctxt /\
+   (name,ty) ∈ ground_consts (sigof ctxt) /\
+   (name,ty) ∈ nonbuiltin_constinsts /\
+   inhabited ind ∧ ctxt ≠ [] ∧
+   is_frag_interpretation (total_fragment(sigof ctxt))
+     (type_interpretation_ext_of ind (HD ctxt) (TL ctxt) Δ Γ)
+     (UNCURRY (term_interpretation_ext_of ind (HD ctxt) (TL ctxt) Δ Γ)) ==>
+   term_interpretation_ext_of ind (HD ctxt) (TL ctxt) Δ Γ (name:mlstring) ty =
+   if ~terminating(subst_clos (dependency ctxt)) then
+     One:'U
+   else if ~orth_ctxt ctxt then
+     One:'U
+   else if (name,ty) ∈ SND (indep_frag_upd ctxt (HD ctxt) (total_fragment (sigof ctxt)))  then
+     Γ (name,ty)
+   else
+     case FILTER ($<> []) (MAP (defn_matches name ty) ctxt) of
+       [] =>
+       (case mapPartial (abs_or_rep_matches name ty) ctxt of
+        | [(is_abs,name0,abs_type,rep_type)] =>
+          (let cty = if is_abs then Fun rep_type abs_type else Fun abs_type rep_type
+           in
+             case instance_subst [(ty, cty)] [] [] of
+             | SOME(sigma,e) =>
+               let
+                 δ = type_interpretation_ext_of0 ^mem ind (HD ctxt) (TL ctxt) Δ Γ;
+                 sigma' = (λx. REV_ASSOCD (Tyvar x) sigma (Tyvar x));
+               in
+                 if is_abs then
+                   Abstract (ext_type_frag_builtins δ (TYPE_SUBST sigma rep_type))
+                            (ext_type_frag_builtins δ (TYPE_SUBST sigma abs_type))
+                            (λv. if v <: ext_type_frag_builtins δ (TYPE_SUBST sigma abs_type) then
+                                   v
+                                 else
+                                   @v. v <: ext_type_frag_builtins δ (TYPE_SUBST sigma abs_type))
+                 else
+                   Abstract (ext_type_frag_builtins δ (TYPE_SUBST sigma abs_type))
+                            (ext_type_frag_builtins δ (TYPE_SUBST sigma rep_type))
+                            I
+             | NONE => One (* cannot happen *))
+        | _ =>
+          let δ = type_interpretation_ext_of0 ^mem ind (HD ctxt) (TL ctxt) Δ Γ in
+            if name = strlit "@" /\ MEM ^select_ax ctxt /\
+               FLOOKUP (tmsof ctxt) (strlit "==>") = SOME (Fun Bool (Fun Bool Bool)) /\
+               FLOOKUP (tmsof ctxt) (strlit "@") = SOME(^select_ty)
+             then
+              Abstract (ext_type_frag_builtins δ (domain ty))
+                       (ext_type_frag_builtins δ (codomain ty))
+                       (λp.
+                         case some x. x <: (ext_type_frag_builtins δ (codomain ty)) ∧
+                                      p ' x = True of
+                           NONE => (@x. x <: ext_type_frag_builtins δ (codomain ty))
+                         | SOME v => v
+                       )
+            else
+              @v. v <: ext_type_frag_builtins δ ty
+       )
+     | l =>
+       let (name0,trm0) = HD(HD l)
+       in
+         case instance_subst [(ty, typeof trm0)] [] [] of
+         | SOME(sigma,e) =>
+           let
+             pty = domain(typeof trm0);
+             consts = consts_of_term trm0 ∩ nonbuiltin_constinsts;
+             inst_consts = {(c,ty) | ?ty'. ty = TYPE_SUBST sigma ty' /\ (c,ty') ∈ consts};
+             sigma' = (λx. REV_ASSOCD (Tyvar x) sigma (Tyvar x));
+             γ = (λ(c,ty). term_interpretation_ext_of0 ^mem ind (HD ctxt) (TL ctxt) Δ Γ c ty);
+             atys = MAP (TYPE_SUBST sigma) (allTypes trm0);
+             δ = type_interpretation_ext_of0 ^mem ind (HD ctxt) (TL ctxt) Δ Γ
+           in
+             termsem (ext_type_frag_builtins δ)
+                       (ext_term_frag_builtins
+                         (ext_type_frag_builtins δ)
+                         γ)
+                       empty_valuation
+                       sigma'
+                       trm0
+         | NONE => One (* cannot happen *)
+  )
+Proof
+  rpt strip_tac >>
+  (Cases_on ‘ctxt’ >- rw[]) >>
+  PURE_REWRITE_TAC[HD,TL] >>
+  rename1 ‘type_interpretation_ext_of ind upd ctxt’ >>
+  CONV_TAC(LHS_CONV(PURE_ONCE_REWRITE_CONV[type_interpretation_ext_of_def])) >>
+  (IF_CASES_TAC >- rw[]) >>
+  (IF_CASES_TAC >- (fs[extends_init_def,ground_consts_def] >> fs[])) >>
+  (IF_CASES_TAC >- rw[])
+  >-
+    ((* type interpretation *)
+     qpat_abbrev_tac ‘a1 = upd::ctxt’ >>
+     rename1 ‘a1 = upd::ctxt'’ >>
+     rename1 ‘ctxt = upd::ctxt'’ >>
+     ntac 6 (TOP_CASE_TAC >> fs[] >> rveq) >>
+     drule_then assume_tac instance_subst_soundness >>
+     simp[mem_sub] >>
+     qmatch_goalsub_abbrev_tac `ext_type_frag_builtins σ` >>
+     qmatch_goalsub_abbrev_tac `ext_term_frag_builtins (ext_type_frag_builtins σ') γ` >>
+     rename1 `TYPE_SUBST sigma (domain (typeof pred))` >>
+     `ext_type_frag_builtins σ (TYPE_SUBST sigma (domain (typeof pred))) =
+      ext_type_frag_builtins (type_interpretation_ext_of ind upd ctxt' Δ Γ) (TYPE_SUBST sigma (domain (typeof pred)))
+     `
+       by(match_mp_tac ext_type_frag_mono_eq >> rw[Abbr `σ`]) >>
+     simp[] >>
+     `termsem (ext_type_frag_builtins σ')
+                 (ext_term_frag_builtins (ext_type_frag_builtins σ') γ)
+                 empty_valuation (λx. REV_ASSOCD (Tyvar x) sigma (Tyvar x))
+                 pred =
+      termsem (ext_type_frag_builtins (type_interpretation_ext_of ind upd ctxt' Δ Γ))
+                 (ext_term_frag_builtins (ext_type_frag_builtins (type_interpretation_ext_of ind upd ctxt' Δ Γ))
+                                         (UNCURRY(term_interpretation_ext_of ind upd ctxt' Δ Γ)))
+                 empty_valuation (λx. REV_ASSOCD (Tyvar x) sigma (Tyvar x))
+                 pred
+     `
+      by(match_mp_tac fleq_term_interp_le_closed >>
+         qabbrev_tac `tyfrag = set(FLAT (MAP allTypes'(MAP (TYPE_SUBST sigma) (allTypes pred))))` >>
+         qabbrev_tac `tmfrag = {(c',ty') | ∃ty''.
+                                 ty' = TYPE_SUBST sigma ty'' ∧ (c',ty'') ∈ consts_of_term pred ∧
+                                 (c',ty') ∈ nonbuiltin_constinsts}` >>
+         ntac 2(qexists_tac `(tyfrag,tmfrag)`) >>
+         qexists_tac `sigof ctxt` >>
+         conj_tac >- (rw[fleq_def,Abbr `σ'`,Abbr`tmfrag`,Abbr `γ`] >> rw[] >>
+                      goal_assum kall_tac >>
+                      fs[] >>
+                      first_x_assum(qspec_then `ty''` mp_tac) >>
+                      simp[] >>
+                      fs[TYPE_SUBST_eq_TYPE_SUBSTf] >>
+                      imp_res_tac nonbuiltin_constinsts_TYPE_SUBSTf) >>
+         conj_asm1_tac >-
+           (MAP_EVERY qunabbrev_tac [`tyfrag`,`tmfrag`] >>
+            rw[is_sig_fragment_def] >>
+            fs[mllistTheory.mapPartial_thm,FILTER_EQ_CONS,MAP_EQ_APPEND,IS_SOME_EXISTS] >>
+            rveq >> fs[] >> rveq >> fs[] >>
+            fs[type_matches_def] >>
+            qpat_x_assum `SOME _ = _` (assume_tac o GSYM) >>
+            fs[CaseEq "update"] >> rveq >> fs[] >>
+            fs[MAP_EQ_f,MEM_MAP,PULL_EXISTS] >>
+            drule extends_append_MID >>
+            (impl_tac >- rw[init_ctxt_def]) >>
+            FULL_SIMP_TAC bool_ss [GSYM APPEND_ASSOC] >>
+            drule_then (assume_tac o C MATCH_MP init_ctxt_extends) extends_trans >>
+            drule extends_APPEND_NIL >> simp[] >> strip_tac >>
+            dxrule extends_NIL_CONS_updates >>
+            simp[updates_cases] >> rpt strip_tac >> rveq >> fs[] >>
+            `q' <> strlit "fun"`
+              by(drule_then strip_assume_tac extends_appends >>
+                 CCONTR_TAC >> fs[init_ctxt_def]) >>
+            `q' <> strlit "bool"`
+              by(drule_then strip_assume_tac extends_appends >>
+                 CCONTR_TAC >> fs[init_ctxt_def]) >>
+            simp[allTypes'_defn] >>
+            imp_res_tac proves_term_ok >>
+            fs[] >>
+            drule extends_NIL_APPEND_extends >> strip_tac >>
+            dxrule_then drule term_ok_extends >> strip_tac >>
+            dxrule_then (assume_tac o C MATCH_MP is_std_sig_init) is_std_sig_extends >>
+            drule_then (assume_tac o C MATCH_MP is_std_sig_init) is_std_sig_extends >>
+            fs[term_ok_clauses]
+            >- (rw[SUBSET_DEF,MEM_FLAT,MEM_MAP] >>
+                rw[ground_types_def]
+                >- (match_mp_tac allTypes'_no_tyvars >>
+                    goal_assum drule >>
+                    `!ty. MEM ty (tyvars (TYPE_SUBST sigma y')) ==> F`
+                      suffices_by(Cases_on `tyvars (TYPE_SUBST sigma y')` >> fs[DISJ_IMP_THM,FORALL_AND_THM] >> fs[]) >>
+                    rpt strip_tac >>
+                    fs[tyvars_TYPE_SUBST] >>
+                    drule_all_then assume_tac MEM_tyvars_allTypes >>
+                    first_x_assum drule >> strip_tac >>
+                    fs[ground_types_def,tyvars_def] >>
+                    drule FOLDR_LIST_UNION_empty' >>
+                    strip_tac >>
+                    fs[EVERY_MEM,MEM_MAP,PULL_EXISTS]) >>
+                drule_then match_mp_tac allTypes'_type_ok >>
+                match_mp_tac type_ok_TYPE_SUBST_strong >>
+                fs[term_ok_clauses] >>
+                conj_tac >- (drule_then drule allTypes_type_ok >> simp[]) >>
+                qpat_x_assum `_ ∈ ground_types _` assume_tac >>
+                rpt strip_tac >>
+                fs[ground_types_def,type_ok_def,EVERY_MEM,MEM_MAP,PULL_EXISTS] >>
+                drule_then drule MEM_tyvars_allTypes >> strip_tac >>
+                first_x_assum drule >>
+                first_x_assum drule >>
+                rw[])
+            >- (rw[SUBSET_DEF,MEM_FLAT,MEM_MAP] >> imp_res_tac allTypes'_nonbuiltin)
+            >- (rw[SUBSET_DEF] >>
+                fs[ground_consts_def] >>
+                conj_tac >-
+                  (simp[ground_types_def] >>
+                   conj_tac >-
+                     (`!ty. MEM ty (tyvars (TYPE_SUBST sigma ty'')) ==> F`
+                      suffices_by(Cases_on `tyvars (TYPE_SUBST sigma ty'')` >> fs[DISJ_IMP_THM,FORALL_AND_THM] >> fs[]) >>
+                      rpt strip_tac >>
+                      fs[tyvars_TYPE_SUBST] >>
+                      drule_then drule consts_of_term_tyvars_tvars >>
+                      fs[ground_types_def,tyvars_def] >>
+                      drule FOLDR_LIST_UNION_empty' >>
+                      strip_tac >>
+                      fs[EVERY_MEM,MEM_MAP,PULL_EXISTS] >>
+                      spose_not_then strip_assume_tac >>
+                      ntac 2(first_x_assum drule) >> rpt strip_tac >>
+                      fs[]) >>
+                   drule_then drule consts_of_term_term_ok >>
+                   strip_tac >>
+                   drule (ONCE_REWRITE_RULE[CONJ_SYM] term_ok_type_ok) >>
+                   impl_tac >- rfs[] >>
+                   simp[] >>
+                   strip_tac >>
+                   drule_then match_mp_tac type_ok_TYPE_SUBST_strong >>
+                   rpt strip_tac >>
+                   drule_then drule consts_of_term_tyvars_tvars >>
+                   strip_tac >>
+                   fs[ground_types_def] >>
+                   qpat_x_assum `type_ok _ (Tyapp _ _)` mp_tac >>
+                   rw[type_ok_def,EVERY_MEM,MEM_MAP,PULL_EXISTS]) >>
+                drule_then drule consts_of_term_term_ok >>
+                strip_tac >>
+                fs[term_ok_def] >>
+                reverse conj_tac >- (metis_tac[TYPE_SUBST_compose]) >>
+                pop_assum(SUBST_ALL_TAC o GSYM) >>
+                drule_then match_mp_tac type_ok_TYPE_SUBST_strong >>
+                rpt strip_tac >>
+                drule_then drule consts_of_term_tyvars_tvars >>
+                strip_tac >>
+                fs[ground_types_def] >>
+                qpat_x_assum `type_ok _ (Tyapp _ _)` mp_tac >>
+                rw[type_ok_def,EVERY_MEM,MEM_MAP,PULL_EXISTS])
+            >- (rw[SUBSET_DEF] >> rw[])
+            >- (simp[TYPE_SUBST_eq_TYPE_SUBSTf] >>
+                match_mp_tac builtin_closure_allTypes''' >>
+                rw[MEM_FLAT,MEM_MAP,PULL_EXISTS] >>
+                drule_then drule allTypes'_consts_of_term_IMP >>
+                metis_tac[TYPE_SUBST_eq_TYPE_SUBSTf])) >>
+         conj_tac >-
+           (MAP_EVERY qunabbrev_tac [`tyfrag`,`tmfrag`] >>
+            rw[terms_of_frag_uninst_def,IMAGE_DEF,SUBSET_DEF,INTER_DEF,PAIR_MAP,TYPE_SUBST_eq_TYPE_SUBSTf]
+            >- (rename1 `SND pp` >> qexists_tac `SND pp` >> rw[])
+            >- (fs[MEM_FLAT,MEM_MAP,PULL_EXISTS,TYPE_SUBST_eq_TYPE_SUBSTf] >> metis_tac[])
+            >- (fs[mllistTheory.mapPartial_thm,FILTER_EQ_CONS,MAP_EQ_APPEND,IS_SOME_EXISTS] >>
+                rveq >> fs[] >> rveq >> fs[] >>
+                fs[type_matches_def] >>
+                qpat_x_assum `SOME _ = _` (assume_tac o GSYM) >>
+                fs[CaseEq "update"] >> rveq >> fs[] >>
+                fs[MAP_EQ_f,MEM_MAP,PULL_EXISTS] >>
+                drule extends_append_MID >>
+                (impl_tac >- rw[init_ctxt_def]) >>
+                FULL_SIMP_TAC bool_ss [GSYM APPEND_ASSOC] >>
+                drule_then (assume_tac o C MATCH_MP init_ctxt_extends) extends_trans >>
+                drule extends_APPEND_NIL >> simp[] >> strip_tac >>
+                dxrule extends_NIL_CONS_updates >>
+                simp[updates_cases] >> rpt strip_tac >> rveq >> fs[] >>
+                imp_res_tac proves_term_ok >>
+                fs[] >>
+                drule extends_NIL_APPEND_extends >> strip_tac >>
+                dxrule_then drule term_ok_extends >> strip_tac >>
+                dxrule_then (assume_tac o C MATCH_MP is_std_sig_init) is_std_sig_extends >>
+                drule_then (assume_tac o C MATCH_MP is_std_sig_init) is_std_sig_extends >>
+                fs[term_ok_clauses])) >>
+           conj_tac >- simp[] >>
+           conj_tac >-
+             (qunabbrev_tac `σ'` >> qunabbrev_tac `γ` >>
+              qmatch_goalsub_abbrev_tac `is_frag_interpretation _ _ γ'` >>
+              `?whatevz. γ' = (λ(c,ty'). if (c,ty') ∈ tmfrag then term_interpretation_ext_of ind upd ctxt' Δ Γ c ty' else whatevz c ty')`
+                by(qexists_tac `CURRY γ'` >>
+                   rw[Abbr `γ'`] >> simp[FUN_EQ_THM] >> rpt strip_tac >>
+                   IF_CASES_TAC >- rw[] >>
+                   rw[Abbr `tmfrag`] >>
+                   fs[] >>
+                   rename1 `(_,tya) ∈ consts_of_term _` >>
+                   goal_assum kall_tac >>
+                   first_x_assum(qspec_then `tya` mp_tac) >>
+                   rw[] >>
+                   fs[TYPE_SUBST_eq_TYPE_SUBSTf] >>
+                   imp_res_tac nonbuiltin_constinsts_TYPE_SUBSTf) >>
+              pop_assum SUBST_ALL_TAC >>
+              pop_assum kall_tac >>
+              match_mp_tac(GEN_ALL is_frag_intepretation_ifI) >>
+              HINT_EXISTS_TAC >> simp[] >>
+              Q.SUBGOAL_THEN ‘HD ctxt = upd’ SUBST_ALL_TAC >- rw[Abbr ‘ctxt’] >>
+              Q.SUBGOAL_THEN ‘TL ctxt = ctxt'’ SUBST_ALL_TAC >- rw[Abbr ‘ctxt’] >>
+              drule_then match_mp_tac is_frag_interpretation_mono >>
+              strip_tac >> imp_res_tac total_fragment_is_top_fragment) >>
+           fs[mllistTheory.mapPartial_thm,FILTER_EQ_CONS,MAP_EQ_APPEND,IS_SOME_EXISTS] >>
+           rveq >> fs[] >> rveq >> fs[] >>
+           fs[type_matches_def] >>
+           qpat_x_assum `SOME _ = _` (assume_tac o GSYM) >>
+           fs[CaseEq "update"] >> rveq >> fs[] >>
+           fs[MAP_EQ_f,MEM_MAP,PULL_EXISTS] >>
+           drule extends_append_MID >>
+           (impl_tac >- rw[init_ctxt_def]) >>
+           FULL_SIMP_TAC bool_ss [GSYM APPEND_ASSOC] >>
+           drule_then (assume_tac o C MATCH_MP init_ctxt_extends) extends_trans >>
+           drule extends_APPEND_NIL >> simp[] >> strip_tac >>
+           dxrule extends_NIL_CONS_updates >>
+           simp[updates_cases] >> rpt strip_tac >> rveq >> fs[]) >>
+     ntac 2 (pop_assum SUBST_ALL_TAC) >>
+     simp[ELIM_UNCURRY]) >>
+  qpat_abbrev_tac ‘a1 = upd::ctxt’ >>
+  rename1 ‘a1 = upd::ctxt'’ >>
+  rename1 ‘ctxt = upd::ctxt'’ >>
+  TOP_CASE_TAC >-
+    ((* Type definition matches (so const is abs/rep) *)
+     TOP_CASE_TAC >-
+       (reverse IF_CASES_TAC >- fs[ground_consts_def] >>
+        simp[] >>
+        reverse IF_CASES_TAC >-
+         (simp[] >>
+          qmatch_goalsub_abbrev_tac `ext_type_frag_builtins σ` >>
+          `ext_type_frag_builtins σ ty = ext_type_frag_builtins (type_interpretation_ext_of ind upd ctxt' Δ Γ) ty`
+            by(match_mp_tac ext_type_frag_mono_eq >>
+               rw[Abbr `σ`]) >>
+          simp[]) >>
+        (* Hilbert choice *)
+        fs[term_ok_def] >>
+        simp[ext_type_frag_builtins_Fun,ext_type_frag_builtins_Bool] >>
+        qmatch_goalsub_abbrev_tac `ext_type_frag_builtins δ` >>
+        `ext_type_frag_builtins δ (REV_ASSOCD (Tyvar «A» ) i (Tyvar «A» )) =
+         ext_type_frag_builtins (type_interpretation_ext_of ind upd ctxt' Δ Γ)
+                                (REV_ASSOCD (Tyvar «A» ) i (Tyvar «A» ))`
+          by(match_mp_tac ext_type_frag_mono_eq >> rw[allTypes'_defn,Abbr`δ`]) >>
+        pop_assum SUBST_ALL_TAC >>
+        drule_then match_mp_tac abstract_eq >>
+        rw[] >>
+        rw[some_def] >> SELECT_ELIM_TAC >> simp[] >- metis_tac[] >>
+        drule_then match_mp_tac ext_inhabited_frag_inhabited >>
+        qexists_tac `sigof ctxt` >>
+        conj_asm1_tac >-
+          (fs[ground_consts_def,ground_types_def,LIST_UNION_EQ_NIL,
+              term_ok_def,tyvars_def,type_ok_def] >>
+           metis_tac[]) >>
+        rw[] >>
+        Q.SUBGOAL_THEN ‘HD ctxt = upd’ SUBST_ALL_TAC >- rw[Abbr ‘ctxt’] >>
+        Q.SUBGOAL_THEN ‘TL ctxt = ctxt'’ SUBST_ALL_TAC >- rw[Abbr ‘ctxt’] >>
+        fs[is_frag_interpretation_def,total_fragment_def,is_type_frag_interpretation_def]) >>
+     reverse TOP_CASE_TAC >-
+       (reverse IF_CASES_TAC >- fs[ground_consts_def] >>
+        simp[] >>
+        reverse IF_CASES_TAC >-
+         (simp[] >>
+          qmatch_goalsub_abbrev_tac `ext_type_frag_builtins σ` >>
+          `ext_type_frag_builtins σ ty = ext_type_frag_builtins (type_interpretation_ext_of ind upd ctxt' Δ Γ) ty`
+            by(match_mp_tac ext_type_frag_mono_eq >>
+               rw[Abbr `σ`]) >>
+          simp[]) >>
+        (* Hilbert choice *)
+        fs[term_ok_def] >>
+        simp[ext_type_frag_builtins_Fun,ext_type_frag_builtins_Bool] >>
+        qmatch_goalsub_abbrev_tac `ext_type_frag_builtins δ` >>
+        `ext_type_frag_builtins δ (REV_ASSOCD (Tyvar «A» ) i (Tyvar «A» )) =
+         ext_type_frag_builtins (type_interpretation_ext_of ind upd ctxt' Δ Γ)
+                                (REV_ASSOCD (Tyvar «A» ) i (Tyvar «A» ))`
+          by(match_mp_tac ext_type_frag_mono_eq >> rw[allTypes'_defn,Abbr`δ`]) >>
+        pop_assum SUBST_ALL_TAC >>
+        drule_then match_mp_tac abstract_eq >>
+        rw[] >>
+        rw[some_def] >> SELECT_ELIM_TAC >> simp[] >- metis_tac[] >>
+        drule_then match_mp_tac ext_inhabited_frag_inhabited >>
+        qexists_tac `sigof ctxt` >>
+        conj_asm1_tac >-
+          (fs[ground_consts_def,ground_types_def,LIST_UNION_EQ_NIL,
+              term_ok_def,tyvars_def,type_ok_def] >>
+           metis_tac[]) >>
+        rw[] >>
+        Q.SUBGOAL_THEN ‘HD ctxt = upd’ SUBST_ALL_TAC >- rw[Abbr ‘ctxt’] >>
+        Q.SUBGOAL_THEN ‘TL ctxt = ctxt'’ SUBST_ALL_TAC >- rw[Abbr ‘ctxt’] >>
+        fs[is_frag_interpretation_def,total_fragment_def,is_type_frag_interpretation_def]) >>
+     simp[] >>
+     ntac 5 TOP_CASE_TAC >>
+     simp[allTypes'_defn] >>
+     rename1 `TYPE_SUBST sigma` >>
+     rename1 `(is_abs,_,abs_type,rep_type)` >> rw[] >>
+     qmatch_goalsub_abbrev_tac `ext_type_frag_builtins σ` >>
+     `ext_type_frag_builtins σ (TYPE_SUBST sigma rep_type) = ext_type_frag_builtins (type_interpretation_ext_of ind upd ctxt' Δ Γ) (TYPE_SUBST sigma rep_type)`
+       by(match_mp_tac ext_type_frag_mono_eq >>
+          rw[Abbr `σ`]) >>
+     `ext_type_frag_builtins σ (TYPE_SUBST sigma abs_type) = ext_type_frag_builtins (type_interpretation_ext_of ind upd ctxt' Δ Γ) (TYPE_SUBST sigma abs_type)`
+       by(match_mp_tac ext_type_frag_mono_eq >>
+          rw[Abbr `σ`]) >>
+     ntac 2 (pop_assum SUBST_ALL_TAC) >> simp[]) >>
+  (* Definition matches *)
+  rename1 `elem ⋲ ind` >>
+  fs[FILTER_EQ_CONS] >>
+  rpt(pairarg_tac >> fs[] >> rveq) >>
+  rename1 `HD ll` >> Cases_on `ll` >> fs[] >> rveq >>
+  fs[MAP_EQ_APPEND,MAP_EQ_CONS] >> rveq >> fs[] >>
+  qpat_x_assum `_ = defn_matches _ _ _` (assume_tac o GSYM) >>
+  drule defn_matches_is_instance >>
+  disch_then(MAP_EVERY assume_tac o CONJUNCTS) >>
+  FULL_SIMP_TAC bool_ss [instance_subst_completeness] >>
+  rveq >>
+  fs[IS_SOME_EXISTS] >>
+  rename1 `instance_subst _ _ _ = SOME result` >>
+  Cases_on `result` >>
+  rename1 `instance_subst _ _ _ = SOME(sigma,result)` >>
+  drule_then assume_tac instance_subst_soundness >>
+  fs[] >>
+  FULL_SIMP_TAC std_ss [GSYM APPEND_ASSOC] >>
+  drule_then (assume_tac o C MATCH_MP init_ctxt_extends) extends_trans >>
+  drule_then (strip_assume_tac o REWRITE_RULE[APPEND]) extends_APPEND_NIL >>
+  dxrule_then strip_assume_tac extends_NIL_CONS_updates >>
+  drule_then (dxrule_then strip_assume_tac) defn_matches_wf >>
+  fs[] >>
+  dxrule_then (drule_then strip_assume_tac) term_ok_extends_APPEND >>
+  rw[] >>
+  qmatch_goalsub_abbrev_tac `termsem (ext_type_frag_builtins σ) (ext_term_frag_builtins (ext_type_frag_builtins σ) γ)` >>
+  qabbrev_tac `tyfrag = set(FLAT(MAP allTypes' (MAP (TYPE_SUBST sigma) (allTypes trm0))))` >>
+  qabbrev_tac `tmfrag = {(c',ty') | ∃ty''.
+                              ty' =
+                              TYPE_SUBSTf (λx. REV_ASSOCD (Tyvar x) sigma (Tyvar x))
+                              ty'' ∧ (c',ty'') ∈ consts_of_term trm0 ∧
+                              (c',ty') ∈ nonbuiltin_constinsts}` >>
+  drule_then (assume_tac o C MATCH_MP is_std_sig_init) is_std_sig_extends >>
+  match_mp_tac fleq_term_interp_le_closed >>
+  ntac 2 (qexists_tac `(tyfrag,tmfrag)`) >>
+  rename1 ‘type_interpretation_ext_of _ upd'’ >>
+  rename1 `ctxt1 ++ [upd] ++ ctxt2` >>
+  qexists_tac `sigof(ctxt1 ++ [upd] ++ ctxt2)` >>
+  conj_tac >- (rw[fleq_def,Abbr `σ`,Abbr`tmfrag`,Abbr `γ`] >> rw[] >>
+               goal_assum kall_tac >>
+               fs[] >>
+               first_x_assum(qspec_then `ty''` mp_tac) >>
+               simp[] >>
+               fs[TYPE_SUBST_eq_TYPE_SUBSTf] >>
+               imp_res_tac nonbuiltin_constinsts_TYPE_SUBSTf) >>
+  conj_asm1_tac >-
+    (MAP_EVERY qunabbrev_tac [`tyfrag`,`tmfrag`] >>
+     rw[is_sig_fragment_def]
+     >- (rw[SUBSET_DEF,MEM_FLAT,MEM_MAP] >>
+         rw[ground_types_def] >-
+           (fs[ground_consts_def,ground_types_def] >>
+            drule allTypes_TYPE_SUBST_no_tyvars >>
+            rpt(disch_then drule) >> strip_tac >>
+            `!tv. MEM tv (tyvars x) ==> F`
+              suffices_by(Cases_on `tyvars x` >> fs[FORALL_AND_THM]) >>
+            rpt strip_tac >>
+            drule_all_then assume_tac MEM_tyvars_allTypes' >>
+            rfs[]) >>
+         match_mp_tac allTypes'_type_ok >>
+         goal_assum drule >>
+         drule_all_then assume_tac allTypes_type_ok >>
+         match_mp_tac type_ok_TYPE_SUBST_strong >>
+         fs[] >> rw[] >>
+         fs[ground_consts_def] >>
+         drule_then dxrule term_ok_type_ok >>
+         drule_then dxrule term_ok_type_ok >>
+         rw[] >>
+         drule type_ok_TYPE_SUBST_imp >>
+         simp[] >>
+         disch_then match_mp_tac >>
+         drule_then (drule_then assume_tac) MEM_tyvars_allTypes >>
+         res_tac)
+     >- (rw[SUBSET_DEF,MEM_FLAT,MEM_MAP] >> imp_res_tac allTypes'_nonbuiltin)
+     >- (rw[SUBSET_DEF] >>
+         simp[GSYM TYPE_SUBST_eq_TYPE_SUBSTf] >>
+         match_mp_tac(GEN_ALL ground_consts_TYPE_SUBST_lemma) >>
+         simp[] >>
+         goal_assum drule >>
+         simp[] >>
+         rfs[])
+     >- (rw[SUBSET_DEF] >> simp[])
+     >- (
+         match_mp_tac builtin_closure_allTypes''' >>
+         rw[MEM_FLAT,MEM_MAP,PULL_EXISTS] >>
+         drule_then (drule_then assume_tac) allTypes'_consts_of_term_IMP >>
+         goal_assum drule >>
+         rw[TYPE_SUBST_eq_TYPE_SUBSTf])) >>
+  conj_tac >-
+    (MAP_EVERY qunabbrev_tac [`tyfrag`,`tmfrag`] >>
+     rw[terms_of_frag_uninst_def,IMAGE_DEF,SUBSET_DEF,INTER_DEF,PAIR_MAP]
+     >- (rename1 `SND pp` >>
+         qexists_tac `SND pp` >>
+         rw[])
+     >- rw[TYPE_SUBST_eq_TYPE_SUBSTf |> Q.GEN `ty` |> REWRITE_RULE[GSYM FUN_EQ_THM]]) >>
+  conj_tac >- simp[] >>
+  conj_tac >-
+    (qunabbrev_tac `σ` >> qunabbrev_tac `γ` >>
+     qmatch_goalsub_abbrev_tac `is_frag_interpretation _ _ γ'` >>
+     `?whatevz. γ' = (λ(c,ty'). if (c,ty') ∈ tmfrag then term_interpretation_ext_of ind upd' ctxt' Δ Γ c ty' else whatevz c ty')`
+       by(qexists_tac `CURRY γ'` >>
+          rw[Abbr `γ'`] >> simp[FUN_EQ_THM] >> rpt strip_tac >>
+          IF_CASES_TAC >- rw[] >>
+          rw[Abbr `tmfrag`] >>
+          fs[] >>
+          rename1 `(_,tya) ∈ consts_of_term _` >>
+          goal_assum kall_tac >>
+          first_x_assum(qspec_then `tya` mp_tac) >>
+          rw[] >>
+          fs[TYPE_SUBST_eq_TYPE_SUBSTf] >>
+          imp_res_tac nonbuiltin_constinsts_TYPE_SUBSTf) >>
+     pop_assum SUBST_ALL_TAC >>
+     pop_assum kall_tac >>
+     match_mp_tac(GEN_ALL is_frag_intepretation_ifI) >>
+     HINT_EXISTS_TAC >> simp[] >>
+     fs[markerTheory.Abbrev_def] >>
+     drule_then match_mp_tac is_frag_interpretation_mono >>
+     strip_tac >> imp_res_tac total_fragment_is_top_fragment >> fs[] >>
+     rveq >> fs[]
+     ) >>
+  fs[mllistTheory.mapPartial_thm,FILTER_EQ_CONS,MAP_EQ_APPEND,IS_SOME_EXISTS] >>
+  rveq >> fs[] >> rveq >> fs[] >>
+  fs[type_matches_def] >>
+  fs[CaseEq "update"] >> rveq >> fs[] >>
+  fs[MAP_EQ_f,MEM_MAP,PULL_EXISTS] >>
+  drule extends_append_MID >>
+  (impl_tac >- rw[init_ctxt_def]) >>
+  FULL_SIMP_TAC bool_ss [GSYM APPEND_ASSOC] >>
+  drule_then (assume_tac o C MATCH_MP init_ctxt_extends) extends_trans >>
+  drule extends_APPEND_NIL >> simp[] >> strip_tac >>
+  dxrule extends_NIL_CONS_updates >>
+  simp[updates_cases] >> rpt strip_tac >> rveq >> fs[]
+QED
+
+Theorem interpretation_models_axioms_lemma:
+  is_set_theory ^mem ⇒
+  ∀ctxt1 upd ctxt2 p Δ Γ.
+    upd updates ctxt2 /\ theory_ok(thyof(ctxt1 ++ upd::ctxt2)) /\
+    is_frag_interpretation (total_fragment (sigof (ctxt1 ++ upd::ctxt2)))
+      (type_interpretation_ext_of ind (HD (ctxt1 ++ upd::ctxt2)) (TL (ctxt1 ++ upd::ctxt2)) Δ Γ)
+      (UNCURRY (term_interpretation_ext_of ind (HD (ctxt1 ++ upd::ctxt2)) (TL (ctxt1 ++ upd::ctxt2)) Δ Γ)) /\
+    is_sig_fragment (sigof (ctxt1 ++ upd::ctxt2)) (total_fragment (sigof (ctxt1 ++ upd::ctxt2))) /\
+    ctxt2 extends init_ctxt /\
+    ctxt1 ++ upd::ctxt2 extends init_ctxt /\
+    is_std_sig (sigof(ctxt1 ++ upd::ctxt2)) /\
+    is_std_sig (sigof(ctxt2)) /\
+    inhabited ind /\
+    (∀p. MEM (NewAxiom p) (upd::ctxt2) ⇒
+          MEM (NewAxiom p) ctxt2 \/
+          admissible_axiom mem ind upd ctxt2
+    ) /\
+    orth_ctxt (ctxt1 ++ upd::ctxt2) /\
+    terminating (subst_clos (dependency (ctxt1 ++ upd::ctxt2))) /\
+    (∀p. MEM p (axiom_list ctxt2) ==>
+          satisfies_t (sigof (ctxt1 ++ upd::ctxt2))
+          (ext_type_frag_builtins (type_interpretation_ext_of ind (HD (ctxt1 ++ upd::ctxt2)) (TL (ctxt1 ++ upd::ctxt2)) Δ Γ))
+          (ext_term_frag_builtins
+             (ext_type_frag_builtins (type_interpretation_ext_of ind (HD (ctxt1 ++ upd::ctxt2)) (TL (ctxt1 ++ upd::ctxt2)) Δ Γ))
+             (UNCURRY (term_interpretation_ext_of ind (HD (ctxt1 ++ upd::ctxt2)) (TL (ctxt1 ++ upd::ctxt2)) Δ Γ))) ([],p)) /\
+    models Δ Γ (thyof(TL((ctxt1 ++ upd::ctxt2)))) ∧
+    MEM p (axioms_of_upd upd)
+    ==>
+    satisfies_t (sigof (ctxt1 ++ upd::ctxt2))
+          (ext_type_frag_builtins (type_interpretation_ext_of ind (HD (ctxt1 ++ upd::ctxt2)) (TL (ctxt1 ++ upd::ctxt2)) Δ Γ))
+          (ext_term_frag_builtins
+             (ext_type_frag_builtins (type_interpretation_ext_of ind  (HD (ctxt1 ++ upd::ctxt2)) (TL (ctxt1 ++ upd::ctxt2)) Δ Γ))
+             (UNCURRY (term_interpretation_ext_of ind (HD (ctxt1 ++ upd::ctxt2)) (TL (ctxt1 ++ upd::ctxt2)) Δ Γ))) ([],p)
+Proof
+  cheat
+(*
+  rw[updates_cases,axexts_of_upd_def,DISJ_IMP_THM] >>
+  fs[axexts_of_upd_def] >> rveq
+  >- ((* pre-existing axiom *)
+      first_x_assum match_mp_tac >>
+      pop_assum(strip_assume_tac o REWRITE_RULE[MEM_SPLIT]) >>
+      fs[])
+  >- ((* new axiom *)
+      fs[admissible_axiom_def]
+      >- ((* ETA axiom*)
+          fs[mk_eta_ctxt_def] >>
+          rw[satisfies_t_def,satisfies_def,termsem_def] >>
+          dep_rewrite.DEP_REWRITE_TAC[termsem_ext_equation |> REWRITE_RULE[termsem_ext_def]] >>
+          simp[] >>
+          conj_tac >-
+            (goal_assum drule >>
+             fs[valuates_frag_builtins] >>
+             drule_then drule terms_of_frag_uninst_equationE >>
+             impl_tac >- (simp[welltyped_equation]) >>
+             rw[] >>
+             simp[term_ok_equation] >>
+             simp[term_ok_clauses]) >>
+          simp[boolean_eq_true] >>
+          simp[termsem_def] >>
+          simp[UPDATE_def] >>
+          qmatch_goalsub_abbrev_tac `type_interpretation_ext_of _ (HD ctxt)` >>
+          `v («f» ,Fun (Tyvar «A» ) (Tyvar «B» )) ⋲
+             ext_type_frag_builtins (type_interpretation_ext_of ind (HD ctxt) (TL ctxt) Δ Γ)
+                                    (TYPE_SUBSTf sigma (Fun (Tyvar «A» ) (Tyvar «B» )))`
+            by(FULL_SIMP_TAC bool_ss [valuates_frag_builtins] >>
+               FULL_SIMP_TAC bool_ss [valuates_frag_def] >>
+               first_x_assum match_mp_tac >>
+               match_mp_tac TYPE_SUBSTf_in_types_of_frag_I >>
+               qexists_tac `Var ARB (Fun (Tyvar «A» ) (Tyvar «B» ))` >>
+               simp[VFREE_IN_def] >>
+               goal_assum drule >>
+               match_mp_tac terms_of_frag_uninst_term_ok >>
+               simp[] >>
+               simp[term_ok_def] >>
+               metis_tac[term_ok_clauses,FST]) >>
+          fs[ext_type_frag_builtins_Fun] >>
+          drule_then drule in_funspace_abstract >>
+          rw[] >> rw[] >>
+          drule_then match_mp_tac abstract_eq >>
+          simp[] >>
+          rw[] >> simp[apply_abstract])
+      >- ((* Axiom of choice *)
+          fs[mk_select_ctxt_def] >>
+          rw[satisfies_t_def,satisfies_def] >>
+          `ALOOKUP (const_list ctxt1) (strlit "@") = NONE`
+            by(drule_then (assume_tac o C MATCH_MP init_ctxt_extends) extends_trans >>
+               drule extends_NIL_DISJOINT >>
+               simp[ALOOKUP_NONE]) >>
+          `ALOOKUP (const_list ctxt1) (strlit "==>") = NONE`
+            by(drule_then (assume_tac o C MATCH_MP init_ctxt_extends) extends_trans >>
+               drule extends_NIL_DISJOINT >>
+               simp[ALOOKUP_NONE,holBoolSyntaxTheory.mk_bool_ctxt_def]) >>
+          rename1 `mk_bool_ctxt ctxt3` >>
+          qmatch_goalsub_abbrev_tac `ext_term_frag_builtins (ext_type_frag_builtins δ) γ` >>
+          qmatch_asmsub_abbrev_tac `ctxt extends init_ctxt` >>
+          `is_bool_interpretation_ext (sigof ctxt) δ γ`
+            by(drule_then match_mp_tac extends_is_bool_interpretation >>
+               qexists_tac `ctxt3` >>
+               qexists_tac `axsof (mk_bool_ctxt ctxt3)` >>
+               conj_tac >-
+                 (qpat_x_assum `NewConst _ _ :: _ extends _` assume_tac >>
+                  drule extends_appends >>
+                  strip_tac >>
+                  Cases_on `c` >- fs[init_ctxt_def] >>
+                  fs[] >>
+                  rveq >>
+                  drule(extends_append_MID |> Q.INST [`a`|->`[]`] |> REWRITE_RULE [APPEND]) >>
+                  impl_tac >- rw[init_ctxt_def] >>
+                  strip_tac >>
+                  drule_then (assume_tac o C MATCH_MP init_theory_ok) extends_theory_ok >>
+                  fs[]) >>
+               `ctxt extends mk_bool_ctxt ctxt3`
+                 by(qunabbrev_tac `ctxt` >>
+                    `mk_bool_ctxt ctxt3 = [] ++ mk_bool_ctxt ctxt3` by simp[] >>
+                    pop_assum(fn thm => PURE_ONCE_REWRITE_TAC[Once thm]) >>
+                    PURE_REWRITE_TAC[GSYM(CONJUNCT2 APPEND)] >>
+                    PURE_REWRITE_TAC[APPEND_ASSOC] >>
+                    match_mp_tac extends_NIL_APPEND_extends >>
+                    drule_then(assume_tac o C MATCH_MP init_ctxt_extends) extends_trans >>
+                    PURE_REWRITE_TAC[GSYM APPEND_ASSOC,APPEND] >> simp[]) >>
+               drule extends_sub >>
+               rw[] >>
+               simp[models_def] >>
+               fs[Abbr `ctxt`]) >>
+          fs[is_bool_interpretation_ext_def,is_bool_interpretation_def,
+             is_implies_interpretation_def] >>
+          simp[termsem_def] >>
+          dep_rewrite.DEP_ONCE_REWRITE_TAC[apply_boolrel_rw] >> simp[] >>
+          fs[valuates_frag_builtins] >> fs[valuates_frag_def] >>
+          `v («P» ,Fun (Tyvar «A» ) Bool) ⋲ ext_type_frag_builtins δ (TYPE_SUBSTf sigma (Fun (Tyvar «A» ) Bool))`
+            by(first_x_assum match_mp_tac >>
+               match_mp_tac TYPE_SUBSTf_in_types_of_frag_I >>
+               Q.REFINE_EXISTS_TAC `Var _ _` >>
+               simp[VFREE_IN_def] >>
+               goal_assum drule >>
+               qexists_tac `ARB` >>
+               match_mp_tac terms_of_frag_uninst_term_ok >>
+               conj_tac >- (rw[term_ok_def] >> metis_tac[term_ok_clauses,FST]) >>
+               simp[]) >>
+          `v («x» ,Tyvar «A») ⋲ ext_type_frag_builtins δ (TYPE_SUBSTf sigma (Tyvar «A»))`
+            by(first_x_assum match_mp_tac >>
+               match_mp_tac TYPE_SUBSTf_in_types_of_frag_I >>
+               Q.REFINE_EXISTS_TAC `Var _ _` >>
+               simp[VFREE_IN_def] >>
+               goal_assum drule >>
+               qexists_tac `ARB` >>
+               match_mp_tac terms_of_frag_uninst_term_ok >>
+               conj_tac >- (rw[term_ok_def] >> metis_tac[term_ok_clauses,FST]) >>
+               simp[]) >>
+          fs[ext_type_frag_builtins_Bool,ext_type_frag_builtins_Fun] >>
+          drule_then drule in_funspace_abstract >>
+          strip_tac >> rveq >>
+          simp[] >>
+          simp[ext_term_frag_builtins_def] >>
+          `γ (strlit "@",Fun (Fun (sigma(strlit "A")) Bool) (sigma(strlit "A"))) =
+           Abstract (ext_type_frag_builtins δ (Fun (sigma(strlit "A")) Bool))
+                          (ext_type_frag_builtins δ (sigma(strlit "A")))
+                          (λp.
+                            case some x. (^mem x (ext_type_frag_builtins δ (sigma(strlit "A"))) ∧
+                                         p ' x = True) of
+                              NONE => (@x. ^mem x (ext_type_frag_builtins δ (sigma(strlit "A"))))
+                            | SOME x => x)`
+            by(rw[Abbr `γ`,Abbr `δ`] >>
+               dep_rewrite.DEP_ONCE_REWRITE_TAC[CONJUNCT2 type_interpretation_ext_of_alt] >>
+               simp[] >>
+               conj_tac >-
+                 (simp[Abbr `ctxt`] >>
+                  simp[nonbuiltin_constinsts_def,builtin_consts_def,ground_consts_def,ground_types_def,tyvars_def] >>
+                  fs[GSYM FUNION_ASSOC,FUNION_FUPDATE_1] >>
+                  reverse conj_tac >- metis_tac[] >>
+                  conj_asm1_tac >- (metis_tac[term_ok_clauses,FST]) >>
+                  simp[term_ok_def,FLOOKUP_FUNION,FLOOKUP_UPDATE] >>
+                  qexists_tac `[(sigma «A»,Tyvar «A»)]` >>
+                  EVAL_TAC) >>
+               IF_CASES_TAC >-
+                 (
+                  )
+               reverse TOP_CASE_TAC >-
+                 (goal_assum kall_tac >>
+                  pop_assum mp_tac >> simp[] >>
+                  qmatch_goalsub_abbrev_tac `FILTER fff lll` >>
+                  `FILTER fff lll = []` suffices_by simp[] >>
+                  MAP_EVERY qunabbrev_tac [`fff`,`lll`] >>
+                  rw[FILTER_EQ_NIL,EVERY_MEM,MEM_MAP] >>
+                  fs[Abbr `ctxt`,defn_matches_NewAxiom,defn_matches_NewConst] >-
+                    (simp[defn_matches_def] >>
+                     TOP_CASE_TAC >> simp[] >>
+                     CONV_TAC SYM_CONV >>
+                     rw[FILTER_EQ_NIL,EVERY_MEM,MEM_MAP] >>
+                     pairarg_tac >> rw[] >>
+                     imp_res_tac ALOOKUP_NONE >>
+                     qpat_x_assum `MEM _ ctxt1` (strip_assume_tac o REWRITE_RULE [MEM_SPLIT]) >>
+                     rveq >> fs[] >>
+                     qpat_x_assum `MEM _ _` (strip_assume_tac o REWRITE_RULE [MEM_SPLIT]) >>
+                     rveq >> fs[] >>
+                     FULL_CASE_TAC >> fs[] >>
+                     qpat_x_assum `_ extends _` assume_tac >>
+                     drule_then (assume_tac o C MATCH_MP init_ctxt_extends) extends_trans >>
+                     FULL_SIMP_TAC bool_ss [GSYM APPEND_ASSOC] >>
+                     dxrule extends_APPEND_NIL >>
+                     simp[extends_NIL_CONS_extends,updates_cases,constspec_ok_def,is_reserved_name_def] >> simp[DISJ_IMP_THM,FORALL_AND_THM] >>
+                     rw[] >> simp[]) >>
+                  simp[defn_matches_def] >>
+                  TOP_CASE_TAC >> simp[] >>
+                  CONV_TAC SYM_CONV >>
+                  rw[FILTER_EQ_NIL,EVERY_MEM,MEM_MAP] >>
+                  pairarg_tac >> rw[] >>
+                  qpat_x_assum `_ :: _ extends _` assume_tac >>
+                  drule_then (assume_tac o C MATCH_MP init_ctxt_extends) extends_trans >>
+                  fs[extends_NIL_CONS_extends,updates_cases] >>
+                  qpat_x_assum `MEM _ (mk_bool_ctxt _)` (strip_assume_tac o REWRITE_RULE [MEM_SPLIT]) >>
+                  rveq >> fs[] >>
+                  Cases_on `b` >-
+                    (FULL_SIMP_TAC bool_ss [GSYM APPEND_ASSOC] >>
+                     dxrule extends_APPEND_NIL >>
+                     simp[extends_NIL_CONS_extends,updates_cases,constspec_ok_def,is_reserved_name_def] >> simp[DISJ_IMP_THM,FORALL_AND_THM] >>
+                     rw[] >> res_tac >>
+                     simp[]) >>
+                  fs[] >>
+                  qpat_x_assum `MEM _ _` (strip_assume_tac o REWRITE_RULE [MEM_SPLIT]) >>
+                  rveq >> fs[]) >>
+               reverse TOP_CASE_TAC >-
+                 (goal_assum kall_tac >>
+                  drule_then (assume_tac o C MATCH_MP init_ctxt_extends) extends_trans >>
+                  drule NewConst_no_abs_rep >>
+                  disch_then(mp_tac o CONV_RULE(RESORT_FORALL_CONV rev)) >>
+                  disch_then(qspecl_then[`strlit "@"`,`^select_ty`] mp_tac) >>
+                  impl_tac >- rw[Abbr `ctxt`] >>
+                  strip_tac >> fs[]) >>
+               simp[Abbr `ctxt`,ALOOKUP_APPEND] >>
+               simp[Once holBoolSyntaxTheory.mk_bool_ctxt_def,holBoolSyntaxTheory.ImpliesDef_def] >>
+               simp[typeof_def,equation_def]) >>
+          simp[ext_type_frag_builtins_Fun,ext_type_frag_builtins_Bool] >>
+          simp[GSYM CONJ_ASSOC] >>
+          conj_asm1_tac >-
+            (dep_rewrite.DEP_ONCE_REWRITE_TAC[apply_abstract] >> simp[]) >>
+          conj_asm1_tac >-
+            (dep_rewrite.DEP_REWRITE_TAC[apply_abstract] >>
+             simp[] >>
+             rename1 `elem ⋲ ind` >>
+             dep_rewrite.DEP_REWRITE_TAC[abstract_in_funspace] >> simp[] >>
+             rw[some_def] >>
+             SELECT_ELIM_TAC >> simp[] >> metis_tac[]) >>
+          rw[boolean_eq_true] >>
+          dep_rewrite.DEP_REWRITE_TAC[apply_abstract] >>
+          simp[] >>
+          rename1 `elem ⋲ ind` >>
+          dep_rewrite.DEP_REWRITE_TAC[abstract_in_funspace] >> simp[] >>
+          rw[some_def] >>
+          SELECT_ELIM_TAC >> simp[] >> metis_tac[apply_abstract])
+      >- ((* Axiom of infinity *)
+          `NewAxiom p = (^infinity_ax)` by
+            (qpat_x_assum `NewAxiom _ :: _ = _` (mp_tac o REWRITE_RULE[mk_infinity_ctxt_def]) >>
+             simp[]) >>
+          fs[] >> rveq >>
+          rw[satisfies_t_def,satisfies_def] >>
+          `ALOOKUP (type_list ctxt1) (strlit "ind") = NONE`
+            by(drule_then (assume_tac o C MATCH_MP init_ctxt_extends) extends_trans >>
+               drule extends_NIL_DISJOINT >>
+               simp[ALOOKUP_NONE,mk_infinity_ctxt_def]) >>
+          `ALOOKUP (const_list ctxt1) (strlit "ONE_ONE") = NONE`
+            by(drule_then (assume_tac o C MATCH_MP init_ctxt_extends) extends_trans >>
+               drule extends_NIL_DISJOINT >>
+               simp[ALOOKUP_NONE,mk_infinity_ctxt_def]) >>
+          `ALOOKUP (const_list ctxt1) (strlit "ONTO") = NONE`
+            by(drule_then (assume_tac o C MATCH_MP init_ctxt_extends) extends_trans >>
+               drule extends_NIL_DISJOINT >>
+               simp[ALOOKUP_NONE,mk_infinity_ctxt_def]) >>
+          `ALOOKUP (const_list ctxt1) (strlit "!") = NONE`
+            by(drule_then (assume_tac o C MATCH_MP init_ctxt_extends) extends_trans >>
+               drule extends_NIL_DISJOINT >>
+               simp[ALOOKUP_NONE,mk_infinity_ctxt_def,holBoolSyntaxTheory.mk_bool_ctxt_def,
+                    mk_select_ctxt_def]) >>
+          `ALOOKUP (const_list ctxt1) (strlit "?") = NONE`
+            by(drule_then (assume_tac o C MATCH_MP init_ctxt_extends) extends_trans >>
+               drule extends_NIL_DISJOINT >>
+               simp[ALOOKUP_NONE,mk_infinity_ctxt_def,holBoolSyntaxTheory.mk_bool_ctxt_def,
+                    mk_select_ctxt_def]) >>
+          `ALOOKUP (const_list ctxt1) (strlit "==>") = NONE`
+            by(drule_then (assume_tac o C MATCH_MP init_ctxt_extends) extends_trans >>
+               drule extends_NIL_DISJOINT >>
+               simp[ALOOKUP_NONE,mk_infinity_ctxt_def,holBoolSyntaxTheory.mk_bool_ctxt_def,
+                    mk_select_ctxt_def]) >>
+          rename1 `mk_bool_ctxt ctxt3` >>
+          qmatch_goalsub_abbrev_tac `ext_term_frag_builtins (ext_type_frag_builtins δ) γ` >>
+          qmatch_asmsub_abbrev_tac `ctxt extends init_ctxt` >>
+          `is_std_sig(sigof ctxt)`
+            by(rpt(qpat_x_assum `is_std_sig _` mp_tac) >>
+               fs[Abbr `ctxt`,mk_infinity_ctxt_def,mk_select_ctxt_def]) >>
+          `is_bool_interpretation_ext (sigof ctxt) δ γ`
+            by(drule_then match_mp_tac extends_is_bool_interpretation >>
+               qexists_tac `ctxt3` >>
+               qexists_tac `axsof (mk_bool_ctxt ctxt3)` >>
+               conj_tac >-
+                 (qpat_x_assum `ctxt2 extends _` mp_tac >>
+                  fs[mk_infinity_ctxt_def,mk_select_ctxt_def] >>
+                  strip_tac >>
+                  drule extends_appends >>
+                  strip_tac >>
+                  Cases_on `c` >- fs[init_ctxt_def] >>
+                  fs[] >>
+                  rename1 `c ++ init_ctxt` >>
+                  Cases_on `c` >- fs[init_ctxt_def] >>
+                  fs[] >>
+                  rename1 `c ++ init_ctxt` >>
+                  Cases_on `c` >- fs[init_ctxt_def] >>
+                  fs[] >>
+                  rename1 `c ++ init_ctxt` >>
+                  Cases_on `c` >- fs[init_ctxt_def] >>
+                  fs[] >>
+                  rename1 `c ++ init_ctxt` >>
+                  Cases_on `c` >- fs[init_ctxt_def] >>
+                  fs[] >>
+                  rveq >>
+                  drule(extends_append_MID |> Q.INST [`a`|->`[x;y;z;å]`] |> REWRITE_RULE [APPEND]) >>
+                  impl_tac >- rw[init_ctxt_def] >>
+                  strip_tac >>
+                  drule_then (assume_tac o C MATCH_MP init_theory_ok) extends_theory_ok >>
+                  fs[]) >>
+               `ctxt extends mk_bool_ctxt ctxt3`
+                 by(qunabbrev_tac `ctxt` >>
+                    rw[mk_infinity_ctxt_def,mk_select_ctxt_def] >>
+                    `mk_bool_ctxt ctxt3 = [] ++ mk_bool_ctxt ctxt3` by simp[] >>
+                    pop_assum(fn thm => PURE_ONCE_REWRITE_TAC[Once thm]) >>
+                    PURE_REWRITE_TAC[GSYM(CONJUNCT2 APPEND)] >>
+                    PURE_REWRITE_TAC[APPEND_ASSOC] >>
+                    match_mp_tac extends_NIL_APPEND_extends >>
+                    drule_then(assume_tac o C MATCH_MP init_ctxt_extends) extends_trans >>
+                    PURE_REWRITE_TAC[GSYM APPEND_ASSOC,APPEND] >> simp[] >>
+                    pop_assum MP_TAC >> EVAL_TAC) >>
+               drule extends_sub >>
+               rw[] >>
+               simp[models_def] >>
+               fs[Abbr `ctxt`] >>
+               fs[mk_infinity_ctxt_def,mk_select_ctxt_def]
+              ) >>
+          fs[is_bool_interpretation_ext_def,is_bool_interpretation_def,
+             is_implies_interpretation_def,is_exists_interpretation_def,
+             is_and_interpretation_def,is_not_interpretation_def
+            ] >>
+          simp[termsem_def] >>
+          qpat_assum `!ty. ty ∈ ground_types (sigof ctxt) ==> _ = _`
+            (fn thm => dep_rewrite.DEP_ONCE_REWRITE_TAC[thm]) >>
+          conj_tac >-
+            (rw[ground_types_def,tyvars_def] >>
+             fs[type_ok_def,is_std_sig_def] >>
+             rw[Abbr `ctxt`] >>
+             simp[ALOOKUP_APPEND] >>
+             EVAL_TAC) >>
+          simp[ext_type_frag_builtins_Fun,ext_type_frag_builtins_Bool,UPDATE_def] >>
+          `ext_type_frag_builtins δ Ind = ind`
+            by(simp[ext_type_frag_builtins_def,Abbr `δ`] >>
+               dep_rewrite.DEP_ONCE_REWRITE_TAC[CONJUNCT1 type_interpretation_of_alt] >>
+               simp[] >>
+               conj_asm1_tac >-
+                 (simp[ground_types_def,nonbuiltin_types_def,tyvars_def,is_builtin_type_def] >>
+                  reverse conj_tac >-
+                    (rw[Abbr `ctxt`,type_ok_def,ALOOKUP_APPEND] >> EVAL_TAC) >>
+                  fs[Abbr `ctxt`,mk_infinity_ctxt_def]) >>
+               drule_then (assume_tac o C MATCH_MP init_ctxt_extends) extends_trans >>
+               drule NewType_no_type_match >>
+               disch_then(qspecl_then [`[]`,`strlit "ind"`,`0`] mp_tac) >>
+               impl_tac >- (rw[Abbr `ctxt`] >> EVAL_TAC) >>
+               disch_then SUBST_ALL_TAC >>
+               simp[]) >>
+          simp[] >>
+          simp[ext_term_frag_builtins_def] >>
+          (* Fish out ONTO's defining equation from the conexts ---
+             this way we don't need to unfold the model construction *)
+          first_assum(qspec_then `HD(^onto_conext)` mp_tac) >>
+          impl_tac >-
+            (qpat_x_assum `_ :: _ = _` mp_tac >>
+             EVAL_TAC >> strip_tac >> rveq >> EVAL_TAC) >>
+          simp[] >>
+          simp[satisfies_t_def] >>
+          disch_then(qspec_then `(K Ind)` mp_tac) >>
+          impl_keep_tac >-
+            (simp[tyvars_def] >>
+             conj_asm1_tac >-
+               (qpat_x_assum `_ :: _ = _` (mp_tac o EVAL_RULE) >>
+                strip_tac >> rveq >>
+                simp[type_ok_def,FLOOKUP_UPDATE,FLOOKUP_FUNION]) >>
+             simp[ground_terms_uninst_def] >>
+             qmatch_goalsub_abbrev_tac `a1 has_type _` >>
+             qexists_tac `typeof a1` >>
+             qunabbrev_tac `a1` >>
+             simp[typeof_def] >>
+             conj_tac >-
+               (rpt(rw[Once has_type_cases,PULL_EXISTS])) >>
+             rw[ground_types_def,tyvars_def] >>
+             metis_tac[term_ok_clauses,FST]) >>
+          simp[satisfies_def] >>
+          drule_then drule exists_valuation >>
+          disch_then(qspec_then `K Ind` mp_tac) >>
+          simp[] >>
+          fs[] >>
+          strip_tac >> simp[valuates_frag_builtins] >>
+          disch_then drule >>
+          impl_tac >-
+            (match_mp_tac terms_of_frag_uninst_term_ok >>
+             rw[term_ok_clauses] >>
+             simp[term_ok_def] >>
+             fs[mk_infinity_ctxt_def,mk_select_ctxt_def,holBoolSyntaxTheory.mk_bool_ctxt_def,
+                FLOOKUP_FUNION,FLOOKUP_UPDATE]
+             >- metis_tac[term_ok_clauses,FST]
+             >- (simp[holBoolSyntaxTheory.ForallDef_def] >>
+                 conj_tac >- metis_tac[term_ok_clauses,FST] >>
+                 rw[equation_def] >>
+                 Q.REFINE_EXISTS_TAC `[(Tyvar _,Tyvar _)]` >>
+                 rw[REV_ASSOCD_def] >>
+                 rpt(pop_assum kall_tac) >> metis_tac[])
+             >- (simp[holBoolSyntaxTheory.ExistsDef_def] >>
+                 conj_tac >- metis_tac[term_ok_clauses,FST] >>
+                 rw[equation_def] >>
+                 Q.REFINE_EXISTS_TAC `[(Tyvar _,Tyvar _)]` >>
+                 rw[REV_ASSOCD_def] >>
+                 rpt(pop_assum kall_tac) >> metis_tac[])) >>
+          simp[termsem_def,UPDATE_def] >>
+          simp[Once ext_term_frag_builtins_def] >>
+          simp[ext_type_frag_builtins_def] >>
+          fs[is_forall_interpretation_def] >>
+          dep_rewrite.DEP_ONCE_REWRITE_TAC[apply_abstract] >>
+          simp[] >>
+          conj_asm1_tac >-
+            (simp[ext_term_frag_builtins_def] >>
+             conj_asm1_tac >-
+               (qpat_x_assum `is_frag_interpretation _ _ _` mp_tac >>
+                rw[is_frag_interpretation_def,total_fragment_def,GSYM PFORALL_THM] >>
+                pop_assum(qspecl_then [`strlit"ONTO"`,`Fun (Fun Ind Ind) Bool`] mp_tac) >>
+                simp[ext_type_frag_builtins_Fun,ext_type_frag_builtins_Bool] >>
+                disch_then match_mp_tac >>
+                rw[ground_consts_def,nonbuiltin_constinsts_def,ground_types_def,tyvars_def,
+                   builtin_consts_def,term_ok_def,FLOOKUP_FUNION] >-
+                  metis_tac[term_ok_clauses,FST] >>
+                fs[mk_infinity_ctxt_def] >>
+                rveq >> fs[] >>
+                conj_tac >- metis_tac[term_ok_clauses,FST] >>
+                qexists_tac `[(Ind,Tyvar «A»);(Ind,Tyvar «B»)]` >>
+                EVAL_TAC) >>
+             dep_rewrite.DEP_REWRITE_TAC[abstract_in_funspace] >>
+             simp[] >> rw[boolean_in_boolset]) >>
+          dep_rewrite.DEP_ONCE_REWRITE_TAC[apply_abstract] >>
+          simp[] >>
+          conj_asm1_tac >-
+            (conj_asm1_tac >-
+               (dep_rewrite.DEP_ONCE_REWRITE_TAC[abstract_in_funspace] >>
+                simp[] >>
+                qpat_assum `∀ty. _ => ext_term_frag_builtins _ _ («!»,_) = _`
+                  (fn thm => dep_rewrite.DEP_ONCE_REWRITE_TAC[thm]) >>
+                simp[ground_types_def] >>
+                conj_asm1_tac >- (simp[Abbr `ctxt`] >> fs[mk_infinity_ctxt_def] >> rveq >> fs[]) >>
+                rw[] >>
+                qpat_assum `∀ty. _ => ext_term_frag_builtins _ _ («?»,_) = _`
+                  (fn thm => dep_rewrite.DEP_ONCE_REWRITE_TAC[thm]) >>
+                simp[ground_types_def] >>
+                rw[] >>
+                simp[ext_term_frag_builtins_def] >>
+                dep_rewrite.DEP_REWRITE_TAC[apply_abstract] >>
+                simp[boolean_in_boolset] >>
+                dep_rewrite.DEP_REWRITE_TAC[abstract_in_funspace] >>
+                rw[] >>
+                dep_rewrite.DEP_REWRITE_TAC[apply_abstract] >>
+                simp[boolean_in_boolset] >>
+                dep_rewrite.DEP_REWRITE_TAC[abstract_in_funspace] >>
+                rw[] >>
+                simp[boolean_in_boolset] >>
+                dep_rewrite.DEP_REWRITE_TAC[apply_abstract] >>
+                simp[boolean_in_boolset] >>
+                qpat_x_assum `m <: Funspace _ _` assume_tac >>
+                drule_then drule in_funspace_abstract >>
+                rw[] >>
+                dep_rewrite.DEP_REWRITE_TAC[apply_abstract] >>
+                rw[]) >>
+             simp[boolean_in_boolset]) >>
+          simp[boolean_eq_true,Once ext_term_frag_builtins_def] >>
+          disch_then kall_tac >>
+          (* Fish out ONE_ONE's defining equation from the conexts ---
+             this way we don't need to unfold the model construction *)
+          first_assum(qspec_then `HD(^one_one_conext)` mp_tac) >>
+          impl_tac >-
+            (qpat_x_assum `_ :: _ = _` mp_tac >>
+             EVAL_TAC >> strip_tac >> rveq >> EVAL_TAC) >>
+          simp[] >>
+          simp[satisfies_t_def] >>
+          disch_then(qspec_then `(K Ind)` mp_tac) >>
+          simp[] >>
+          impl_keep_tac >-
+            (simp[ground_terms_uninst_def] >>
+             qmatch_goalsub_abbrev_tac `a1 has_type _` >>
+             qexists_tac `typeof a1` >>
+             qunabbrev_tac `a1` >>
+             simp[typeof_def] >>
+             conj_tac >-
+               (rpt(rw[Once has_type_cases,PULL_EXISTS])) >>
+             rw[ground_types_def,tyvars_def] >>
+             metis_tac[term_ok_clauses,FST]) >>
+          simp[satisfies_def] >>
+          simp[valuates_frag_builtins] >>
+          disch_then drule >>
+          impl_tac >-
+            (match_mp_tac terms_of_frag_uninst_term_ok >>
+             rw[term_ok_clauses] >>
+             simp[term_ok_def] >>
+             fs[mk_infinity_ctxt_def,mk_select_ctxt_def,holBoolSyntaxTheory.mk_bool_ctxt_def,
+                FLOOKUP_FUNION,FLOOKUP_UPDATE]
+             >- metis_tac[term_ok_clauses,FST]
+             >- (simp[holBoolSyntaxTheory.ForallDef_def] >>
+                 conj_tac >- metis_tac[term_ok_clauses,FST] >>
+                 rw[equation_def] >>
+                 Q.REFINE_EXISTS_TAC `[(Tyvar _,Tyvar _)]` >>
+                 rw[REV_ASSOCD_def] >>
+                 rpt(pop_assum kall_tac) >> metis_tac[])
+             >- (simp[holBoolSyntaxTheory.ForallDef_def] >>
+                 conj_tac >- metis_tac[term_ok_clauses,FST] >>
+                 rw[equation_def] >>
+                 Q.REFINE_EXISTS_TAC `[(Tyvar _,Tyvar _)]` >>
+                 rw[REV_ASSOCD_def] >>
+                 rpt(pop_assum kall_tac) >> metis_tac[])
+             >- (simp[holBoolSyntaxTheory.ImpliesDef_def] >>
+                 rw[equation_def] >>
+                 metis_tac[term_ok_clauses,FST])
+            ) >>
+          simp[termsem_def,UPDATE_def] >>
+          simp[Once ext_term_frag_builtins_def] >>
+          simp[ext_type_frag_builtins_def] >>
+          dep_rewrite.DEP_ONCE_REWRITE_TAC[apply_abstract] >>
+          simp[] >>
+          conj_asm1_tac >-
+            (simp[ext_term_frag_builtins_def] >>
+             conj_asm1_tac >-
+               (qpat_x_assum `is_frag_interpretation _ _ _` mp_tac >>
+                disch_then(strip_assume_tac o Ho_Rewrite.REWRITE_RULE[is_frag_interpretation_def,total_fragment_def,GSYM PFORALL_THM]) >>
+                pop_assum(qspecl_then [`strlit"ONE_ONE"`,`Fun (Fun Ind Ind) Bool`] mp_tac) >>
+                simp[ext_type_frag_builtins_Fun,ext_type_frag_builtins_Bool] >>
+                disch_then match_mp_tac >>
+                rw[ground_consts_def,nonbuiltin_constinsts_def,ground_types_def,tyvars_def,
+                   builtin_consts_def,term_ok_def,FLOOKUP_FUNION] >-
+                  metis_tac[term_ok_clauses,FST] >>
+                fs[mk_infinity_ctxt_def] >>
+                rveq >> fs[] >>
+                conj_tac >- metis_tac[term_ok_clauses,FST] >>
+                qexists_tac `[(Ind,Tyvar «A»);(Ind,Tyvar «B»)]` >>
+                EVAL_TAC) >>
+             dep_rewrite.DEP_REWRITE_TAC[abstract_in_funspace] >>
+             simp[] >> rw[boolean_in_boolset]) >>
+          dep_rewrite.DEP_ONCE_REWRITE_TAC[apply_abstract] >>
+          simp[] >>
+          conj_asm1_tac >-
+            (conj_asm1_tac >-
+               (dep_rewrite.DEP_ONCE_REWRITE_TAC[abstract_in_funspace] >>
+                simp[] >>
+                qpat_assum `∀ty. _ => ext_term_frag_builtins _ _ («!»,_) = _`
+                  (fn thm => dep_rewrite.DEP_ONCE_REWRITE_TAC[thm]) >>
+                simp[ground_types_def] >>
+                conj_asm1_tac >- (simp[Abbr `ctxt`] >> fs[mk_infinity_ctxt_def] >> rveq >> fs[]) >>
+                rw[] >>
+                qpat_assum `∀ty. _ => ext_term_frag_builtins _ _ («?»,_) = _`
+                  (fn thm => dep_rewrite.DEP_ONCE_REWRITE_TAC[thm]) >>
+                simp[ground_types_def] >>
+                rw[] >>
+                simp[ext_term_frag_builtins_def] >>
+                dep_rewrite.DEP_REWRITE_TAC[apply_abstract] >>
+                simp[boolean_in_boolset] >>
+                dep_rewrite.DEP_REWRITE_TAC[abstract_in_funspace] >>
+                rw[] >>
+                dep_rewrite.DEP_REWRITE_TAC[apply_abstract] >>
+                simp[boolean_in_boolset] >>
+                dep_rewrite.DEP_REWRITE_TAC[abstract_in_funspace] >>
+                rw[] >>
+                simp[boolean_in_boolset] >>
+                dep_rewrite.DEP_REWRITE_TAC[apply_abstract] >>
+                simp[boolean_in_boolset] >>
+                qpat_x_assum `m <: Funspace _ _` assume_tac >>
+                drule_then drule in_funspace_abstract >>
+                rw[] >>
+                dep_rewrite.DEP_REWRITE_TAC[apply_abstract] >>
+                rw[] >>
+                dep_rewrite.DEP_REWRITE_TAC[abstract_in_funspace] >> rw[boolean_in_boolset] >>
+                dep_rewrite.DEP_REWRITE_TAC[apply_boolrel_rw] >>
+                simp[boolean_in_boolset]) >>
+             simp[boolean_in_boolset]) >>
+          simp[boolean_eq_true,Once ext_term_frag_builtins_def] >>
+          disch_then kall_tac >>
+          qpat_assum `∀ty. _ => ext_term_frag_builtins _ _ («!»,_) = _`
+            (fn thm => dep_rewrite.DEP_ONCE_REWRITE_TAC[thm]) >>
+          simp[ground_types_def] >>
+          conj_asm1_tac >- (simp[Abbr `ctxt`] >> fs[mk_infinity_ctxt_def] >> rveq >> fs[]) >>
+          rw[] >>
+          qpat_assum `∀ty. _ => ext_term_frag_builtins _ _ («?»,_) = _`
+            (fn thm => dep_rewrite.DEP_ONCE_REWRITE_TAC[thm]) >>
+          simp[ground_types_def] >>
+          simp[ext_term_frag_builtins_def] >>
+          dep_rewrite.DEP_REWRITE_TAC[apply_abstract] >>
+          simp[boolean_in_boolset,boolean_eq_true] >>
+          conj_asm1_tac >-
+            (dep_rewrite.DEP_REWRITE_TAC[abstract_in_funspace] >>
+             rw[] >>
+             dep_rewrite.DEP_REWRITE_TAC[apply_boolrel_rw] >>
+             simp[boolean_in_boolset] >>
+             dep_rewrite.DEP_REWRITE_TAC[apply_abstract] >>
+             simp[boolean_in_boolset] >>
+             dep_rewrite.DEP_REWRITE_TAC[apply_abstract] >>
+             simp[boolean_in_boolset] >>
+             dep_rewrite.DEP_REWRITE_TAC[apply_abstract] >>
+             simp[boolean_in_boolset] >>
+             dep_rewrite.DEP_REWRITE_TAC[abstract_in_funspace] >>
+             simp[boolean_in_boolset] >>
+             conj_tac >-
+               (rw[] >>
+                dep_rewrite.DEP_REWRITE_TAC[apply_abstract] >>
+                simp[boolean_in_boolset] >>
+                qpat_x_assum `m <: Funspace _ _` assume_tac >>
+                drule_then drule in_funspace_abstract >>
+                strip_tac >> simp[] >>
+                dep_rewrite.DEP_REWRITE_TAC[apply_abstract] >>
+                simp[] >>
+                dep_rewrite.DEP_REWRITE_TAC[abstract_in_funspace] >>
+                simp[boolean_in_boolset] >>
+                rw[] >>
+                dep_rewrite.DEP_REWRITE_TAC[apply_boolrel_rw] >>
+                simp[boolean_in_boolset] >>
+                dep_rewrite.DEP_REWRITE_TAC[apply_abstract] >>
+                simp[boolean_in_boolset] >>
+                dep_rewrite.DEP_REWRITE_TAC[abstract_in_funspace] >>
+                simp[boolean_in_boolset]) >>
+             dep_rewrite.DEP_REWRITE_TAC[apply_abstract] >>
+             simp[boolean_in_boolset] >>
+             dep_rewrite.DEP_REWRITE_TAC[abstract_in_funspace] >>
+             simp[boolean_in_boolset] >>
+             rw[] >>
+             dep_rewrite.DEP_REWRITE_TAC[apply_abstract] >>
+             simp[boolean_in_boolset] >>
+             dep_rewrite.DEP_REWRITE_TAC[abstract_in_funspace] >>
+             simp[boolean_in_boolset] >>
+             rw[] >>
+             dep_rewrite.DEP_REWRITE_TAC[apply_abstract] >>
+             simp[boolean_in_boolset] >>
+             qpat_x_assum `m <: Funspace _ _` assume_tac >>
+             drule_then drule in_funspace_abstract >>
+             strip_tac >> simp[] >>
+             dep_rewrite.DEP_REWRITE_TAC[apply_abstract] >>
+             simp[]) >>
+          qpat_x_assum `is_infinite _ _` mp_tac >>
+          simp[is_infinite_def] >>
+          simp[INFINITE_INJ_NOT_SURJ] >>
+          strip_tac >>
+          rename1 `INJ f` >>
+          qexists_tac`Abstract (ext_type_frag_builtins δ Ind) (ext_type_frag_builtins δ Ind) f` >>
+          fs[] >>
+          conj_asm1_tac >-
+            (dep_rewrite.DEP_REWRITE_TAC[abstract_in_funspace] >> simp[] >>
+             ntac 2 (pop_assum mp_tac) >> simp[INJ_DEF]) >>
+          simp[holds_def] >>
+          dep_rewrite.DEP_REWRITE_TAC[apply_abstract] >>
+          simp[boolean_in_boolset,boolean_eq_true] >>
+          conj_asm1_tac >-
+            (dep_rewrite.DEP_REWRITE_TAC[abstract_in_funspace] >>
+             simp[boolean_in_boolset] >>
+             rw[] >>
+             dep_rewrite.DEP_REWRITE_TAC[apply_abstract] >>
+             simp[boolean_in_boolset] >>
+             conj_asm1_tac >- (qhdtm_x_assum `INJ` mp_tac >> simp[INJ_DEF]) >>
+             simp[] >>
+             dep_rewrite.DEP_REWRITE_TAC[abstract_in_funspace] >>
+             simp[boolean_in_boolset] >>
+             rw[] >>
+             dep_rewrite.DEP_REWRITE_TAC[apply_boolrel_rw] >>
+             simp[boolean_in_boolset] >>
+             dep_rewrite.DEP_REWRITE_TAC[apply_abstract] >>
+             simp[boolean_in_boolset] >>
+             dep_rewrite.DEP_REWRITE_TAC[abstract_in_funspace] >>
+             simp[boolean_in_boolset] >>
+             qhdtm_x_assum `INJ` mp_tac >> simp[INJ_DEF]) >>
+          simp[] >>
+          conj_asm1_tac >-
+            (dep_rewrite.DEP_REWRITE_TAC[apply_boolrel_rw] >>
+             simp[boolean_in_boolset] >>
+             dep_rewrite.DEP_REWRITE_TAC[apply_abstract] >>
+             simp[boolean_in_boolset] >>
+             dep_rewrite.DEP_REWRITE_TAC[abstract_in_funspace] >>
+             simp[boolean_in_boolset] >>
+             rw[] >>
+             dep_rewrite.DEP_REWRITE_TAC[apply_abstract] >>
+             simp[boolean_in_boolset] >>
+             dep_rewrite.DEP_REWRITE_TAC[abstract_in_funspace] >>
+             simp[boolean_in_boolset] >>
+             rw[] >>
+             dep_rewrite.DEP_REWRITE_TAC[apply_abstract] >>
+             simp[boolean_in_boolset] >>
+             qhdtm_x_assum `INJ` mp_tac >> simp[INJ_DEF]) >>
+          dep_rewrite.DEP_REWRITE_TAC[apply_boolrel_rw] >>
+          simp[boolean_in_boolset,boolean_eq_true] >>
+          conj_asm1_tac >-
+            (dep_rewrite.DEP_REWRITE_TAC[apply_abstract] >>
+             simp[boolean_in_boolset] >>
+             dep_rewrite.DEP_REWRITE_TAC[abstract_in_funspace] >>
+             simp[boolean_in_boolset] >>
+             rw[] >>
+             dep_rewrite.DEP_REWRITE_TAC[apply_abstract] >>
+             simp[boolean_in_boolset] >>
+             dep_rewrite.DEP_REWRITE_TAC[abstract_in_funspace] >>
+             simp[boolean_in_boolset] >>
+             rw[] >>
+             dep_rewrite.DEP_REWRITE_TAC[apply_abstract] >>
+             simp[boolean_in_boolset] >>
+             qhdtm_x_assum `INJ` mp_tac >> simp[INJ_DEF]) >>
+          conj_tac >-
+            (rw[] >>
+             dep_rewrite.DEP_REWRITE_TAC[apply_abstract] >>
+             simp[boolean_in_boolset] >>
+             conj_asm1_tac >- (qhdtm_x_assum `INJ` mp_tac >> simp[INJ_DEF]) >>
+             simp[] >>
+             dep_rewrite.DEP_REWRITE_TAC[abstract_in_funspace] >>
+             simp[boolean_in_boolset] >>
+             conj_tac >-
+               (rw[] >>
+                dep_rewrite.DEP_REWRITE_TAC[apply_boolrel_rw] >>
+                simp[boolean_in_boolset] >>
+                dep_rewrite.DEP_REWRITE_TAC[apply_abstract] >>
+                simp[boolean_in_boolset] >>
+                conj_asm1_tac >- (qhdtm_x_assum `INJ` mp_tac >> simp[INJ_DEF]) >>
+                simp[] >>
+                dep_rewrite.DEP_REWRITE_TAC[abstract_in_funspace] >>
+                simp[boolean_in_boolset]) >>
+             rw[boolean_eq_true] >>
+             dep_rewrite.DEP_REWRITE_TAC[apply_abstract] >>
+             simp[boolean_in_boolset] >>
+             conj_asm1_tac >- (qhdtm_x_assum `INJ` mp_tac >> simp[INJ_DEF]) >>
+             simp[] >>
+             dep_rewrite.DEP_REWRITE_TAC[abstract_in_funspace] >>
+             simp[boolean_in_boolset] >>
+             dep_rewrite.DEP_REWRITE_TAC[apply_boolrel_rw] >>
+             simp[boolean_in_boolset] >>
+             simp[boolean_eq_true] >>
+             qhdtm_x_assum `INJ` mp_tac >> simp[INJ_DEF]) >>
+          dep_rewrite.DEP_REWRITE_TAC[apply_abstract] >>
+          simp[boolean_in_boolset,boolean_eq_true] >>
+          conj_asm1_tac >-
+            (dep_rewrite.DEP_REWRITE_TAC[abstract_in_funspace] >>
+             simp[boolean_in_boolset,boolean_eq_true] >>
+             rw[] >>
+             dep_rewrite.DEP_REWRITE_TAC[apply_abstract] >>
+             simp[boolean_in_boolset] >>
+             dep_rewrite.DEP_REWRITE_TAC[abstract_in_funspace] >>
+             simp[boolean_in_boolset,boolean_eq_true] >>
+             rw[] >>
+             dep_rewrite.DEP_REWRITE_TAC[apply_abstract] >>
+             simp[boolean_in_boolset] >>
+             qhdtm_x_assum `INJ` mp_tac >> simp[INJ_DEF]) >>
+          simp[] >>
+          qpat_x_assum`¬(SURJ f X Y)`mp_tac >>
+          simp[SURJ_DEF] >>
+          strip_tac >-
+            (qpat_x_assum`INJ f X Y`mp_tac >>
+             simp[INJ_DEF] >>
+             PROVE_TAC[]) >>
+          rename1 `w <: ext_type_frag_builtins _ Ind` >>
+          qexists_tac `w` >>
+          simp[] >>
+          dep_rewrite.DEP_REWRITE_TAC[apply_abstract] >>
+          simp[boolean_in_boolset,boolean_eq_true] >>
+          fs[GSYM IMP_DISJ_THM] >>
+          dep_rewrite.DEP_REWRITE_TAC[abstract_in_funspace] >>
+          simp[boolean_in_boolset,boolean_eq_true] >>
+          conj_asm1_tac >-
+            (rw[] >>
+             dep_rewrite.DEP_REWRITE_TAC[apply_abstract] >>
+             simp[boolean_in_boolset] >>
+             qhdtm_x_assum `INJ` mp_tac >> simp[INJ_DEF]) >>
+          ntac 2 strip_tac >>
+          dep_rewrite.DEP_REWRITE_TAC[apply_abstract] >>
+          simp[boolean_in_boolset] >>
+          simp[boolean_def,true_neq_false] >>
+          qhdtm_x_assum `INJ` mp_tac >> simp[INJ_DEF])
+      )
+  >- ((* conexts of new axiom (vacuous) *)
+      first_x_assum match_mp_tac >>
+      pop_assum(strip_assume_tac o REWRITE_RULE[MEM_SPLIT]) >>
+      fs[conexts_of_upd_def])
+  >- ((* NewConst *)
+      fs[conexts_of_upd_def])
+  >- ((* NewConst *)
+      fs[conexts_of_upd_def])
+  >- ((* ConstSpec *)
+      fs[conexts_of_upd_def] >>
+      rw[satisfies_t_def,satisfies_def] >>
+      `!name. MEM name (MAP FST eqs) ==> ~MEM name (MAP FST (const_list ctxt1))`
+        by(rw[] >>
+           drule_then (assume_tac o C MATCH_MP init_ctxt_extends) extends_trans >>
+           drule extends_NIL_DISJOINT >>
+           fs[DISJOINT_DEF,INTER_DEF,FUN_EQ_THM,GSYM IMP_DISJ_THM,map_fst] >>
+           TRY(rename1 `ConstSpec F` >> metis_tac[]) >>
+           fs[constspec_ok_def] >>
+           qpat_x_assum `MEM _ (MAP FST _)` (strip_assume_tac o REWRITE_RULE[MEM_MAP]) >>
+           rveq >>
+           rename1 `MEM pp eqs` >>
+           Cases_on `pp` >>
+           rename1 `MEM (name,typ) eqs` >>
+           res_tac >>
+           qpat_x_assum `MEM (NewConst _ _) _` (strip_assume_tac o REWRITE_RULE[MEM_SPLIT]) >>
+           rw[IMP_CONJ_THM,FORALL_AND_THM]) >>
+      TRY(rename1 `ConstSpec T` >> (* overloads case *)
+          drule proves_theory_mono >>
+          qmatch_asmsub_abbrev_tac `total_fragment (tyenv,tmenv)` >>
+          disch_then(qspecl_then [`tysof ctxt2`,`tmsof ctxt2`,`axsof ctxt2`,
+                                   `tyenv`,`tmenv`] mp_tac) >>
+          simp[] >>
+          MAP_EVERY qunabbrev_tac [`tyenv`,`tmenv`] >>
+          impl_tac >-
+            (rw[] >>
+             TRY(match_mp_tac (CONJUNCT2 SUBMAP_FUNION_ID) >>
+                 drule_then (assume_tac o C MATCH_MP init_ctxt_extends) extends_trans >>
+                 drule extends_NIL_DISJOINT >>
+                 simp[] >> NO_TAC) >>
+             TRY(match_mp_tac (CONJUNCT2 SUBMAP_FUNION_ID) >> rw[FDOM_FUPDATE] >>
+                drule_then (assume_tac o C MATCH_MP init_ctxt_extends) extends_trans >>
+                drule extends_NIL_DISJOINT >>
+                simp[] >> NO_TAC) >>
+             qhdtm_x_assum `theory_ok` mp_tac >>
+             rw[theory_ok_def]) >>
+          strip_tac >>
+          drule_then assume_tac proves_term_ok >>
+          fs[] >>
+          drule_then assume_tac term_ok_welltyped >>
+          drule termsem_VSUBST >>
+          disch_then(qspec_then `^mem` mp_tac) >>
+          qmatch_goalsub_abbrev_tac `VSUBST ilist` >>
+          disch_then(qspec_then `ilist` mp_tac) >>
+          impl_tac >-
+            (rw[Abbr `ilist`,MEM_MAP,ELIM_UNCURRY] >> metis_tac[has_type_rules]) >>
+          simp[] >>
+          disch_then kall_tac >>
+          qmatch_asmsub_abbrev_tac `total_fragment (tyenv,tmenv)` >>
+          `models (type_interpretation_of ind (ctxt1 ++ ConstSpec T eqs prop::ctxt2)) (UNCURRY (term_interpretation_of ind (ctxt1 ++ ConstSpec T eqs prop::ctxt2))) ((tyenv,tmenv),axsof ctxt2)`
+            by(rw[models_def]) >>
+          drule_then drule proves_sound >>
+          simp[entails_def] >>
+          strip_tac >>
+          first_x_assum drule >>
+          simp[satisfies_t_def] >>
+          ntac 2 (disch_then drule) >>
+          impl_keep_tac >-
+            (rw[ground_terms_uninst_def,EVERY_MEM,MEM_MAP] >>
+             qexists_tac `Bool` >>
+             fs[EVERY_MEM,MEM_MAP,PULL_EXISTS] >>
+             res_tac >>
+             fs[ELIM_UNCURRY] >>
+             simp[ground_types_def,tyvars_def] >>
+             imp_res_tac theory_ok_sig >>
+             metis_tac[FST,term_ok_clauses]) >>
+          simp[satisfies_def] >>
+          fs[valuates_frag_builtins] >>
+          qmatch_goalsub_abbrev_tac `termsem _ _ vv sigma prop = True` >>
+          disch_then(qspec_then `vv` mp_tac) >>
+          impl_tac >-
+            (conj_asm1_tac >-
+               (rw[valuates_frag_def,Abbr `vv`] >>
+                simp[MAP_REVERSE,APPLY_UPDATE_LIST_ALOOKUP,ALOOKUP_MAP] >>
+                TOP_CASE_TAC >- metis_tac[valuates_frag_def] >>
+                fs[ALOOKUP_SOME_EQ] >>
+                fs[MAP_EQ_APPEND] >> rveq >>
+                pairarg_tac >> fs[] >> rveq >>
+                qpat_x_assum `Abbrev (_ ++ _ ++ _ = _)` (assume_tac o REWRITE_RULE[markerTheory.Abbrev_def]) >>
+                fs[MAP_EQ_APPEND |> CONV_RULE(LHS_CONV SYM_CONV)] >> rveq >> fs[] >>
+                pairarg_tac >> fs[] >> rveq >>
+                fs[] >>
+                SIMP_TAC std_ss [GSYM APPEND_ASSOC,APPEND] >>
+                rename1 `Const name` >>
+                drule_then(drule_then drule) termsem_in_type_ext2 >>
+                disch_then(qspecl_then [`v`,`sigma`,`Const name (typeof t)`] mp_tac) >>
+                impl_tac >-
+                  (conj_tac >-
+                     (match_mp_tac terms_of_frag_uninst_term_ok >>
+                      simp[term_ok_def] >>
+                      rw[Abbr `tmenv`,FLOOKUP_UPDATE,FLOOKUP_FUNION] >>
+                      fs[DISJ_IMP_THM,FORALL_AND_THM] >>
+                      fs[GSYM ALOOKUP_NONE] >>
+                      fs[constspec_ok_def,ALL_DISTINCT_APPEND,DISJ_IMP_THM,FORALL_AND_THM,ALOOKUP_MAP] >>
+                      reverse conj_tac >- metis_tac[] >>
+                      rfs[term_ok_clauses]) >>
+                   simp[VFREE_IN_def]) >>
+                simp[typeof_def] >>
+                SIMP_TAC std_ss [GSYM APPEND_ASSOC,APPEND]) >>
+             conj_asm1_tac >- (match_mp_tac terms_of_frag_uninst_term_ok >> simp[]) >>
+             conj_asm1_tac >-
+               (rw[EVERY_MEM,MEM_MAP] >> pairarg_tac >> rveq >> fs[] >>
+                fs[EVERY_MEM,MEM_MAP] >> res_tac >> fs[] >>
+                match_mp_tac terms_of_frag_uninst_term_ok >> simp[]) >>
+             rw[EVERY_MEM,MEM_MAP] >> pairarg_tac >> rveq >> fs[] >>
+             drule_then (drule_then(drule_then drule)) termsem_ext_equation >>
+             fs[EVERY_MEM,MEM_MAP,PULL_EXISTS] >>
+             first_x_assum(drule_then strip_assume_tac) >>
+             fs[] >>
+             drule_then drule terms_of_frag_uninst_equationE >>
+             impl_tac >-
+               (fs[EVERY_MEM,MEM_MAP,PULL_EXISTS] >> res_tac >>
+                fs[welltyped_equation]) >>
+             disch_then(MAP_EVERY assume_tac o rev o CONJUNCTS) >>
+             disch_then dxrule >>
+             disch_then dxrule >>
+             impl_tac >-
+               (fs[EVERY_MEM,MEM_MAP,PULL_EXISTS] >> res_tac >>
+                fs[term_ok_clauses]) >>
+             simp[termsem_ext_def] >>
+             disch_then kall_tac >>
+             simp[boolean_eq_true] >>
+             simp[termsem_def,Abbr `vv`] >>
+             simp[APPLY_UPDATE_LIST_ALOOKUP,Abbr `ilist`,MAP_REVERSE] >>
+             simp[GSYM MAP_MAP_o] >>
+             qmatch_goalsub_abbrev_tac `ALOOKUP (MAP _ ll)` >>
+             `EVERY (λs. ∃x ty. s = Var x ty) (MAP FST ll)`
+               by(fs[Abbr`ll`,EVERY_MEM,MEM_MAP,PULL_EXISTS] >> Cases >> rw[]) >>
+             simp[ALOOKUP_MAP_dest_var] >>
+             simp[Abbr `ll`,MAP_MAP_o,o_DEF,ELIM_UNCURRY] >>
+             drule_then(drule_then (fn thm => simp[thm])) orth_ctxt_ALOOKUP_eqs >>
+             simp[termsem_def] >>
+             `s <> strlit "="`
+               by(fs[constspec_ok_def,is_builtin_name_def,is_reserved_name_def] >> metis_tac[]) >>
+             simp[SimpL``$=``,ext_term_frag_builtins_def] >>
+             qmatch_goalsub_abbrev_tac `type_interpretation_of ind ctxt` >>
+             `is_frag_interpretation (total_fragment (sigof ctxt))
+                (type_interpretation_of ind ctxt)
+                (UNCURRY (term_interpretation_of ind ctxt))`
+               by(fs[Abbr `ctxt`]) >>
+             `(s,TYPE_SUBSTf sigma (typeof t)) ∈ ground_consts (sigof ctxt)`
+               by(rw[Abbr`ctxt`] >>
+                  simp[ground_consts_def] >>
+                  conj_tac >-
+                    (rw[ground_types_def,tyvars_TYPE_SUBSTf_eq_NIL] >>
+                     match_mp_tac type_ok_TYPE_SUBSTf >>
+                     simp[] >>
+                     fs[EVERY_MEM,MEM_MAP,PULL_EXISTS] >> res_tac >> fs[] >>
+                     rfs[term_ok_clauses]) >>
+                  fs[constspec_ok_def] >> res_tac >>
+                  rw[term_ok_def,Abbr`tmenv`,FLOOKUP_FUNION] >>
+                  reverse(Cases_on `ALOOKUP (const_list ctxt1) s`) >-
+                    (imp_res_tac ALOOKUP_MEM >>
+                     res_tac >> metis_tac[FST]) >>
+                  simp[] >>
+                  reverse conj_tac >-
+                    (metis_tac[TYPE_SUBSTf_TYPE_SUBST_compose,TYPE_SUBSTf_eq_TYPE_SUBST]) >>
+                  match_mp_tac type_ok_TYPE_SUBSTf >>
+                  simp[] >>
+                  fs[] >>
+                  rfs[term_ok_clauses]) >>
+             `(s,TYPE_SUBSTf sigma (typeof t)) ∈ nonbuiltin_constinsts`
+               by(rw[nonbuiltin_constinsts_def,builtin_consts_def]) >>
+             Q.SUBGOAL_THEN `inhabited ind` assume_tac >- metis_tac[] >>
+             simp[type_interpretation_of_alt] >>
+             drule orth_ctxt_FILTER_ctxt >>
+             disch_then(drule o ONCE_REWRITE_RULE[CONJ_SYM]) >>
+             disch_then(qspecl_then [`sigma`,`prop`,`T`] mp_tac) >>
+             impl_tac >- rw[Abbr`ctxt`] >>
+             strip_tac >> simp[] >> pop_assum kall_tac >>
+             TOP_CASE_TAC >-
+               (goal_assum kall_tac >>
+                Q.SUBGOAL_THEN `is_instance (typeof t) (TYPE_SUBSTf sigma (typeof t))` assume_tac >-
+                  metis_tac[TYPE_SUBSTf_eq_TYPE_SUBST] >>
+                metis_tac[instance_subst_completeness,IS_SOME_DEF]) >>
+             rename1 `instance_subst _ _ _ = SOME result` >>
+             Cases_on `result` >>
+             rename1 `instance_subst _ _ _ = SOME(sigma',e)` >>
+             drule_then (assume_tac o GSYM) instance_subst_soundness >>
+             simp[ELIM_UNCURRY] >>
+             qmatch_goalsub_abbrev_tac `termsem a1 a2 a3 a4 t = termsem _ _ a5 _ _` >>
+             `termsem a1 a2 a3 a4 t = termsem a1 a2 a5 a4 t`
+               by(MAP_EVERY qunabbrev_tac [`a1`,`a2`,`a3`,`a4`,`a5`] >>
+                  match_mp_tac termsem_frees >>
+                  res_tac >> fs[CLOSED_def] >>
+                  rfs[term_ok_equation] >> imp_res_tac term_ok_welltyped) >>
+             pop_assum SUBST_ALL_TAC >>
+             match_mp_tac termsem_subst >>
+             conj_tac >-
+               (MAP_EVERY qunabbrev_tac [`a1`,`a2`,`a3`,`a4`,`a5`] >>
+                res_tac >> fs[] >> rfs[term_ok_equation] >> imp_res_tac term_ok_welltyped) >>
+             MAP_EVERY qunabbrev_tac [`a1`,`a2`,`a3`,`a4`,`a5`] >>
+             fs[TYPE_SUBST_eq_TYPE_SUBSTf,TYPE_SUBSTf_eq_TYPE_SUBSTf] >>
+             metis_tac[SND]) >>
+          simp[]) >>
+      TRY(rename1 `ConstSpec F` >> (* fresh constants case *)
+          drule proves_theory_mono >>
+          qmatch_asmsub_abbrev_tac `total_fragment (tyenv,tmenv)` >>
+          disch_then(qspecl_then [`tysof ctxt2`,`tmsof ctxt2`,`axsof ctxt2`,
+                                   `tyenv`,`tmenv`] mp_tac) >>
+          simp[] >>
+          MAP_EVERY qunabbrev_tac [`tyenv`,`tmenv`] >>
+          impl_tac >-
+            (rw[] >>
+             TRY(match_mp_tac (CONJUNCT2 SUBMAP_FUNION_ID) >>
+                 drule_then (assume_tac o C MATCH_MP init_ctxt_extends) extends_trans >>
+                 drule extends_NIL_DISJOINT >>
+                 simp[] >> NO_TAC) >>
+             TRY(match_mp_tac (CONJUNCT2 SUBMAP_FUNION_ID) >> rw[FDOM_FUPDATE] >>
+                 drule_then (assume_tac o C MATCH_MP init_ctxt_extends) extends_trans >>
+                 drule extends_NIL_DISJOINT >>
+                 simp[] >- metis_tac[DISJOINT_SYM] >>
+                 disch_then kall_tac >>
+                 fs[constspec_ok_def,map_fst] >>
+                 fs[DISJOINT_DEF,FUN_EQ_THM] >> metis_tac[]) >>
+             qhdtm_x_assum `theory_ok` mp_tac >>
+             rw[theory_ok_def]) >>
+          strip_tac >>
+          drule_then assume_tac proves_term_ok >>
+          fs[] >>
+          drule_then assume_tac term_ok_welltyped >>
+          drule termsem_VSUBST >>
+          disch_then(qspec_then `^mem` mp_tac) >>
+          qmatch_goalsub_abbrev_tac `VSUBST ilist` >>
+          disch_then(qspec_then `ilist` mp_tac) >>
+          impl_tac >-
+            (rw[Abbr `ilist`,MEM_MAP,ELIM_UNCURRY] >> metis_tac[has_type_rules]) >>
+          simp[] >>
+          disch_then kall_tac >>
+          qmatch_asmsub_abbrev_tac `total_fragment (tyenv,tmenv)` >>
+          `models (type_interpretation_of ind (ctxt1 ++ ConstSpec F eqs prop::ctxt2)) (UNCURRY (term_interpretation_of ind (ctxt1 ++ ConstSpec F eqs prop::ctxt2))) ((tyenv,tmenv),axsof ctxt2)`
+            by(rw[models_def]) >>
+          drule_then drule proves_sound >>
+          simp[entails_def] >>
+          strip_tac >>
+          first_x_assum drule >>
+          simp[satisfies_t_def] >>
+          ntac 2 (disch_then drule) >>
+          impl_keep_tac >-
+            (rw[ground_terms_uninst_def,EVERY_MEM,MEM_MAP] >>
+             qexists_tac `Bool` >>
+             fs[EVERY_MEM,MEM_MAP,PULL_EXISTS] >>
+             res_tac >>
+             fs[ELIM_UNCURRY] >>
+             simp[ground_types_def,tyvars_def] >>
+             imp_res_tac theory_ok_sig >>
+             metis_tac[FST,term_ok_clauses]) >>
+          simp[satisfies_def] >>
+          fs[valuates_frag_builtins] >>
+          qmatch_goalsub_abbrev_tac `termsem _ _ vv sigma prop = True` >>
+          disch_then(qspec_then `vv` mp_tac) >>
+          impl_tac >-
+            (conj_asm1_tac >-
+               (rw[valuates_frag_def,Abbr `vv`] >>
+                simp[MAP_REVERSE,APPLY_UPDATE_LIST_ALOOKUP,ALOOKUP_MAP] >>
+                TOP_CASE_TAC >- metis_tac[valuates_frag_def] >>
+                fs[ALOOKUP_SOME_EQ] >>
+                fs[MAP_EQ_APPEND] >> rveq >>
+                pairarg_tac >> fs[] >> rveq >>
+                qpat_x_assum `Abbrev (_ ++ _ ++ _ = _)` (assume_tac o REWRITE_RULE[markerTheory.Abbrev_def]) >>
+                fs[MAP_EQ_APPEND |> CONV_RULE(LHS_CONV SYM_CONV)] >> rveq >> fs[] >>
+                pairarg_tac >> fs[] >> rveq >>
+                fs[] >>
+                SIMP_TAC std_ss [GSYM APPEND_ASSOC,APPEND] >>
+                rename1 `Const name` >>
+                drule_then(drule_then drule) termsem_in_type_ext2 >>
+                disch_then(qspecl_then [`v`,`sigma`,`Const name (typeof t)`] mp_tac) >>
+                impl_tac >-
+                  (conj_tac >-
+                     (match_mp_tac terms_of_frag_uninst_term_ok >>
+                      simp[term_ok_def] >>
+                      rw[Abbr `tmenv`,FLOOKUP_UPDATE,FLOOKUP_FUNION] >>
+                      fs[DISJ_IMP_THM,FORALL_AND_THM] >>
+                      fs[GSYM ALOOKUP_NONE] >>
+                      fs[constspec_ok_def,ALL_DISTINCT_APPEND,DISJ_IMP_THM,FORALL_AND_THM,ALOOKUP_MAP] >>
+                      fs[GSYM ALOOKUP_NONE] >>
+                      rfs[term_ok_clauses]) >>
+                   simp[VFREE_IN_def]) >>
+                simp[typeof_def] >>
+                SIMP_TAC std_ss [GSYM APPEND_ASSOC,APPEND]) >>
+             conj_asm1_tac >- (match_mp_tac terms_of_frag_uninst_term_ok >> simp[]) >>
+             conj_asm1_tac >-
+               (rw[EVERY_MEM,MEM_MAP] >> pairarg_tac >> rveq >> fs[] >>
+                fs[EVERY_MEM,MEM_MAP] >> res_tac >> fs[] >>
+                match_mp_tac terms_of_frag_uninst_term_ok >> simp[]) >>
+             rw[EVERY_MEM,MEM_MAP] >> pairarg_tac >> rveq >> fs[] >>
+             drule_then (drule_then(drule_then drule)) termsem_ext_equation >>
+             fs[EVERY_MEM,MEM_MAP,PULL_EXISTS] >>
+             first_x_assum(drule_then strip_assume_tac) >>
+             fs[] >>
+             drule_then drule terms_of_frag_uninst_equationE >>
+             impl_tac >-
+               (fs[EVERY_MEM,MEM_MAP,PULL_EXISTS] >> res_tac >>
+                fs[welltyped_equation]) >>
+             disch_then(MAP_EVERY assume_tac o rev o CONJUNCTS) >>
+             disch_then dxrule >>
+             disch_then dxrule >>
+             impl_tac >-
+               (fs[EVERY_MEM,MEM_MAP,PULL_EXISTS] >> res_tac >>
+                fs[term_ok_clauses]) >>
+             simp[termsem_ext_def] >>
+             disch_then kall_tac >>
+             simp[boolean_eq_true] >>
+             simp[termsem_def,Abbr `vv`] >>
+             simp[APPLY_UPDATE_LIST_ALOOKUP,Abbr `ilist`,MAP_REVERSE] >>
+             simp[GSYM MAP_MAP_o] >>
+             qmatch_goalsub_abbrev_tac `ALOOKUP (MAP _ ll)` >>
+             `EVERY (λs. ∃x ty. s = Var x ty) (MAP FST ll)`
+               by(fs[Abbr`ll`,EVERY_MEM,MEM_MAP,PULL_EXISTS] >> Cases >> rw[]) >>
+             simp[ALOOKUP_MAP_dest_var] >>
+             simp[Abbr `ll`,MAP_MAP_o,o_DEF,ELIM_UNCURRY] >>
+             qmatch_goalsub_abbrev_tac `ALOOKUP ll` >>
+             `ALL_DISTINCT(MAP FST ll)`
+               by(rw[Abbr `ll`,ALL_DISTINCT_MAP] >>
+                  fs[constspec_ok_def] >>
+                  qpat_x_assum `ALL_DISTINCT _` mp_tac >>
+                  rpt(pop_assum kall_tac) >>
+                  Induct_on `eqs` >- rw[] >>
+                  Cases >> rw[] >>
+                  rw[MEM_MAP,GSYM IMP_DISJ_THM] >>
+                  Cases_on `x` >> fs[] >>
+                  rveq >>
+                  fs[MEM_MAP,GSYM IMP_DISJ_THM]) >>
+             `MEM (Var s (typeof t),Const s (typeof t)) ll`
+               by(rw[Abbr `ll`,MEM_MAP,PULL_EXISTS] >> metis_tac[FST,SND]) >>
+             drule_then drule ALOOKUP_ALL_DISTINCT_MEM >>
+             simp[] >> disch_then kall_tac >>
+             simp[termsem_def] >>
+             `s <> strlit "="`
+               by(fs[constspec_ok_def] >>
+                  qpat_x_assum `ctxt2 extends init_ctxt` assume_tac >>
+                  drule_then strip_assume_tac extends_appends >>
+                  rveq >> fs[init_ctxt_def] >>
+                  fs[MEM_MAP,PULL_EXISTS] >> res_tac >>
+                  fs[]) >>
+             simp[SimpL``$=``,ext_term_frag_builtins_def] >>
+             qmatch_goalsub_abbrev_tac `type_interpretation_of ind ctxt` >>
+             `is_frag_interpretation (total_fragment (sigof ctxt))
+                (type_interpretation_of ind ctxt)
+                (UNCURRY (term_interpretation_of ind ctxt))`
+               by(fs[Abbr `ctxt`]) >>
+             `(s,TYPE_SUBSTf sigma (typeof t)) ∈ ground_consts (sigof ctxt)`
+               by(rw[Abbr`ctxt`] >>
+                  simp[ground_consts_def] >>
+                  conj_tac >-
+                    (rw[ground_types_def,tyvars_TYPE_SUBSTf_eq_NIL] >>
+                     match_mp_tac type_ok_TYPE_SUBSTf >>
+                     simp[] >>
+                     fs[EVERY_MEM,MEM_MAP,PULL_EXISTS] >> res_tac >> fs[] >>
+                     rfs[term_ok_clauses]) >>
+                  rw[term_ok_def,Abbr`tmenv`,FLOOKUP_FUNION] >>
+                  reverse(Cases_on `ALOOKUP (const_list ctxt1) s`) >-
+                    (imp_res_tac ALOOKUP_MEM >>
+                     res_tac >> metis_tac[FST]) >>
+                  simp[] >>
+                  simp[ALOOKUP_MAP] >>
+                  fs[constspec_ok_def] >>
+                  dxrule_then dxrule ALOOKUP_ALL_DISTINCT_MEM >>
+                  drule_then drule ALOOKUP_ALL_DISTINCT_MEM >>
+                  simp[] >> ntac 2 (disch_then kall_tac) >>
+                  conj_tac >-
+                    (match_mp_tac type_ok_TYPE_SUBSTf >>
+                     simp[] >>
+                     fs[EVERY_MEM,MEM_MAP,PULL_EXISTS] >> res_tac >> fs[] >>
+                     rfs[term_ok_clauses]) >>
+                  metis_tac[TYPE_SUBSTf_eq_TYPE_SUBST]) >>
+             `(s,TYPE_SUBSTf sigma (typeof t)) ∈ nonbuiltin_constinsts`
+               by(rw[nonbuiltin_constinsts_def,builtin_consts_def]) >>
+             Q.SUBGOAL_THEN `inhabited ind` assume_tac >- metis_tac[] >>
+             simp[type_interpretation_of_alt] >>
+             simp[Abbr `ctxt`,FILTER_APPEND] >>
+             qmatch_goalsub_abbrev_tac `FILTER fff lll` >>
+             `FILTER fff lll = []`
+               by(fs[Abbr `fff`,Abbr `lll`,FILTER_EQ_NIL,EVERY_MEM,MEM_MAP,PULL_EXISTS] >>
+                  strip_tac >>
+                  disch_then(strip_assume_tac o REWRITE_RULE[MEM_SPLIT]) >> rveq >>
+                  rename1` defn_matches _ _ aaa` >> Cases_on `aaa` >> fs[defn_matches_def] >>
+                  fs[FILTER_EQ_NIL,EVERY_MEM] >>
+                  FULL_SIMP_TAC bool_ss [GSYM APPEND_ASSOC] >>
+                  drule_then (assume_tac o C MATCH_MP init_ctxt_extends) extends_trans >>
+                  dxrule_then assume_tac extends_APPEND_NIL >>
+                  fs[] >>
+                  dxrule_then assume_tac extends_NIL_CONS_updates >>
+                  Cases >> strip_tac >>
+                  fs[updates_cases,constspec_ok_def] >>
+                  reverse(Cases_on `b`) >-
+                    (fs[MEM_MAP,PULL_EXISTS] >>
+                     first_x_assum drule >>
+                     qpat_x_assum `!y. MEM y eqs ==> !y'. _` assume_tac >>
+                     first_x_assum drule >>
+                     rpt strip_tac >>
+                     spose_not_then strip_assume_tac >>
+                     rveq >>
+                     first_x_assum(qspec_then `(q,t)` mp_tac) >>
+                     simp[]) >>
+                  fs[] >>
+                  first_x_assum drule >>
+                  strip_tac
+                  >- (qpat_x_assum `MEM (NewConst _ _) _` (strip_assume_tac o REWRITE_RULE[MEM_SPLIT]) >>
+                      rveq >>
+                      qpat_x_assum `!y. MEM y eqs ==> !y'. _` assume_tac >>
+                      first_x_assum drule >>
+                      rpt strip_tac >>
+                      fs[] >> metis_tac[FST]) >>
+                  qpat_x_assum `MEM (NewConst _ _) _` (strip_assume_tac o REWRITE_RULE[MEM_SPLIT]) >>
+                  rveq >> fs[MEM_MAP,PULL_EXISTS] >>
+                  qpat_x_assum `!y. MEM y eqs ==> !y'. _` assume_tac >>
+                  first_x_assum drule >>
+                  rpt strip_tac >>
+                  fs[] >> metis_tac[FST]) >>
+             pop_assum SUBST_ALL_TAC >>
+             qunabbrev_tac `lll` >>
+             qmatch_goalsub_abbrev_tac `FILTER fff lll` >>
+             `FILTER fff lll = []`
+               by(fs[Abbr `fff`,Abbr `lll`,FILTER_EQ_NIL,EVERY_MEM,MEM_MAP,PULL_EXISTS] >>
+                  strip_tac >>
+                  disch_then(strip_assume_tac o REWRITE_RULE[MEM_SPLIT]) >> rveq >>
+                  rename1` defn_matches _ _ aaa` >> Cases_on `aaa` >> fs[defn_matches_def] >>
+                  fs[FILTER_EQ_NIL,EVERY_MEM] >>
+                  fs[constspec_ok_def] >>
+                  Cases >> disch_then(strip_assume_tac o REWRITE_RULE[MEM_SPLIT]) >> rveq >>
+                  reverse(Cases_on `b`) >-
+                    (fs[MEM_MAP,PULL_EXISTS] >>
+                     qpat_x_assum `!y. MEM y eqs ==> !y'. _` assume_tac >>
+                     first_x_assum drule >>
+                     rpt strip_tac >>
+                     fs[] >> metis_tac[FST]) >>
+                  fs[] >>
+                  qpat_x_assum `_ ++ ConstSpec T _ _::_ extends _` assume_tac >>
+                  drule_then (assume_tac o C MATCH_MP init_ctxt_extends) extends_trans >>
+                  dxrule_then assume_tac extends_APPEND_NIL >>
+                  fs[] >>
+                  dxrule_then assume_tac extends_NIL_CONS_updates >>
+                  fs[updates_cases,constspec_ok_def,DISJ_IMP_THM,FORALL_AND_THM] >>
+                  qpat_x_assum `MEM (NewConst _ _) _` (strip_assume_tac o REWRITE_RULE[MEM_SPLIT]) >>
+                  rveq >> fs[] >>
+                  metis_tac[MEM_MAP,FST]) >>
+             pop_assum SUBST_ALL_TAC >>
+             simp[] >>
+             MAP_EVERY qunabbrev_tac [`fff`,`lll`] >>
+             simp[defn_matches_def] >>
+             qmatch_goalsub_abbrev_tac `FILTER fff lll` >>
+             `FILTER fff lll = [(s,t)]`
+               by(MAP_EVERY qunabbrev_tac [`fff`,`lll`] >>
+                  qpat_x_assum `MEM _ eqs` (strip_assume_tac o REWRITE_RULE[MEM_SPLIT]) >> rveq >>
+                  fs[FILTER_APPEND] >>
+                  reverse IF_CASES_TAC >- metis_tac[TYPE_SUBSTf_eq_TYPE_SUBST] >>
+                  simp[APPEND_EQ_CONS] >>
+                  fs[constspec_ok_def,ALL_DISTINCT_APPEND,IMP_CONJ_THM,FORALL_AND_THM,DISJ_IMP_THM] >>
+                  fs[FILTER_EQ_NIL,EVERY_MEM] >>
+                  conj_tac >> Cases >> fs[MEM_MAP,PULL_EXISTS] >> metis_tac[FST]) >>
+             pop_assum SUBST_ALL_TAC >> simp[] >>
+             fs[Abbr `fff`,Abbr `lll`] >>
+             TOP_CASE_TAC >-
+               (goal_assum kall_tac >>
+                Q.SUBGOAL_THEN `is_instance (typeof t) (TYPE_SUBSTf sigma (typeof t))` assume_tac >-
+                  metis_tac[TYPE_SUBSTf_eq_TYPE_SUBST] >>
+                metis_tac[instance_subst_completeness,IS_SOME_DEF]) >>
+             rename1 `instance_subst _ _ _ = SOME result` >>
+             Cases_on `result` >>
+             rename1 `instance_subst _ _ _ = SOME(sigma',e)` >>
+             drule_then (assume_tac o GSYM) instance_subst_soundness >>
+             simp[ELIM_UNCURRY] >>
+             qmatch_goalsub_abbrev_tac `termsem a1 a2 a3 a4 t = termsem _ _ a5 _ _` >>
+             `termsem a1 a2 a3 a4 t = termsem a1 a2 a5 a4 t`
+               by(MAP_EVERY qunabbrev_tac [`a1`,`a2`,`a3`,`a4`,`a5`] >>
+                  match_mp_tac termsem_frees >>
+                  res_tac >> fs[CLOSED_def] >>
+                  rfs[term_ok_equation] >> imp_res_tac term_ok_welltyped) >>
+             pop_assum SUBST_ALL_TAC >>
+             match_mp_tac termsem_subst >>
+             conj_tac >-
+               (MAP_EVERY qunabbrev_tac [`a1`,`a2`,`a3`,`a4`,`a5`] >>
+                res_tac >> fs[] >> rfs[term_ok_equation] >> imp_res_tac term_ok_welltyped) >>
+             MAP_EVERY qunabbrev_tac [`a1`,`a2`,`a3`,`a4`,`a5`] >>
+             fs[TYPE_SUBST_eq_TYPE_SUBSTf,TYPE_SUBSTf_eq_TYPE_SUBSTf] >>
+             metis_tac[SND]) >>
+            simp[])
+     )
+  >- ((* NewType *)
+      fs[conexts_of_upd_def])
+  >- ((* TypeDefn *)
+      rename1 `elem ⋲ ind` >>
+      fs[conexts_of_upd_def] >>
+      rw[satisfies_t_def,satisfies_def,termsem_def] >>
+      `~MEM name (MAP FST (type_list ctxt1))`
+        by(drule_then (assume_tac o C MATCH_MP init_ctxt_extends) extends_trans >>
+           drule extends_NIL_DISJOINT >>
+           rw[]) >>
+      `~MEM abs (MAP FST (const_list ctxt1))`
+        by(drule_then (assume_tac o C MATCH_MP init_ctxt_extends) extends_trans >>
+           drule extends_NIL_DISJOINT >>
+           rw[]) >>
+      `~MEM rep (MAP FST (const_list ctxt1))`
+        by(drule_then (assume_tac o C MATCH_MP init_ctxt_extends) extends_trans >>
+           drule extends_NIL_DISJOINT >>
+           rw[]) >>
+      `ALOOKUP (type_list ctxt1) name = NONE`
+        by rw[ALOOKUP_NONE] >>
+       `ALOOKUP (const_list ctxt1) abs = NONE`
+        by rw[ALOOKUP_NONE] >>
+      `ALOOKUP (const_list ctxt1) rep = NONE`
+        by rw[ALOOKUP_NONE]
+      >- ((* First abs/rep axiom *)
+       drule proves_theory_mono >>
+       qmatch_asmsub_abbrev_tac `total_fragment (tyenv,tmenv)` >>
+       disch_then(qspecl_then [`tysof ctxt2`,`tmsof ctxt2`,`axsof ctxt2`,
+                               `tyenv`,`tmenv`] mp_tac) >>
+       simp[] >>
+       MAP_EVERY qunabbrev_tac [`tyenv`,`tmenv`] >>
+       impl_tac >-
+         (rw[] >>
+          TRY(match_mp_tac (CONJUNCT2 SUBMAP_FUNION_ID) >> rw[FDOM_FUPDATE] >>
+              drule_then (assume_tac o C MATCH_MP init_ctxt_extends) extends_trans >>
+              drule extends_NIL_DISJOINT >>
+              simp[] >> NO_TAC) >>
+          qhdtm_x_assum `theory_ok` mp_tac >>
+          rw[theory_ok_def]) >>
+      strip_tac >>
+      drule_then drule (MP_CANON termsem_ext_equation) >>
+      disch_then drule >>
+      fs[valuates_frag_builtins] >>
+      disch_then drule >>
+      drule_then drule terms_of_frag_uninst_equationE >>
+      impl_keep_tac >- rw[welltyped_equation,EQUATION_HAS_TYPE_BOOL] >>
+      disch_then (MAP_EVERY assume_tac o rev o CONJUNCTS) >>
+      ntac 2 (disch_then dxrule) >>
+      impl_keep_tac >-
+        (rw[term_ok_clauses] >> rw[term_ok_def] >>
+         qpat_assum `is_std_sig(FUNION _ _,_)` (strip_assume_tac o REWRITE_RULE[is_std_sig_def]) >>
+         rw[type_ok_def,EVERY_MEM,MEM_MAP,FLOOKUP_FUNION,FLOOKUP_UPDATE] >>
+         rw[type_ok_def] >>
+         drule proves_term_ok >>
+         rw[EVERY_MEM,term_ok_def] >> rw[] >>
+         drule_then drule term_ok_type_ok >> rw[]) >>
+      simp[termsem_ext_def] >>
+      disch_then kall_tac >>
+      rw[boolean_eq_true] >>
+      rw[termsem_def] >>
+      `~MEM (strlit "=") (MAP FST (const_list ctxt1))`
+        by(drule_then strip_assume_tac extends_appends >>
+           fs[APPEND_EQ_APPEND,init_ctxt_def] >>
+           rveq >> fs[] >>
+           fs[APPEND_EQ_CONS |> CONV_RULE(LHS_CONV SYM_CONV)] >>
+           rveq >> fs[] >>
+           drule_then(assume_tac o C MATCH_MP (REWRITE_RULE[init_ctxt_def] init_ctxt_extends))
+                     extends_trans >>
+           drule extends_NIL_DISJOINT >>
+           rw[]) >>
+      `MEM (strlit "=") (MAP FST (const_list ctxt2))`
+        by(imp_res_tac extends_appends >> rw[init_ctxt_def]) >>
+      `abs <> strlit "="` by(CCONTR_TAC >> fs[]) >>
+      `rep <> strlit "="` by(CCONTR_TAC >> fs[]) >>
+      simp[ext_term_frag_builtins_def] >>
+      qmatch_asmsub_abbrev_tac `total_fragment (tyenv,tmenv)` >>
+      `models (type_interpretation_of ind (ctxt1 ++ TypeDefn name pred abs rep::ctxt2))
+              (UNCURRY (term_interpretation_of ind (ctxt1 ++ TypeDefn name pred abs rep::ctxt2)))
+              ((tyenv,tmenv),axsof ctxt2)`
+        by(rw[models_def]) >>
+      drule_then drule proves_sound >>
+      simp[entails_def] >>
+      strip_tac >>
+      first_x_assum drule >>
+      simp[satisfies_t_def] >>
+      ntac 2 (disch_then drule) >>
+      impl_keep_tac >-
+        (rw[ground_terms_uninst_def] >>
+         goal_assum drule >>
+         rw[ground_types_def,tyvars_def] >>
+         imp_res_tac term_ok_type_ok >>
+         qpat_x_assum `is_std_sig (tyenv,tmenv)` mp_tac >>
+         rw[is_std_sig_def,type_ok_def]) >>
+      simp[satisfies_def] >>
+      simp[valuates_frag_builtins] >>
+      disch_then drule >>
+      impl_tac >-
+        (match_mp_tac terms_of_frag_uninst_term_ok >> simp[]) >>
+      simp[termsem_def] >> strip_tac >>
+      `termsem
+           (ext_type_frag_builtins
+              (type_interpretation_of ind (ctxt1 ++ TypeDefn name pred abs rep::ctxt2)))
+           (ext_term_frag_builtins
+              (ext_type_frag_builtins
+                 (type_interpretation_of ind (ctxt1 ++ TypeDefn name pred abs rep::ctxt2)))
+              (UNCURRY
+                 (term_interpretation_of ind (ctxt1 ++ TypeDefn name pred abs rep::ctxt2))))
+           v sigma witness ⋲
+         (ext_type_frag_builtins
+              (type_interpretation_of ind (ctxt1 ++ TypeDefn name pred abs rep::ctxt2)))
+           (TYPE_SUBSTf sigma (typeof witness))
+      `
+        by(match_mp_tac termsem_in_type_ext2 >>
+           rpt(goal_assum drule) >>
+           conj_tac >-
+             (match_mp_tac terms_of_frag_uninst_term_ok >>
+              simp[] >>
+              drule proves_term_ok >>
+              rw[EVERY_MEM,MEM_MAP,term_ok_def]) >>
+           rpt strip_tac >>
+           qpat_x_assum `valuates_frag _ _ _ _` mp_tac >>
+           simp[valuates_frag_def] >>
+           disch_then match_mp_tac >>
+           match_mp_tac TYPE_SUBSTf_in_types_of_frag_I >>
+           goal_assum drule >>
+           goal_assum drule >>
+           match_mp_tac terms_of_frag_uninst_term_ok >>
+           simp[] >>
+           drule proves_term_ok >> rw[EVERY_MEM,MEM_MAP,term_ok_def]) >>
+      qmatch_goalsub_abbrev_tac `term_interpretation_of ind _ abs abstype` >>
+      qmatch_goalsub_abbrev_tac `term_interpretation_of ind _ rep reptype` >>
+      `(abs,abstype) ∈ ground_consts (sigof(ctxt1 ++ TypeDefn name pred abs rep::ctxt2))`
+        by(fs[Abbr `abstype`,ground_consts_def,ground_types_def] >>
+           conj_tac >-
+             (simp[tyvars_def,LIST_UNION_EQ_NIL,tyvars_TYPE_SUBSTf_eq_NIL] >>
+              match_mp_tac FOLDR_LIST_UNION_empty >>
+              rw[EVERY_MEM,MEM_MAP,PULL_EXISTS]) >>
+           conj_asm1_tac >-
+             (qmatch_goalsub_abbrev_tac `type_ok tyenv'` >>
+              `tyenv' = tysof(tyenv,tmenv)`
+                by(fs[Abbr `tyenv`,Abbr `tmenv`,Abbr`tyenv'`] >>
+                   fs[GSYM FUNION_ASSOC,FUNION_FUPDATE_1]) >>
+              pop_assum SUBST_ALL_TAC >>
+              simp[term_ok_clauses] >>
+              conj_tac >-
+                (match_mp_tac type_ok_TYPE_SUBSTf >> simp[] >>
+                 qpat_x_assum `term_ok _ (Comb _ _)` mp_tac >>
+                 simp[term_ok_clauses] >>
+                 rpt strip_tac >>
+                 simp[] >> metis_tac[term_ok_type_ok,FST]) >>
+              simp[type_ok_def,EVERY_MAP,MEM_MAP,PULL_EXISTS] >>
+              rw[Abbr `tyenv`,FLOOKUP_FUNION,FLOOKUP_UPDATE]) >>
+           rw[term_ok_def,FLOOKUP_FUNION,FLOOKUP_UPDATE] >>
+           qexists_tac `(MAP (λx. (sigma x,Tyvar x)) (tvars pred))` >>
+           simp[TYPE_SUBST_eq_TYPE_SUBSTf,MAP_EQ_f,MEM_MAP,PULL_EXISTS,
+                REV_ASSOCD_ALOOKUP,MAP_MAP_o,o_DEF,ALOOKUP_Tyvar,ALOOKUP_MAPf] >>
+           simp[TYPE_SUBSTf_eq_TYPE_SUBSTf] >>
+           rfs[term_ok_clauses] >>
+           rpt strip_tac >>
+           IF_CASES_TAC >> simp[] >>
+           fs[welltyped_def] >> qpat_x_assum `pred has_type _` assume_tac >>
+           drule_then assume_tac WELLTYPED_LEMMA >> rveq >>
+           drule_then (mp_tac o REWRITE_RULE[SUBSET_DEF,Once MONO_NOT_EQ]) tyvars_typeof_subset_tvars >>
+           disch_then drule >>
+           simp[tyvars_def]) >>
+      `(abs,abstype) ∈ nonbuiltin_constinsts`
+        by simp[nonbuiltin_constinsts_def,builtin_consts_def] >>
+      `(rep,reptype) ∈ ground_consts (sigof(ctxt1 ++ TypeDefn name pred abs rep::ctxt2))`
+        by(qpat_x_assum `(abs,abstype) ∈ ground_consts _` mp_tac >>
+           fs[Abbr `reptype`,Abbr `abstype`,ground_consts_def,ground_types_def] >>
+           qmatch_goalsub_abbrev_tac `type_ok tyenv'` >>
+           `tyenv' = tysof(tyenv,tmenv)`
+                by(fs[Abbr `tyenv`,Abbr `tmenv`,Abbr`tyenv'`] >>
+                   fs[GSYM FUNION_ASSOC,FUNION_FUPDATE_1]) >>
+           pop_assum SUBST_ALL_TAC >>
+           simp[term_ok_clauses] >>
+           simp[tyvars_def,LIST_UNION_EQ_NIL] >>
+           rw[term_ok_def,term_ok_clauses,FLOOKUP_FUNION,FLOOKUP_UPDATE,MAP_EQ_f] >>
+           fs[type_ok_def] >>
+           metis_tac[]) >>
+      `(rep,reptype) ∈ nonbuiltin_constinsts`
+        by simp[nonbuiltin_constinsts_def,builtin_consts_def] >>
+      `is_frag_interpretation (total_fragment (sigof (ctxt1 ++ TypeDefn name pred abs rep::ctxt2)))
+          (type_interpretation_of ind
+             (ctxt1 ++ TypeDefn name pred abs rep::ctxt2))
+          (UNCURRY
+             (term_interpretation_of ind
+                (ctxt1 ++ TypeDefn name pred abs rep::ctxt2)))`
+        by(qhdtm_x_assum `is_frag_interpretation0` mp_tac >>
+           simp[Abbr `tyenv`,Abbr `tmenv`,GSYM FUNION_ASSOC,FUNION_FUPDATE_1]) >>
+      MAP_EVERY qunabbrev_tac [`abstype`,`reptype`] >>
+      Q.SUBGOAL_THEN `inhabited ind` assume_tac >- metis_tac[] >>
+      simp[type_interpretation_of_alt] >>
+      qpat_x_assum `inhabited ind` kall_tac >>
+      simp[FILTER_APPEND] >>
+      IF_CASES_TAC >- fs[defn_matches_def] >>
+      Cases_on `[] ≠
+              defn_matches rep
+                (Fun
+                   (Tyapp name
+                      (MAP (λa. TYPE_SUBSTf sigma a)
+                         (MAP Tyvar
+                            (MAP implode
+                               (STRING_SORT (MAP explode (tvars pred)))))))
+                   (TYPE_SUBSTf sigma (domain (typeof pred))))
+                (TypeDefn name pred abs rep)` >-
+        (fs[defn_matches_def]) >>
+      simp[] >>
+      ntac 2 (pop_assum kall_tac) >>
+      ntac 2 (
+        qmatch_goalsub_abbrev_tac `FILTER ff ll` >>
+        `FILTER ff ll = []`
+          by(simp[Abbr `ff`,Abbr `ll`,FILTER_EQ_NIL,EVERY_MEM,MEM_MAP,PULL_EXISTS,
+                  defn_matches_def] >> rpt strip_tac >>
+             TOP_CASE_TAC >> simp[] >>
+             simp[FILTER_EQ_NIL,EVERY_MEM,MEM_MAP,PULL_EXISTS] >>
+             Cases >> simp[] >> strip_tac >>
+             simp[RIGHT_FORALL_OR_THM] >> disj1_tac >>
+             qpat_x_assum `MEM (ConstSpec _ _ _) _` (strip_assume_tac o REWRITE_RULE[MEM_SPLIT]) >>
+             rveq >>
+             drule_then (assume_tac o C MATCH_MP init_ctxt_extends) extends_trans >>
+             FULL_SIMP_TAC bool_ss [GSYM APPEND_ASSOC] >>
+             dxrule_then assume_tac extends_APPEND_NIL >>
+             fs[] >>
+             dxrule_then assume_tac extends_NIL_CONS_updates >>
+             Cases_on `b` >>
+             fs[updates_cases,constspec_ok_def]
+             >- (pop_assum(drule_then strip_assume_tac) >>
+                 qpat_x_assum `MEM (NewConst _ _) _` (strip_assume_tac o REWRITE_RULE[MEM_SPLIT]) >>
+                 fs[]) >>
+             qpat_x_assum `MEM (_,_) l` (strip_assume_tac o REWRITE_RULE[MEM_SPLIT]) >>
+             fs[]) >>
+        pop_assum SUBST_ALL_TAC >>
+        MAP_EVERY qunabbrev_tac [`ff`,`ll`] >>
+        qmatch_goalsub_abbrev_tac `FILTER ff ll` >>
+        `FILTER ff ll = []`
+          by(simp[Abbr `ff`,Abbr `ll`,FILTER_EQ_NIL,EVERY_MEM,MEM_MAP,PULL_EXISTS,
+                  defn_matches_def] >> rpt strip_tac >>
+             TOP_CASE_TAC >> simp[] >>
+             simp[FILTER_EQ_NIL,EVERY_MEM,MEM_MAP,PULL_EXISTS] >>
+             Cases >> simp[] >> strip_tac >>
+             simp[RIGHT_FORALL_OR_THM] >> disj1_tac >>
+             qpat_x_assum `MEM (ConstSpec _ _ _) _` (strip_assume_tac o REWRITE_RULE[MEM_SPLIT]) >>
+             rveq >>
+             drule_then (assume_tac o C MATCH_MP init_ctxt_extends) extends_trans >>
+             dxrule_then assume_tac extends_APPEND_NIL >>
+             dxrule_then assume_tac (extends_APPEND_NIL |> Q.SPEC `[e]` |> REWRITE_RULE[APPEND]) >>
+             dxrule_then assume_tac extends_APPEND_NIL >>
+             dxrule_then assume_tac extends_NIL_CONS_updates >>
+             Cases_on `b` >>
+             fs[updates_cases,constspec_ok_def]
+             >- (pop_assum(drule_then strip_assume_tac) >>
+                 qpat_x_assum `MEM (NewConst _ _) _` (strip_assume_tac o REWRITE_RULE[MEM_SPLIT]) >>
+                 fs[])
+             >- (pop_assum(drule_then strip_assume_tac) >>
+                 qpat_x_assum `MEM (NewConst _ _) _` (strip_assume_tac o REWRITE_RULE[MEM_SPLIT]) >>
+                 fs[]) >>
+             qpat_x_assum `MEM (_,_) l` (strip_assume_tac o REWRITE_RULE[MEM_SPLIT]) >>
+             fs[]) >>
+        pop_assum SUBST_ALL_TAC >>
+        MAP_EVERY qunabbrev_tac [`ff`,`ll`]) >>
+      simp[] >>
+      simp[mllistTheory.mapPartial_def,mapPartial_APPEND] >>
+      rpt
+        (qmatch_goalsub_abbrev_tac `mapPartial a1 a2` >>
+        `mapPartial a1 a2 = []`
+          by(rw[Abbr `a1`,Abbr `a2`,mllistTheory.mapPartial_thm,FILTER_EQ_NIL,EVERY_MEM,MEM_MAP,
+                PULL_EXISTS] >>
+             simp[abs_or_rep_matches_def,abs_matches_def,rep_matches_def] >>
+             ntac 3 (PURE_TOP_CASE_TAC >> fs[] >> rveq) >>
+             fs[pair_case_eq] >>
+             PURE_FULL_CASE_TAC >> fs[] >> rveq >>
+             qpat_x_assum `MEM (TypeDefn _ _ _ _) _` (strip_assume_tac o REWRITE_RULE[MEM_SPLIT]) >>
+             rveq >>
+             drule_then (assume_tac o C MATCH_MP init_ctxt_extends) extends_trans >>
+             dxrule_then assume_tac extends_APPEND_NIL >>
+             dxrule_then assume_tac extends_NIL_CONS_updates >>
+             fs[updates_cases]) >>
+        pop_assum SUBST_ALL_TAC >>
+        MAP_EVERY qunabbrev_tac [`a1`,`a2`]) >>
+      simp[abs_or_rep_matches_def,abs_matches_def,rep_matches_def] >>
+      reverse IF_CASES_TAC >-
+        (goal_assum kall_tac >>
+         pop_assum mp_tac >> simp[] >>
+         simp[TYPE_SUBSTf_eq_TYPE_SUBST] >>
+         rw[MAP_EQ_f,MEM_MAP,PULL_EXISTS] >>
+         qexists_tac `MAP (λx. (sigma x,Tyvar x)) (tvars pred)` >>
+         conj_tac >-
+           (rw[TYPE_SUBST_tyvars,REV_ASSOCD_ALOOKUP] >>
+            ntac 2 TOP_CASE_TAC >>
+            fs[ALOOKUP_NONE,MEM_MAP,GSYM IMP_DISJ_THM,PULL_FORALL] >>
+            imp_res_tac ALOOKUP_MEM >>
+            fs[MEM_MAP] >> rveq >> pairarg_tac >> rveq >> fs[] >>
+            rveq >> fs[] >> rveq >> fs[] >>
+            rfs[term_ok_def] >> rfs[] >> fs[welltyped_def] >>
+            imp_res_tac WELLTYPED_LEMMA >> rveq >>
+            `MEM x (tyvars(typeof pred))` by simp[tyvars_def] >>
+            drule_then drule (tyvars_typeof_subset_tvars |> REWRITE_RULE[SUBSET_DEF] |> MP_CANON) >>
+            simp[]) >>
+         strip_tac >>
+         simp[REV_ASSOCD_ALOOKUP,ALOOKUP_MAP,MAP_MAP_o,o_DEF,tyvars_def] >>
+         simp[ALOOKUP_Tyvar,ALOOKUP_MAPf]) >>
+      simp[] >>
+      qmatch_goalsub_abbrev_tac `if a1 then SOME _ else NONE` >>
+      reverse(first_assum (fn thm =>
+                              qunabbrev_tac `a1` >>
+                              Cases_on [ANTIQUOTE (rhs(rand(concl thm)))])) >-
+        (goal_assum kall_tac >>
+         pop_assum mp_tac >> pop_assum kall_tac >> simp[] >>
+         simp[TYPE_SUBSTf_eq_TYPE_SUBST] >>
+         rw[MAP_EQ_f,MEM_MAP,PULL_EXISTS] >>
+         qexists_tac `MAP (λx. (sigma x,Tyvar x)) (tvars pred)` >>
+         reverse conj_tac >-
+           (rw[TYPE_SUBST_tyvars,REV_ASSOCD_ALOOKUP] >>
+            ntac 2 TOP_CASE_TAC >>
+            fs[ALOOKUP_NONE,MEM_MAP,GSYM IMP_DISJ_THM,PULL_FORALL] >>
+            imp_res_tac ALOOKUP_MEM >>
+            fs[MEM_MAP] >> rveq >> pairarg_tac >> rveq >> fs[] >>
+            rveq >> fs[] >> rveq >> fs[] >>
+            rfs[term_ok_def] >> rfs[] >> fs[welltyped_def] >>
+            imp_res_tac WELLTYPED_LEMMA >> rveq >>
+            `MEM x (tyvars(typeof pred))` by simp[tyvars_def] >>
+            drule_then drule (tyvars_typeof_subset_tvars |> REWRITE_RULE[SUBSET_DEF] |> MP_CANON) >>
+            simp[]) >>
+         strip_tac >>
+         simp[REV_ASSOCD_ALOOKUP,ALOOKUP_MAP,MAP_MAP_o,o_DEF,tyvars_def] >>
+         simp[ALOOKUP_Tyvar,ALOOKUP_MAPf]) >>
+      simp[] >>
+      qmatch_goalsub_abbrev_tac `instance_subst [(ty0,ty1)]` >>
+      Q.SUBGOAL_THEN `is_instance ty1 ty0` mp_tac >-
+        (fs[Abbr `ty0`,Abbr`ty1`] >> metis_tac[]) >>
+      disch_then (strip_assume_tac o REWRITE_RULE[instance_subst_completeness,IS_SOME_EXISTS]) >>
+      rename1 `instance_subst _ _ _ = SOME result` >>
+      Cases_on `result` >>
+      rename1 `SOME(sigma',stuff)` >>
+      simp[] >>
+      drule_then assume_tac instance_subst_soundness >>
+      MAP_EVERY qunabbrev_tac [`ty0`,`ty1`] >>
+      qmatch_goalsub_abbrev_tac `instance_subst [ty0,ty1]` >>
+      Q.SUBGOAL_THEN `is_instance ty1 ty0` mp_tac >-
+        (fs[Abbr `ty0`,Abbr`ty1`] >> metis_tac[]) >>
+      disch_then (strip_assume_tac o REWRITE_RULE[instance_subst_completeness,IS_SOME_EXISTS]) >>
+      rename1 `instance_subst _ _ _ = SOME result` >>
+      Cases_on `result` >>
+      rename1 `SOME(sigma'',stuff')` >>
+      simp[] >>
+      drule_then assume_tac instance_subst_soundness >>
+      MAP_EVERY qunabbrev_tac [`ty0`,`ty1`] >>
+      ntac 2 (PRED_ASSUM is_exists kall_tac) >>
+      rpt(qpat_x_assum `Fun _ _ = TYPE_SUBST _ _` (mp_tac o GSYM)) >>
+      rw[] >> fs[MAP_EQ_f,MEM_MAP,PULL_EXISTS] >>
+      qmatch_goalsub_abbrev_tac `ext_type_frag_builtins _ (Tyapp name ntys)` >>
+      `Tyapp name ntys ∈ nonbuiltin_types`
+        by(simp[Abbr`ntys`] >>
+           drule_then strip_assume_tac extends_appends >>
+           fs[APPEND_EQ_APPEND,init_ctxt_def,
+              APPEND_EQ_CONS |> CONV_RULE(LHS_CONV SYM_CONV)] >>
+           rveq >> fs[] >>
+           last_assum(qspec_then `(name,0)` mp_tac) >>
+           last_x_assum(qspec_then `(name,2)` mp_tac) >>
+           simp[] >>
+           rw[nonbuiltin_types_def,is_builtin_type_def]) >>
+      qunabbrev_tac `ntys` >>
+      simp[ext_type_frag_builtins_nonbuiltin] >>
+      qmatch_goalsub_abbrev_tac `v (vname,vty)` >>
+      `v (vname,vty) ⋲ (type_interpretation_of ind (ctxt1 ++ TypeDefn name pred abs rep::ctxt2)) (TYPE_SUBSTf sigma vty)`
+        by(qhdtm_x_assum `valuates_frag0` mp_tac >>
+           simp[valuates_frag_def] >>
+           disch_then(qspecl_then [`vname`,`vty`] mp_tac) >>
+           simp[Abbr `vty`,ext_type_frag_builtins_nonbuiltin] >>
+           disch_then match_mp_tac >>
+           drule_then drule terms_of_frag_uninst_equationE >>
+           impl_tac >- simp[welltyped_equation] >>
+           strip_tac >>
+           PURE_REWRITE_TAC[GSYM TYPE_SUBSTf_def] >>
+           match_mp_tac TYPE_SUBSTf_in_types_of_frag_I >>
+           Q.REFINE_EXISTS_TAC `Var _ _` >>
+           simp[] >>
+           metis_tac[]) >>
+      `TYPE_SUBSTf sigma vty ∈ ground_types (sigof (ctxt1 ++ TypeDefn name pred abs rep::ctxt2))`
+        by(qunabbrev_tac `vty` >>
+           simp[ground_types_def,tyvars_def,type_ok_def,EVERY_MEM,MEM_MAP,PULL_EXISTS,
+                FLOOKUP_FUNION,FLOOKUP_UPDATE] >>
+           fs[Abbr`tyenv`,GSYM FUNION_ASSOC,FUNION_FUPDATE_1] >>
+           match_mp_tac FOLDR_LIST_UNION_empty >>
+           rw[EVERY_MEM,MEM_MAP,PULL_EXISTS]) >>
+      `v (vname,vty) ⋲ ext_type_frag_builtins(type_interpretation_of ind (ctxt1 ++ TypeDefn name pred abs rep::ctxt2)) (TYPE_SUBSTf sigma (domain(typeof pred)))`
+        by(qpat_x_assum `_ ⋲ type_interpretation_of ind _ _` mp_tac >>
+           fs[Abbr `vty`] >>
+           Q.SUBGOAL_THEN `inhabited ind` assume_tac >- metis_tac[] >>
+           simp[type_interpretation_of_alt] >>
+           qpat_x_assum `inhabited ind` kall_tac >>
+           simp[mllistTheory.mapPartial_thm,FILTER_APPEND] >>
+           qmatch_goalsub_abbrev_tac `FILTER IS_SOME (MAP f1 c1)` >>
+           `FILTER IS_SOME (MAP f1 c1) = []`
+             by(fs[Abbr `f1`,Abbr `c1`,FILTER_EQ_NIL,EVERY_MEM,MEM_MAP,PULL_EXISTS] >>
+                strip_tac >>
+                simp[type_matches_def] >>
+                TOP_CASE_TAC >> fs[] >>
+                strip_tac >>
+                pop_assum(strip_assume_tac o REWRITE_RULE[MEM_SPLIT]) >>
+                fs[] >> metis_tac[FST,SND]) >>
+           MAP_EVERY qunabbrev_tac [`f1`,`c1`] >>
+           simp[] >>
+           qmatch_goalsub_abbrev_tac `FILTER IS_SOME (MAP f1 c1)` >>
+           `FILTER IS_SOME (MAP f1 c1) = []`
+             by(fs[Abbr `f1`,Abbr `c1`,FILTER_EQ_NIL,EVERY_MEM,MEM_MAP,PULL_EXISTS] >>
+                strip_tac >>
+                simp[type_matches_def] >>
+                TOP_CASE_TAC >> fs[] >>
+                strip_tac >>
+                pop_assum(strip_assume_tac o REWRITE_RULE[MEM_SPLIT]) >>
+                fs[] >> metis_tac[FST,SND]) >>
+           MAP_EVERY qunabbrev_tac [`f1`,`c1`] >>
+           simp[] >>
+           simp[type_matches_def] >>
+           qmatch_goalsub_abbrev_tac `if predd then SOME _ else NONE` >>
+           Q.SUBGOAL_THEN `predd` assume_tac >-
+             (qunabbrev_tac `predd` >>
+              simp[MAP_EQ_f,MEM_MAP,PULL_EXISTS,REV_ASSOCD_ALOOKUP] >>
+              qexists_tac `MAP (λx. (sigma x, Tyvar x)) (tvars pred)` >>
+              simp[ALOOKUP_Tyvar,MAP_MAP_o,o_DEF,ALOOKUP_MAPf]) >>
+           qunabbrev_tac `predd` >>
+           simp[] >>
+           qmatch_goalsub_abbrev_tac `instance_subst [(ty0,ty1)]` >>
+           Q.SUBGOAL_THEN `is_instance ty1 ty0` mp_tac >-
+             (fs[Abbr `ty0`,Abbr`ty1`] >> metis_tac[]) >>
+           disch_then (strip_assume_tac o REWRITE_RULE[instance_subst_completeness,IS_SOME_EXISTS]) >>
+           rename1 `instance_subst _ _ _ = SOME result` >>
+           Cases_on `result` >>
+           rename1 `SOME(sigma''',stuff'')` >>
+           simp[] >>
+           drule_then assume_tac instance_subst_soundness >>
+           MAP_EVERY qunabbrev_tac [`ty0`,`ty1`] >>
+           qpat_x_assum `Tyapp _ _ = TYPE_SUBST _ _` (assume_tac o GSYM) >>
+           simp[] >>
+           `TYPE_SUBST sigma'³' (domain (typeof pred)) =
+            TYPE_SUBSTf sigma (domain (typeof pred))
+           `
+             by(simp[TYPE_SUBST_eq_TYPE_SUBSTf,TYPE_SUBSTf_eq_TYPE_SUBSTf] >>
+                fs[MAP_EQ_f,MEM_MAP,PULL_EXISTS] >>
+                rpt strip_tac >> first_x_assum match_mp_tac >>
+                rfs[term_ok_clauses] >>
+                fs[welltyped_def] >> qpat_x_assum `pred has_type _` assume_tac >>
+                drule_then assume_tac WELLTYPED_LEMMA >> rveq >>
+                drule_then (match_mp_tac o REWRITE_RULE[SUBSET_DEF]) tyvars_typeof_subset_tvars >>
+                rfs[tyvars_def] >>
+                disch_then drule) >>
+           rw[mem_sub]) >>
+      MAP_EVERY qunabbrev_tac [`vname`,`vty`] >>
+      qmatch_goalsub_abbrev_tac `Abstract a1 a2 a3 ' a4` >>
+      `Abstract a1 a2 a3 ' a4 = a3 a4`
+        by(drule_then match_mp_tac apply_abstract >>
+           MAP_EVERY qunabbrev_tac [`a1`,`a2`,`a3`,`a4`] >>
+           conj_tac >-
+             (qmatch_goalsub_abbrev_tac `Abstract a1 a2 a3 ' a4` >>
+              `Abstract a1 a2 a3 ' a4 = a3 a4`
+                by(drule_then match_mp_tac apply_abstract >>
+                   MAP_EVERY qunabbrev_tac [`a1`,`a2`,`a3`,`a4`] >>
+                   simp[] >> fs[]) >>
+              MAP_EVERY qunabbrev_tac [`a1`,`a2`,`a3`,`a4`] >>
+              pop_assum SUBST_ALL_TAC >>
+              simp[]) >>
+           rw[] >>
+           SELECT_ELIM_TAC >>
+           simp[] >>
+           qhdtm_x_assum `is_frag_interpretation0` mp_tac >>
+           simp[is_frag_interpretation_def,total_fragment_def,is_type_frag_interpretation_def] >>
+           strip_tac >>
+           first_x_assum match_mp_tac >>
+           simp[ground_types_def,tyvars_def,type_ok_def,EVERY_MEM,MEM_MAP,PULL_EXISTS,
+                FLOOKUP_FUNION,FLOOKUP_UPDATE] >>
+           fs[Abbr`tyenv`,GSYM FUNION_ASSOC,FUNION_FUPDATE_1] >>
+           match_mp_tac FOLDR_LIST_UNION_empty >>
+           rw[EVERY_MEM,MEM_MAP,PULL_EXISTS]) >>
+      MAP_EVERY qunabbrev_tac [`a1`,`a2`,`a3`,`a4`] >>
+      simp[] >>
+      qmatch_goalsub_abbrev_tac `Abstract a1 a2 a3 ' a4` >>
+      `Abstract a1 a2 a3 ' a4 = a3 a4`
+        by(drule_then match_mp_tac apply_abstract >>
+           MAP_EVERY qunabbrev_tac [`a1`,`a2`,`a3`,`a4`] >>
+           simp[] >> fs[]) >>
+      MAP_EVERY qunabbrev_tac [`a1`,`a2`,`a3`,`a4`] >>
+      pop_assum SUBST_ALL_TAC >>
+      simp[] >>
+      fs[]) >>
+      (* Second abs/rep axiom *)
+       drule proves_theory_mono >>
+       qmatch_asmsub_abbrev_tac `total_fragment (tyenv,tmenv)` >>
+       disch_then(qspecl_then [`tysof ctxt2`,`tmsof ctxt2`,`axsof ctxt2`,
+                               `tyenv`,`tmenv`] mp_tac) >>
+       simp[] >>
+       MAP_EVERY qunabbrev_tac [`tyenv`,`tmenv`] >>
+       impl_tac >-
+         (rw[] >>
+          TRY(match_mp_tac (CONJUNCT2 SUBMAP_FUNION_ID) >> rw[FDOM_FUPDATE] >>
+              drule_then (assume_tac o C MATCH_MP init_ctxt_extends) extends_trans >>
+              drule extends_NIL_DISJOINT >>
+              simp[] >> NO_TAC) >>
+          qhdtm_x_assum `theory_ok` mp_tac >>
+          rw[theory_ok_def]) >>
+      strip_tac >>
+      drule_then drule (MP_CANON termsem_ext_equation) >>
+      disch_then drule >>
+      fs[valuates_frag_builtins] >>
+      disch_then drule >>
+      drule_then drule terms_of_frag_uninst_equationE >>
+      impl_keep_tac >-
+        (rw[welltyped_equation,EQUATION_HAS_TYPE_BOOL] >>
+         imp_res_tac proves_term_ok >>
+         fs[] >> rfs[term_ok_clauses] >>
+         qpat_x_assum `Comb _ _ has_type Bool` (strip_assume_tac o ONCE_REWRITE_RULE[has_type_cases]) >>
+         fs[] >> rveq >>
+         imp_res_tac WELLTYPED_LEMMA >>
+         rfs[] >> rveq >> fs[] >> rw[equation_def]) >>
+      disch_then (MAP_EVERY assume_tac o rev o CONJUNCTS) >>
+      ntac 2 (disch_then dxrule) >>
+      impl_keep_tac >-
+        (rw[term_ok_clauses] >> rw[term_ok_def] >>
+         qpat_assum `is_std_sig(FUNION _ _,_)` (strip_assume_tac o REWRITE_RULE[is_std_sig_def]) >>
+         rw[type_ok_def,EVERY_MEM,MEM_MAP,FLOOKUP_FUNION,FLOOKUP_UPDATE] >>
+         rw[type_ok_def] >>
+         drule proves_term_ok >>
+         rw[EVERY_MEM,term_ok_def] >> rw[] >>
+         drule_then drule term_ok_type_ok >> rw[] >>
+         fs[] >> rfs[term_ok_clauses] >>
+         qpat_x_assum `Comb _ _ has_type Bool` (strip_assume_tac o ONCE_REWRITE_RULE[has_type_cases]) >>
+         fs[] >> rveq >>
+         imp_res_tac WELLTYPED_LEMMA >>
+         rfs[] >> rveq >> fs[] >> rw[equation_def]
+        ) >>
+      simp[termsem_ext_def] >>
+      disch_then kall_tac >>
+      rw[boolean_eq_true] >>
+      rw[termsem_def] >>
+      drule_then drule terms_of_frag_uninst_equationE >>
+      impl_tac >- rw[welltyped_equation] >>
+      strip_tac >>
+      drule_then dxrule terms_of_frag_uninst_equationE >>
+      impl_tac >- rw[welltyped_equation,EQUATION_HAS_TYPE_BOOL] >>
+      disch_then(MAP_EVERY assume_tac o rev o CONJUNCTS) >>
+      drule_then drule termsem_ext_equation >>
+      disch_then drule >> disch_then drule >>
+      disch_then dxrule >> disch_then dxrule >>
+      impl_keep_tac >-
+        (rw[term_ok_clauses] >> rw[term_ok_def] >>
+         qpat_assum `is_std_sig(FUNION _ _,_)` (strip_assume_tac o REWRITE_RULE[is_std_sig_def]) >>
+         rw[type_ok_def,EVERY_MEM,MEM_MAP,FLOOKUP_FUNION,FLOOKUP_UPDATE] >>
+         rw[type_ok_def] >>
+         drule proves_term_ok >>
+         rw[EVERY_MEM,term_ok_def] >> rw[] >>
+         drule_then drule term_ok_type_ok >> rw[] >>
+         fs[] >> rfs[term_ok_clauses] >>
+         qpat_x_assum `Comb _ _ has_type Bool` (strip_assume_tac o ONCE_REWRITE_RULE[has_type_cases]) >>
+         fs[] >> rveq >>
+         imp_res_tac WELLTYPED_LEMMA >>
+         rfs[] >> rveq >> fs[] >> rw[equation_def]) >>
+      simp[termsem_ext_def] >>
+      disch_then kall_tac >>
+      rw[boolean_eq_true] >>
+      rw[termsem_def] >>
+      `~MEM (strlit "=") (MAP FST (const_list ctxt1))`
+        by(drule_then strip_assume_tac extends_appends >>
+           fs[APPEND_EQ_APPEND,init_ctxt_def] >>
+           rveq >> fs[] >>
+           fs[APPEND_EQ_CONS |> CONV_RULE(LHS_CONV SYM_CONV)] >>
+           rveq >> fs[] >>
+           drule_then(assume_tac o C MATCH_MP (REWRITE_RULE[init_ctxt_def] init_ctxt_extends))
+                     extends_trans >>
+           drule extends_NIL_DISJOINT >>
+           rw[]) >>
+      `MEM (strlit "=") (MAP FST (const_list ctxt2))`
+        by(imp_res_tac extends_appends >> rw[init_ctxt_def]) >>
+      `abs <> strlit "="` by(CCONTR_TAC >> fs[]) >>
+      `rep <> strlit "="` by(CCONTR_TAC >> fs[]) >>
+      simp[ext_term_frag_builtins_def] >>
+       qmatch_asmsub_abbrev_tac `total_fragment (tyenv,tmenv)` >>
+      `models (type_interpretation_of ind (ctxt1 ++ TypeDefn name pred abs rep::ctxt2))
+              (UNCURRY (term_interpretation_of ind (ctxt1 ++ TypeDefn name pred abs rep::ctxt2)))
+              ((tyenv,tmenv),axsof ctxt2)`
+        by(rw[models_def]) >>
+      drule_then drule proves_sound >>
+      simp[entails_def] >>
+      strip_tac >>
+      first_x_assum drule >>
+      simp[satisfies_t_def] >>
+      ntac 2 (disch_then drule) >>
+      impl_keep_tac >-
+        (rw[ground_terms_uninst_def] >>
+         goal_assum drule >>
+         rw[ground_types_def,tyvars_def] >>
+         imp_res_tac term_ok_type_ok >>
+         qpat_x_assum `is_std_sig (tyenv,tmenv)` mp_tac >>
+         rw[is_std_sig_def,type_ok_def]) >>
+      simp[satisfies_def] >>
+      simp[valuates_frag_builtins] >>
+      disch_then drule >>
+      impl_tac >-
+        (match_mp_tac terms_of_frag_uninst_term_ok >> simp[]) >>
+      simp[termsem_def] >> strip_tac >>
+      `termsem
+           (ext_type_frag_builtins
+              (type_interpretation_of ind (ctxt1 ++ TypeDefn name pred abs rep::ctxt2)))
+           (ext_term_frag_builtins
+              (ext_type_frag_builtins
+                 (type_interpretation_of ind (ctxt1 ++ TypeDefn name pred abs rep::ctxt2)))
+              (UNCURRY
+                 (term_interpretation_of ind (ctxt1 ++ TypeDefn name pred abs rep::ctxt2))))
+           v sigma witness ⋲
+         (ext_type_frag_builtins
+              (type_interpretation_of ind (ctxt1 ++ TypeDefn name pred abs rep::ctxt2)))
+           (TYPE_SUBSTf sigma (typeof witness))
+      `
+        by(match_mp_tac termsem_in_type_ext2 >>
+           rpt(goal_assum drule) >>
+           conj_tac >-
+             (match_mp_tac terms_of_frag_uninst_term_ok >>
+              simp[] >>
+              drule proves_term_ok >>
+              rw[EVERY_MEM,MEM_MAP,term_ok_def]) >>
+           rpt strip_tac >>
+           qpat_x_assum `valuates_frag _ _ _ _` mp_tac >>
+           simp[valuates_frag_def] >>
+           disch_then match_mp_tac >>
+           match_mp_tac TYPE_SUBSTf_in_types_of_frag_I >>
+           goal_assum drule >>
+           goal_assum drule >>
+           match_mp_tac terms_of_frag_uninst_term_ok >>
+           simp[] >>
+           drule proves_term_ok >> rw[EVERY_MEM,MEM_MAP,term_ok_def]) >>
+      qmatch_goalsub_abbrev_tac `term_interpretation_of ind _ abs abstype` >>
+      qmatch_goalsub_abbrev_tac `term_interpretation_of ind _ rep reptype` >>
+      `(abs,abstype) ∈ ground_consts (sigof(ctxt1 ++ TypeDefn name pred abs rep::ctxt2))`
+        by(fs[Abbr `abstype`,ground_consts_def,ground_types_def] >>
+           conj_tac >-
+             (simp[tyvars_def,LIST_UNION_EQ_NIL,tyvars_TYPE_SUBSTf_eq_NIL] >>
+              match_mp_tac FOLDR_LIST_UNION_empty >>
+              rw[EVERY_MEM,MEM_MAP,PULL_EXISTS]) >>
+           conj_asm1_tac >-
+             (qmatch_goalsub_abbrev_tac `type_ok tyenv'` >>
+              `tyenv' = tysof(tyenv,tmenv)`
+                by(fs[Abbr `tyenv`,Abbr `tmenv`,Abbr`tyenv'`] >>
+                   fs[GSYM FUNION_ASSOC,FUNION_FUPDATE_1]) >>
+              pop_assum SUBST_ALL_TAC >>
+              simp[term_ok_clauses] >>
+              conj_tac >-
+                (match_mp_tac type_ok_TYPE_SUBSTf >> simp[] >>
+                 qpat_x_assum `term_ok _ (Comb _ _)` mp_tac >>
+                 simp[term_ok_clauses] >>
+                 rpt strip_tac >>
+                 simp[] >> metis_tac[term_ok_type_ok,FST]) >>
+              simp[type_ok_def,EVERY_MAP,MEM_MAP,PULL_EXISTS] >>
+              rw[Abbr `tyenv`,FLOOKUP_FUNION,FLOOKUP_UPDATE]) >>
+           rw[term_ok_def,FLOOKUP_FUNION,FLOOKUP_UPDATE] >>
+           qexists_tac `(MAP (λx. (sigma x,Tyvar x)) (tvars pred))` >>
+           simp[TYPE_SUBST_eq_TYPE_SUBSTf,MAP_EQ_f,MEM_MAP,PULL_EXISTS,
+                REV_ASSOCD_ALOOKUP,MAP_MAP_o,o_DEF,ALOOKUP_Tyvar,ALOOKUP_MAPf] >>
+           simp[TYPE_SUBSTf_eq_TYPE_SUBSTf] >>
+           rfs[term_ok_clauses] >>
+           rpt strip_tac >>
+           IF_CASES_TAC >> simp[] >>
+           fs[welltyped_def] >> qpat_x_assum `pred has_type _` assume_tac >>
+           drule_then assume_tac WELLTYPED_LEMMA >> rveq >>
+           drule_then (mp_tac o REWRITE_RULE[SUBSET_DEF,Once MONO_NOT_EQ]) tyvars_typeof_subset_tvars >>
+           disch_then drule >>
+           simp[tyvars_def]) >>
+      `(abs,abstype) ∈ nonbuiltin_constinsts`
+        by simp[nonbuiltin_constinsts_def,builtin_consts_def] >>
+      `(rep,reptype) ∈ ground_consts (sigof(ctxt1 ++ TypeDefn name pred abs rep::ctxt2))`
+        by(qpat_x_assum `(abs,abstype) ∈ ground_consts _` mp_tac >>
+           fs[Abbr `reptype`,Abbr `abstype`,ground_consts_def,ground_types_def] >>
+           qmatch_goalsub_abbrev_tac `type_ok tyenv'` >>
+           `tyenv' = tysof(tyenv,tmenv)`
+                by(fs[Abbr `tyenv`,Abbr `tmenv`,Abbr`tyenv'`] >>
+                   fs[GSYM FUNION_ASSOC,FUNION_FUPDATE_1]) >>
+           pop_assum SUBST_ALL_TAC >>
+           simp[term_ok_clauses] >>
+           simp[tyvars_def,LIST_UNION_EQ_NIL] >>
+           rw[term_ok_def,term_ok_clauses,FLOOKUP_FUNION,FLOOKUP_UPDATE,MAP_EQ_f] >>
+           fs[type_ok_def] >>
+           metis_tac[]) >>
+      `(rep,reptype) ∈ nonbuiltin_constinsts`
+        by simp[nonbuiltin_constinsts_def,builtin_consts_def] >>
+      `is_frag_interpretation (total_fragment (sigof (ctxt1 ++ TypeDefn name pred abs rep::ctxt2)))
+          (type_interpretation_of ind
+             (ctxt1 ++ TypeDefn name pred abs rep::ctxt2))
+          (UNCURRY
+             (term_interpretation_of ind
+                (ctxt1 ++ TypeDefn name pred abs rep::ctxt2)))`
+        by(qhdtm_x_assum `is_frag_interpretation0` mp_tac >>
+           simp[Abbr `tyenv`,Abbr `tmenv`,GSYM FUNION_ASSOC,FUNION_FUPDATE_1]) >>
+      MAP_EVERY qunabbrev_tac [`abstype`,`reptype`] >>
+      Q.SUBGOAL_THEN `inhabited ind` assume_tac >- metis_tac[] >>
+      simp[type_interpretation_of_alt] >>
+      qpat_x_assum `inhabited ind` kall_tac >>
+      simp[FILTER_APPEND] >>
+      IF_CASES_TAC >- fs[defn_matches_def] >>
+      Cases_on `[] ≠
+                 defn_matches abs
+                   (Fun (TYPE_SUBSTf sigma (domain (typeof pred)))
+                      (Tyapp name
+                         (MAP (λa. TYPE_SUBSTf sigma a)
+                            (MAP Tyvar
+                               (MAP implode
+                                  (STRING_SORT (MAP explode (tvars pred))))))))
+                   (TypeDefn name pred abs rep)` >-
+        fs[defn_matches_def] >>
+      simp[] >>
+      ntac 2 (pop_assum kall_tac) >>
+      ntac 2 (
+        qmatch_goalsub_abbrev_tac `FILTER ff ll` >>
+        `FILTER ff ll = []`
+          by(simp[Abbr `ff`,Abbr `ll`,FILTER_EQ_NIL,EVERY_MEM,MEM_MAP,PULL_EXISTS,
+                  defn_matches_def] >> rpt strip_tac >>
+             TOP_CASE_TAC >> simp[] >>
+             simp[FILTER_EQ_NIL,EVERY_MEM,MEM_MAP,PULL_EXISTS] >>
+             Cases >> simp[] >> strip_tac >>
+             simp[RIGHT_FORALL_OR_THM] >> disj1_tac >>
+             qpat_x_assum `MEM (ConstSpec _ _ _) _` (strip_assume_tac o REWRITE_RULE[MEM_SPLIT]) >>
+             rveq >>
+             drule_then (assume_tac o C MATCH_MP init_ctxt_extends) extends_trans >>
+             FULL_SIMP_TAC bool_ss [GSYM APPEND_ASSOC] >>
+             dxrule_then assume_tac extends_APPEND_NIL >>
+             fs[] >>
+             dxrule_then assume_tac extends_NIL_CONS_updates >>
+             Cases_on `b` >>
+             fs[updates_cases,constspec_ok_def]
+             >- (pop_assum(drule_then strip_assume_tac) >>
+                 qpat_x_assum `MEM (NewConst _ _) _` (strip_assume_tac o REWRITE_RULE[MEM_SPLIT]) >>
+                 fs[]) >>
+             qpat_x_assum `MEM (_,_) l` (strip_assume_tac o REWRITE_RULE[MEM_SPLIT]) >>
+             fs[]) >>
+        pop_assum SUBST_ALL_TAC >>
+        MAP_EVERY qunabbrev_tac [`ff`,`ll`] >>
+        qmatch_goalsub_abbrev_tac `FILTER ff ll` >>
+        `FILTER ff ll = []`
+          by(simp[Abbr `ff`,Abbr `ll`,FILTER_EQ_NIL,EVERY_MEM,MEM_MAP,PULL_EXISTS,
+                  defn_matches_def] >> rpt strip_tac >>
+             TOP_CASE_TAC >> simp[] >>
+             simp[FILTER_EQ_NIL,EVERY_MEM,MEM_MAP,PULL_EXISTS] >>
+             Cases >> simp[] >> strip_tac >>
+             simp[RIGHT_FORALL_OR_THM] >> disj1_tac >>
+             qpat_x_assum `MEM (ConstSpec _ _ _) _` (strip_assume_tac o REWRITE_RULE[MEM_SPLIT]) >>
+             rveq >>
+             drule_then (assume_tac o C MATCH_MP init_ctxt_extends) extends_trans >>
+             dxrule_then assume_tac extends_APPEND_NIL >>
+             dxrule_then assume_tac (extends_APPEND_NIL |> Q.SPEC `[e]` |> REWRITE_RULE[APPEND]) >>
+             dxrule_then assume_tac extends_APPEND_NIL >>
+             dxrule_then assume_tac extends_NIL_CONS_updates >>
+             Cases_on `b` >>
+             fs[updates_cases,constspec_ok_def]
+             >- (pop_assum(drule_then strip_assume_tac) >>
+                 qpat_x_assum `MEM (NewConst _ _) _` (strip_assume_tac o REWRITE_RULE[MEM_SPLIT]) >>
+                 fs[])
+             >- (pop_assum(drule_then strip_assume_tac) >>
+                 qpat_x_assum `MEM (NewConst _ _) _` (strip_assume_tac o REWRITE_RULE[MEM_SPLIT]) >>
+                 fs[]) >>
+             qpat_x_assum `MEM (_,_) l` (strip_assume_tac o REWRITE_RULE[MEM_SPLIT]) >>
+             fs[]) >>
+        pop_assum SUBST_ALL_TAC >>
+        MAP_EVERY qunabbrev_tac [`ff`,`ll`]) >>
+      simp[] >>
+      simp[mllistTheory.mapPartial_def,mapPartial_APPEND] >>
+      rpt
+        (qmatch_goalsub_abbrev_tac `mapPartial a1 a2` >>
+        `mapPartial a1 a2 = []`
+          by(rw[Abbr `a1`,Abbr `a2`,mllistTheory.mapPartial_thm,FILTER_EQ_NIL,EVERY_MEM,MEM_MAP,
+                PULL_EXISTS] >>
+             simp[abs_or_rep_matches_def,abs_matches_def,rep_matches_def] >>
+             ntac 3 (PURE_TOP_CASE_TAC >> fs[] >> rveq) >>
+             fs[pair_case_eq] >>
+             PURE_FULL_CASE_TAC >> fs[] >> rveq >>
+             qpat_x_assum `MEM (TypeDefn _ _ _ _) _` (strip_assume_tac o REWRITE_RULE[MEM_SPLIT]) >>
+             rveq >>
+             drule_then (assume_tac o C MATCH_MP init_ctxt_extends) extends_trans >>
+             dxrule_then assume_tac extends_APPEND_NIL >>
+             dxrule_then assume_tac extends_NIL_CONS_updates >>
+             fs[updates_cases]) >>
+        pop_assum SUBST_ALL_TAC >>
+        MAP_EVERY qunabbrev_tac [`a1`,`a2`]) >>
+      simp[abs_or_rep_matches_def,abs_matches_def,rep_matches_def] >>
+      reverse IF_CASES_TAC >-
+        (goal_assum kall_tac >>
+         pop_assum mp_tac >> pop_assum kall_tac >> simp[] >>
+         simp[TYPE_SUBSTf_eq_TYPE_SUBST] >>
+         rw[MAP_EQ_f,MEM_MAP,PULL_EXISTS] >>
+         qexists_tac `MAP (λx. (sigma x,Tyvar x)) (tvars pred)` >>
+         reverse conj_tac >-
+           (rw[TYPE_SUBST_tyvars,REV_ASSOCD_ALOOKUP] >>
+            ntac 2 TOP_CASE_TAC >>
+            fs[ALOOKUP_NONE,MEM_MAP,GSYM IMP_DISJ_THM,PULL_FORALL] >>
+            imp_res_tac ALOOKUP_MEM >>
+            fs[MEM_MAP] >> rveq >> pairarg_tac >> rveq >> fs[] >>
+            rveq >> fs[] >> rveq >> fs[] >>
+            rfs[term_ok_def] >> rfs[] >> fs[welltyped_def] >>
+            imp_res_tac WELLTYPED_LEMMA >> rveq >>
+            `MEM x (tyvars(typeof pred))` by simp[tyvars_def] >>
+            drule_then drule (tyvars_typeof_subset_tvars |> REWRITE_RULE[SUBSET_DEF] |> MP_CANON) >>
+            simp[]) >>
+         strip_tac >>
+         simp[REV_ASSOCD_ALOOKUP,ALOOKUP_MAP,MAP_MAP_o,o_DEF,tyvars_def] >>
+         simp[ALOOKUP_Tyvar,ALOOKUP_MAPf]) >>
+      simp[] >>
+      reverse IF_CASES_TAC >-
+        (goal_assum kall_tac >>
+         pop_assum mp_tac >> simp[] >>
+         fs[] >>
+         metis_tac[]) >>
+      CONV_TAC(SIMP_CONV (srw_ss())[]) >>
+      qmatch_goalsub_abbrev_tac `instance_subst [(ty0,ty1)]` >>
+      Q.SUBGOAL_THEN `is_instance ty1 ty0` mp_tac >-
+        (fs[Abbr `ty0`,Abbr`ty1`] >> metis_tac[]) >>
+      disch_then (strip_assume_tac o REWRITE_RULE[instance_subst_completeness,IS_SOME_EXISTS]) >>
+      rename1 `instance_subst _ _ _ = SOME result` >>
+      Cases_on `result` >>
+      rename1 `SOME(sigma',stuff)` >>
+      simp[] >>
+      drule_then assume_tac instance_subst_soundness >>
+      MAP_EVERY qunabbrev_tac [`ty0`,`ty1`] >>
+      qmatch_goalsub_abbrev_tac `instance_subst [ty0,ty1]` >>
+      Q.SUBGOAL_THEN `is_instance ty1 ty0` mp_tac >-
+        (fs[Abbr `ty0`,Abbr`ty1`] >> metis_tac[]) >>
+      disch_then (strip_assume_tac o REWRITE_RULE[instance_subst_completeness,IS_SOME_EXISTS]) >>
+      rename1 `instance_subst _ _ _ = SOME result` >>
+      Cases_on `result` >>
+      rename1 `SOME(sigma'',stuff')` >>
+      simp[] >>
+      drule_then assume_tac instance_subst_soundness >>
+      MAP_EVERY qunabbrev_tac [`ty0`,`ty1`] >>
+      ntac 2 (PRED_ASSUM is_exists kall_tac) >>
+      rpt(qpat_x_assum `Fun _ _ = TYPE_SUBST _ _` (mp_tac o GSYM)) >>
+      rw[] >> fs[MAP_EQ_f,MEM_MAP,PULL_EXISTS] >>
+      qmatch_goalsub_abbrev_tac `ext_type_frag_builtins _ (Tyapp name ntys)` >>
+      `Tyapp name ntys ∈ nonbuiltin_types`
+        by(simp[Abbr`ntys`] >>
+           drule_then strip_assume_tac extends_appends >>
+           fs[APPEND_EQ_APPEND,init_ctxt_def,
+              APPEND_EQ_CONS |> CONV_RULE(LHS_CONV SYM_CONV)] >>
+           rveq >> fs[] >>
+           last_assum(qspec_then `(name,0)` mp_tac) >>
+           last_x_assum(qspec_then `(name,2)` mp_tac) >>
+           simp[] >>
+           rw[nonbuiltin_types_def,is_builtin_type_def]) >>
+      qunabbrev_tac `ntys` >>
+      simp[ext_type_frag_builtins_nonbuiltin] >>
+      qmatch_goalsub_abbrev_tac `v (vname,vty)` >>
+      `v (vname,vty) ⋲ ext_type_frag_builtins (type_interpretation_of ind (ctxt1 ++ TypeDefn name pred abs rep::ctxt2)) (TYPE_SUBSTf sigma vty)`
+        by(qhdtm_x_assum `valuates_frag0` mp_tac >>
+           simp[valuates_frag_def] >>
+           disch_then(qspecl_then [`vname`,`vty`] mp_tac) >>
+           simp[Abbr `vty`,ext_type_frag_builtins_nonbuiltin] >>
+           disch_then match_mp_tac >>
+           drule_then drule terms_of_frag_uninst_equationE >>
+           impl_tac >- simp[welltyped_equation] >>
+           strip_tac >>
+           PURE_REWRITE_TAC[GSYM TYPE_SUBSTf_def] >>
+           match_mp_tac TYPE_SUBSTf_in_types_of_frag_I >>
+           Q.REFINE_EXISTS_TAC `Var _ _` >>
+           simp[] >>
+           drule_then drule terms_of_frag_uninst_equationE >>
+           impl_tac >- rw[welltyped_equation,EQUATION_HAS_TYPE_BOOL] >>
+           strip_tac >>
+           metis_tac[]) >>
+      `TYPE_SUBSTf sigma vty ∈ ground_types (sigof (ctxt1 ++ TypeDefn name pred abs rep::ctxt2))`
+        by(qunabbrev_tac `vty` >>
+           simp[ground_types_def,tyvars_def,type_ok_def,EVERY_MEM,MEM_MAP,PULL_EXISTS,
+                FLOOKUP_FUNION,FLOOKUP_UPDATE] >>
+           fs[Abbr`tyenv`,GSYM FUNION_ASSOC,FUNION_FUPDATE_1] >>
+           simp[tyvars_TYPE_SUBSTf_eq_NIL] >>
+           match_mp_tac type_ok_TYPE_SUBSTf >>
+           simp[] >>
+           rfs[term_ok_clauses]) >>
+      qmatch_goalsub_abbrev_tac `Abstract (type_interpretation_of ind ctxt vty')` >>
+      `vty' ∈ ground_types (sigof ctxt)`
+        by(qunabbrev_tac `vty'` >> qunabbrev_tac `ctxt` >>
+           simp[ground_types_def,tyvars_def,type_ok_def,EVERY_MEM,MEM_MAP,PULL_EXISTS,
+                FLOOKUP_FUNION,FLOOKUP_UPDATE] >>
+           fs[Abbr`tyenv`,GSYM FUNION_ASSOC,FUNION_FUPDATE_1] >>
+           match_mp_tac FOLDR_LIST_UNION_empty >>
+           rw[EVERY_MEM,MEM_MAP,PULL_EXISTS]) >>
+      `type_interpretation_of ind ctxt vty'
+       =
+       (ext_type_frag_builtins (type_interpretation_of ind ctxt)
+         (TYPE_SUBSTf sigma vty) suchthat
+        (λtm. termsem
+          (ext_type_frag_builtins (type_interpretation_of ind ctxt))
+          (ext_term_frag_builtins (ext_type_frag_builtins (type_interpretation_of ind ctxt))
+                                 (UNCURRY (term_interpretation_of ind ctxt))) v sigma
+          pred ' tm = True))`
+        by(`is_frag_interpretation (total_fragment(sigof ctxt)) (type_interpretation_of ind ctxt)
+                                   (UNCURRY (term_interpretation_of ind ctxt))`
+             by(simp[Abbr`ctxt`]) >>
+           Q.SUBGOAL_THEN `inhabited ind` assume_tac >- metis_tac[] >>
+           simp[type_interpretation_of_alt] >>
+           qpat_x_assum `inhabited ind` kall_tac >>
+           fs[Abbr `vty`,Abbr `vty'`,Abbr `ctxt`] >>
+           simp[mllistTheory.mapPartial_thm,FILTER_APPEND] >>
+           qmatch_goalsub_abbrev_tac `FILTER IS_SOME (MAP f1 c1)` >>
+           `FILTER IS_SOME (MAP f1 c1) = []`
+             by(fs[Abbr `f1`,Abbr `c1`,FILTER_EQ_NIL,EVERY_MEM,MEM_MAP,PULL_EXISTS] >>
+                strip_tac >>
+                simp[type_matches_def] >>
+                TOP_CASE_TAC >> fs[] >>
+                strip_tac >>
+                pop_assum(strip_assume_tac o REWRITE_RULE[MEM_SPLIT]) >>
+                fs[] >> metis_tac[FST,SND]) >>
+           MAP_EVERY qunabbrev_tac [`f1`,`c1`] >>
+           simp[] >>
+           qmatch_goalsub_abbrev_tac `FILTER IS_SOME (MAP f1 c1)` >>
+           `FILTER IS_SOME (MAP f1 c1) = []`
+             by(fs[Abbr `f1`,Abbr `c1`,FILTER_EQ_NIL,EVERY_MEM,MEM_MAP,PULL_EXISTS] >>
+                strip_tac >>
+                simp[type_matches_def] >>
+                TOP_CASE_TAC >> fs[] >>
+                strip_tac >>
+                pop_assum(strip_assume_tac o REWRITE_RULE[MEM_SPLIT]) >>
+                fs[] >> metis_tac[FST,SND]) >>
+           MAP_EVERY qunabbrev_tac [`f1`,`c1`] >>
+           simp[] >>
+           simp[type_matches_def] >>
+           qmatch_goalsub_abbrev_tac `if predd then SOME _ else NONE` >>
+           Q.SUBGOAL_THEN `predd` assume_tac >-
+             (qunabbrev_tac `predd` >>
+              simp[MAP_EQ_f,MEM_MAP,PULL_EXISTS,REV_ASSOCD_ALOOKUP] >>
+              qexists_tac `MAP (λx. (sigma x, Tyvar x)) (tvars pred)` >>
+              simp[ALOOKUP_Tyvar,MAP_MAP_o,o_DEF,ALOOKUP_MAPf]) >>
+           qunabbrev_tac `predd` >>
+           simp[] >>
+           qmatch_goalsub_abbrev_tac `instance_subst [(ty0,ty1)]` >>
+           Q.SUBGOAL_THEN `is_instance ty1 ty0` mp_tac >-
+             (fs[Abbr `ty0`,Abbr`ty1`] >> metis_tac[]) >>
+           disch_then (strip_assume_tac o REWRITE_RULE[instance_subst_completeness,IS_SOME_EXISTS]) >>
+           rename1 `instance_subst _ _ _ = SOME result` >>
+           Cases_on `result` >>
+           rename1 `SOME(sigma''',stuff'')` >>
+           simp[] >>
+           drule_then assume_tac instance_subst_soundness >>
+           MAP_EVERY qunabbrev_tac [`ty0`,`ty1`] >>
+           qpat_x_assum `Tyapp _ _ = TYPE_SUBST _ _` (assume_tac o GSYM) >>
+           simp[] >>
+           `TYPE_SUBST sigma'³' (domain (typeof pred)) =
+            TYPE_SUBSTf sigma (domain (typeof pred))
+           `
+             by(simp[TYPE_SUBST_eq_TYPE_SUBSTf,TYPE_SUBSTf_eq_TYPE_SUBSTf] >>
+                fs[MAP_EQ_f,MEM_MAP,PULL_EXISTS] >>
+                rpt strip_tac >> first_x_assum match_mp_tac >>
+                rfs[term_ok_clauses] >>
+                fs[welltyped_def] >> qpat_x_assum `pred has_type _` assume_tac >>
+                drule_then assume_tac WELLTYPED_LEMMA >> rveq >>
+                drule_then (match_mp_tac o REWRITE_RULE[SUBSET_DEF]) tyvars_typeof_subset_tvars >>
+                rfs[tyvars_def] >>
+                disch_then drule) >>
+           simp[] >>
+           simp[mem_sub] >>
+           simp[ELIM_UNCURRY] >>
+           qmatch_goalsub_abbrev_tac `termsem a1 a2 a3 a4` >>
+           `termsem a1 a2 a3 a4 pred =
+            termsem a1 a2 v a4 pred`
+             by(match_mp_tac(GEN_ALL termsem_frees) >>
+                fs[CLOSED_def] >>
+                rfs[term_ok_clauses]) >>
+           pop_assum SUBST_ALL_TAC >>
+           `termsem a1 a2 v a4 pred =
+            termsem a1 a2 v sigma pred`
+             by(MAP_EVERY qunabbrev_tac [`a1`,`a2`,`a3`,`a4`] >>
+                match_mp_tac termsem_subst >>
+                rfs[term_ok_clauses] >>
+                fs[MAP_EQ_f,MEM_MAP,PULL_EXISTS]) >>
+           pop_assum SUBST_ALL_TAC >>
+           MAP_EVERY qunabbrev_tac [`a1`,`a2`,`a3`,`a4`] >>
+           reverse IF_CASES_TAC
+           >- (goal_assum kall_tac >>
+               pop_assum mp_tac >> simp[] >>
+               fs[ELIM_UNCURRY] >>
+               rfs[term_ok_clauses] >> metis_tac[]) >>
+           pop_assum kall_tac >>
+           rw[]) >>
+      MAP_EVERY qunabbrev_tac [`vname`,`vty`] >>
+      MAP_EVERY qunabbrev_tac [`ctxt`,`vty'`] >>
+      qmatch_goalsub_abbrev_tac `Abstract a1 a2 a3 ' a4` >>
+      `Abstract a1 a2 a3 ' a4 = a3 a4`
+        by(drule_then match_mp_tac apply_abstract >>
+           MAP_EVERY qunabbrev_tac [`a1`,`a2`,`a3`,`a4`] >>
+           conj_tac >-
+             (qmatch_goalsub_abbrev_tac `Abstract a1 a2 a3 ' a4` >>
+              `Abstract a1 a2 a3 ' a4 = a3 a4`
+                by(drule_then match_mp_tac apply_abstract >>
+                   MAP_EVERY qunabbrev_tac [`a1`,`a2`,`a3`,`a4`] >>
+                   simp[] >> rw[] >>
+                   SELECT_ELIM_TAC >>
+                   simp[] >>
+                   simp[mem_sub] >>
+                   rfs[term_ok_clauses] >>
+                   metis_tac[]) >>
+              MAP_EVERY qunabbrev_tac [`a1`,`a2`,`a3`,`a4`] >>
+              simp[] >>
+              rw[] >>
+              SELECT_ELIM_TAC >>
+              simp[] >>
+              simp[mem_sub] >>
+              rfs[term_ok_clauses] >>
+              metis_tac[]) >>
+           simp[] >>
+           qmatch_goalsub_abbrev_tac `Abstract a1 a2 a3 ' a4` >>
+           `Abstract a1 a2 a3 ' a4 = a3 a4`
+             by(drule_then match_mp_tac apply_abstract >>
+                MAP_EVERY qunabbrev_tac [`a1`,`a2`,`a3`,`a4`] >>
+                simp[] >>
+                rw[] >>
+                SELECT_ELIM_TAC >> simp[] >>
+                simp[mem_sub] >>
+                rfs[term_ok_clauses] >>
+                metis_tac[]) >>
+           MAP_EVERY qunabbrev_tac [`a1`,`a2`,`a3`,`a4`] >>
+           simp[] >>
+           rw[] >>
+           SELECT_ELIM_TAC >> simp[] >>
+           simp[mem_sub] >>
+           rfs[term_ok_clauses] >>
+           metis_tac[]) >>
+      MAP_EVERY qunabbrev_tac [`a1`,`a2`,`a3`,`a4`] >>
+      simp[] >>
+      qmatch_goalsub_abbrev_tac `Abstract a1 a2 a3 ' a4` >>
+      `Abstract a1 a2 a3 ' a4 = a3 a4`
+        by(drule_then match_mp_tac apply_abstract >>
+           MAP_EVERY qunabbrev_tac [`a1`,`a2`,`a3`,`a4`] >>
+           conj_tac >- simp[] >>
+           simp[] >>
+           rw[] >>
+           SELECT_ELIM_TAC >>
+           simp[] >>
+           simp[mem_sub] >>
+           rfs[term_ok_clauses] >>
+           metis_tac[]) >>
+      MAP_EVERY qunabbrev_tac [`a1`,`a2`,`a3`,`a4`] >>
+      simp[] >>
+      IF_CASES_TAC >- rfs[mem_sub,boolean_def] >>
+      rfs[mem_sub] >>
+      SELECT_ELIM_TAC >>
+      conj_tac >- (rfs[term_ok_clauses] >> metis_tac[]) >>
+      rpt strip_tac >>
+      `x <> v («r» ,domain (typeof pred))` by
+        (spose_not_then strip_assume_tac >>
+         rveq >> fs[]) >>
+      simp[boolean_def] >>
+      qmatch_goalsub_abbrev_tac `a1 ' a2 = False` >>
+      `a1 ' a2 ⋲ boolset`
+        by(MAP_EVERY qunabbrev_tac [`a1`,`a2`] >>
+           drule_then match_mp_tac apply_in_rng >>
+           goal_assum drule >>
+           qmatch_goalsub_abbrev_tac `_ ⋲ a1` >>
+           `a1 = ext_type_frag_builtins
+                   (type_interpretation_of ind
+                      (ctxt1 ++ TypeDefn name pred abs rep::ctxt2))
+                   (TYPE_SUBSTf sigma(typeof pred))`
+             by(rfs[Abbr `a1`,term_ok_clauses] >>
+                simp[ext_type_frag_builtins_Fun] >>
+                qpat_x_assum `Comb pred witness has_type Bool` (strip_assume_tac o REWRITE_RULE[Once has_type_cases]) >>
+                pop_assum mp_tac >> simp[] >>
+                pop_assum mp_tac >> simp[] >>
+                pop_assum mp_tac >> simp[] >>
+                strip_tac >> rveq >>
+                ntac 2 strip_tac >>
+                ntac 2(dxrule WELLTYPED_LEMMA) >>
+                ntac 2 strip_tac >>
+                rveq >>
+                rfs[] >>
+                CONV_TAC(RHS_CONV(RAND_CONV(PURE_ONCE_REWRITE_CONV[ext_type_frag_builtins_def]))) >>
+                simp[]) >>
+           simp[] >>
+           match_mp_tac termsem_in_type_ext2 >>
+           simp[] >>
+           goal_assum drule >>
+           simp[] >>
+           fs[CLOSED_def] >>
+           qpat_x_assum `Comb pred _ ∈ terms_of_frag_uninst _ _` assume_tac >>
+           drule_then drule terms_of_frag_uninst_combE >>
+           rw[]) >>
+      metis_tac[mem_boolset,true_neq_false])
+  *)
+QED
+
+Theorem interpretation_is_model:
+  is_set_theory ^mem ⇒
+    ∀upd ctxt Δ Γ. ctxt extends init_ctxt ∧ inhabited ind ∧ upd updates ctxt
+            ∧ (axioms_admissible mem ind (upd::ctxt))
+            ∧ (models Δ Γ (thyof ctxt))
+    ⇒
+        models (type_interpretation_ext_of ind upd ctxt Δ Γ) (UNCURRY (term_interpretation_ext_of ind upd ctxt Δ Γ))
+               (thyof ((upd::ctxt)))
+Proof
+  rpt strip_tac >>
+  ‘upd::ctxt extends init_ctxt’ by(fs[extends_def] >> rw[Once RTC_CASES1]) >>
+  drule_then (assume_tac o MATCH_MP extends_nil_orth o C MATCH_MP init_ctxt_extends) extends_trans >>
+  imp_res_tac extends_init_ctxt_terminating >>
+  ‘ctxt extends []’ by(drule_then match_mp_tac extends_trans >> simp[init_ctxt_extends]) >>
+  SIMP_TAC std_ss [models_def] >>
+  conj_asm1_tac >-
+   (drule_then match_mp_tac interpretation_is_total_frag_interpretation >>
+    fs[models_def] >>
+    metis_tac[]) >>
+  rw[] >>
+  qpat_x_assum `_ extends init_ctxt` assume_tac >>
+  `!ctxt2. ctxt2 extends init_ctxt ==>
+    !ctxt1 p.
+    orth_ctxt (ctxt1 ++ ctxt2) /\
+    terminating (subst_clos (dependency (ctxt1 ++ ctxt2))) /\
+    (axioms_admissible mem ind (ctxt1 ++ ctxt2)) /\ inhabited ind /\
+    is_frag_interpretation (total_fragment (sigof (ctxt1 ++ ctxt2)))
+      (type_interpretation_ext_of ind (HD(ctxt1 ++ ctxt2)) (TL(ctxt1 ++ ctxt2)) Δ Γ)
+      (UNCURRY (term_interpretation_ext_of ind (HD(ctxt1 ++ ctxt2)) (TL(ctxt1 ++ ctxt2)) Δ Γ)) /\
+    MEM p (axiom_list ctxt2) /\ models Δ Γ (thyof (TL (ctxt1 ++ ctxt2))) ∧
+    ctxt1 ++ ctxt2 extends init_ctxt ==>
+    satisfies_t (sigof (ctxt1 ++ ctxt2))
+      (ext_type_frag_builtins (type_interpretation_ext_of ind (HD(ctxt1 ++ ctxt2)) (TL(ctxt1 ++ ctxt2)) Δ Γ))
+      (ext_term_frag_builtins
+         (ext_type_frag_builtins (type_interpretation_ext_of ind (HD(ctxt1 ++ ctxt2)) (TL(ctxt1 ++ ctxt2)) Δ Γ))
+         (UNCURRY (term_interpretation_ext_of ind (HD(ctxt1 ++ ctxt2)) (TL(ctxt1 ++ ctxt2)) Δ Γ))) ([],p)`
+    by(qhdtm_x_assum `is_set_theory` (fn thm => rpt(pop_assum kall_tac) >> assume_tac thm) >>
+       ntac 2 strip_tac >>
+       drule_then ho_match_mp_tac extends_init_ind >>
+       rpt strip_tac
+       >- ((* init ctxt axioms*)
+           fs[init_ctxt_def,conexts_of_upd_def])
+       >- (rename1 `ctxt0 ++ upd::ctxt1` >>
+           first_x_assum(qspec_then `ctxt0 ++ [upd]` mp_tac) >>
+           PURE_REWRITE_TAC[GSYM APPEND_ASSOC,APPEND] >>
+           strip_tac >>
+           qpat_x_assum `MEM _ _` (strip_assume_tac o SIMP_RULE bool_ss [FLAT,MAP,MEM_APPEND])
+           >- (* Axiom in update *)
+              (drule_then match_mp_tac interpretation_models_axioms_lemma >>
+               rfs[total_fragment_is_fragment] >>
+               drule_then (assume_tac o C MATCH_MP init_theory_ok) extends_theory_ok >>
+               imp_res_tac theory_ok_sig >>
+               fs[] >>
+               rw[DISJ_IMP_THM,FORALL_AND_THM] >>
+               imp_res_tac extends_appends >>
+               rveq >> simp[] >>
+               dxrule_then (assume_tac o C MATCH_MP init_theory_ok) extends_theory_ok >>
+               dxrule_then (assume_tac o C MATCH_MP init_theory_ok) extends_theory_ok >>
+               imp_res_tac theory_ok_sig >>
+               fs[] >-
+                 metis_tac[] >-
+                 (imp_res_tac axioms_admissibleE >> simp[]) >>
+               metis_tac[APPEND_ASSOC,APPEND]
+              )
+           >- (* Axiom in update (again) *)
+              (drule_then match_mp_tac interpretation_models_axioms_lemma >>
+               rfs[total_fragment_is_fragment] >>
+               drule_then (assume_tac o C MATCH_MP init_theory_ok) extends_theory_ok >>
+               imp_res_tac theory_ok_sig >>
+               fs[] >>
+               rw[DISJ_IMP_THM,FORALL_AND_THM] >>
+               imp_res_tac extends_appends >>
+               rveq >> simp[] >>
+               dxrule_then (assume_tac o C MATCH_MP init_theory_ok) extends_theory_ok >>
+               dxrule_then (assume_tac o C MATCH_MP init_theory_ok) extends_theory_ok >>
+               imp_res_tac theory_ok_sig >>
+               fs[] >-
+                 metis_tac[] >-
+                 (imp_res_tac axioms_admissibleE >> simp[]) >>
+               metis_tac[APPEND_ASSOC,APPEND]
+              )
+           >- (* Axiom not in update *)
+              (fs[] >> metis_tac[])
+          )
+      ) >>
+  first_x_assum (drule_then (qspec_then `[]` mp_tac)) >>
+  rw[] >> pop_assum match_mp_tac >>
+  fs[] >> metis_tac[]
 QED
 
 val _ = export_theory()
